<?xml version="1.0"?>
<rdf:RDF xmlns="http://purl.org/ai4se/ontology#"
     xml:base="http://purl.org/ai4se/ontology"
     xmlns:dc="http://purl.org/dc/elements/1.1/"
     xmlns:owl="http://www.w3.org/2002/07/owl#"
     xmlns:rdf="http://www.w3.org/1999/02/22-rdf-syntax-ns#"
     xmlns:xml="http://www.w3.org/XML/1998/namespace"
     xmlns:xsd="http://www.w3.org/2001/XMLSchema#"
     xmlns:gufo="http://purl.org/nemo/gufo#"
     xmlns:rdfs="http://www.w3.org/2000/01/rdf-schema#"
     xmlns:vann="http://purl.org/vocab/vann/"
     xmlns:ai4se="http://purl.org/ai4se/ontology#"
     xmlns:terms="http://purl.org/dc/terms/">
    <owl:Ontology rdf:about="http://purl.org/ai4se/ontology#">
        <owl:versionIRI rdf:resource="http://purl.org/ai4se/ontology#/1.0.0"/>
        <owl:imports rdf:resource="http://purl.org/nemo/gufo#/1.0.0"/>
        <dc:creator>Schieferdecker, Ina K.</dc:creator>
        <dc:title xml:lang="en">ai4se: A taxonomy of research papers on the support of software engineering (SE) through the use of artificial intelligence (AI) methods and techniques.</dc:title>
        <terms:bibliographicCitation xml:lang="en">Schieferdecker, I.K.: &quot;ai4se: A taxonomy of research papers on the support of software engineering (SE) through the use of artificial intelligence (AI) methods and techniques&quot;, 2025, http://purl.org/ai4se/doc</terms:bibliographicCitation>
        <terms:license>https://creativecommons.org/licenses/by/4.0/legalcode.en</terms:license>
        <vann:preferredNamespacePrefix xml:lang="en">ai4se</vann:preferredNamespacePrefix>
        <vann:preferredNamespaceUri rdf:datatype="http://www.w3.org/2001/XMLSchema#anyURI">http://purl.org/ai4se/ontology/</vann:preferredNamespaceUri>
        <rdfs:comment>An ontology of research papers generated from a BibTeX file.</rdfs:comment>
        <rdfs:comment xml:lang="en">tbd</rdfs:comment>
        <rdfs:label>AI for SE Ontology</rdfs:label>
        <owl:versionInfo rdf:datatype="http://www.w3.org/2001/XMLSchema#integer">2</owl:versionInfo>
    </owl:Ontology>
    


    <!-- 
    ///////////////////////////////////////////////////////////////////////////////////////
    //
    // Object Properties
    //
    ///////////////////////////////////////////////////////////////////////////////////////
     -->

    


    <!-- http://purl.org/ai4se/ontology#belongsTo -->

    <owl:ObjectProperty rdf:about="http://purl.org/ai4se/ontology#belongsTo">
        <rdf:type rdf:resource="http://www.w3.org/2002/07/owl#AsymmetricProperty"/>
        <rdf:type rdf:resource="http://www.w3.org/2002/07/owl#IrreflexiveProperty"/>
        <rdfs:domain rdf:resource="http://purl.org/nemo/gufo#AbstractIndividualType"/>
        <rdfs:range rdf:resource="http://purl.org/nemo/gufo#AbstractIndividualType"/>
    </owl:ObjectProperty>
    


    <!-- http://purl.org/ai4se/ontology#belongsToAIType -->

    <owl:ObjectProperty rdf:about="http://purl.org/ai4se/ontology#belongsToAIType">
        <rdfs:subPropertyOf rdf:resource="http://purl.org/ai4se/ontology#belongsTo"/>
        <rdfs:domain rdf:resource="http://purl.org/ai4se/ontology#AIType"/>
        <rdfs:range rdf:resource="http://purl.org/ai4se/ontology#AIType"/>
    </owl:ObjectProperty>
    


    <!-- http://purl.org/ai4se/ontology#belongsToSEActivity -->

    <owl:ObjectProperty rdf:about="http://purl.org/ai4se/ontology#belongsToSEActivity">
        <rdfs:subPropertyOf rdf:resource="http://purl.org/ai4se/ontology#belongsTo"/>
        <rdfs:domain rdf:resource="http://purl.org/ai4se/ontology#Target"/>
        <rdfs:range rdf:resource="http://purl.org/ai4se/ontology#Target"/>
    </owl:ObjectProperty>
    


    <!-- http://purl.org/ai4se/ontology#hasLevel -->

    <owl:ObjectProperty rdf:about="http://purl.org/ai4se/ontology#hasLevel">
        <rdfs:subPropertyOf rdf:resource="http://purl.org/nemo/gufo#hasAssociatedQualityValueType"/>
        <owl:inverseOf rdf:resource="http://purl.org/ai4se/ontology#levelEnabledBy"/>
        <rdfs:domain rdf:resource="http://purl.org/ai4se/ontology#ResearchPaper"/>
        <rdfs:range rdf:resource="http://purl.org/ai4se/ontology#AutomationLevel"/>
    </owl:ObjectProperty>
    


    <!-- http://purl.org/ai4se/ontology#hasPurpose -->

    <owl:ObjectProperty rdf:about="http://purl.org/ai4se/ontology#hasPurpose">
        <rdfs:subPropertyOf rdf:resource="http://purl.org/nemo/gufo#hasAssociatedQualityValueType"/>
        <owl:inverseOf rdf:resource="http://purl.org/ai4se/ontology#purposeAdressedBy"/>
        <rdfs:domain rdf:resource="http://purl.org/ai4se/ontology#ResearchPaper"/>
        <rdfs:range rdf:resource="http://purl.org/ai4se/ontology#SolutionPurpose"/>
    </owl:ObjectProperty>
    


    <!-- http://purl.org/ai4se/ontology#hasTarget -->

    <owl:ObjectProperty rdf:about="http://purl.org/ai4se/ontology#hasTarget">
        <rdfs:subPropertyOf rdf:resource="http://purl.org/nemo/gufo#hasAssociatedQualityValueType"/>
        <owl:inverseOf rdf:resource="http://purl.org/ai4se/ontology#targetFocussedBy"/>
        <rdfs:domain rdf:resource="http://purl.org/ai4se/ontology#ResearchPaper"/>
        <rdfs:range rdf:resource="http://purl.org/ai4se/ontology#Target"/>
    </owl:ObjectProperty>
    


    <!-- http://purl.org/ai4se/ontology#hasType -->

    <owl:ObjectProperty rdf:about="http://purl.org/ai4se/ontology#hasType">
        <rdfs:subPropertyOf rdf:resource="http://purl.org/nemo/gufo#hasAssociatedQualityValueType"/>
        <owl:inverseOf rdf:resource="http://purl.org/ai4se/ontology#typeUsedBy"/>
        <rdfs:domain rdf:resource="http://purl.org/ai4se/ontology#ResearchPaper"/>
        <rdfs:range rdf:resource="http://purl.org/ai4se/ontology#AIType"/>
    </owl:ObjectProperty>
    


    <!-- http://purl.org/ai4se/ontology#implementedIn -->

    <owl:ObjectProperty rdf:about="http://purl.org/ai4se/ontology#implementedIn">
        <rdfs:domain rdf:resource="http://purl.org/nemo/gufo#AbstractIndividualType"/>
        <rdfs:range rdf:resource="http://purl.org/nemo/gufo#EndurantType"/>
    </owl:ObjectProperty>
    


    <!-- http://purl.org/ai4se/ontology#isAboutResearchTopic -->

    <owl:ObjectProperty rdf:about="http://purl.org/ai4se/ontology#isAboutResearchTopic">
        <rdfs:subPropertyOf rdf:resource="http://purl.org/nemo/gufo#hasAssociatedQualityValueType"/>
        <owl:inverseOf rdf:resource="http://purl.org/ai4se/ontology#topicAddressedBy"/>
        <rdfs:domain rdf:resource="http://purl.org/ai4se/ontology#ResearchPaper"/>
        <rdfs:range rdf:resource="http://purl.org/ai4se/ontology#CSO:Topic"/>
        <rdfs:comment xml:lang="en">Represents the research topics that a research paper contributes to.</rdfs:comment>
        <rdfs:label>isAboutResearchTopic</rdfs:label>
    </owl:ObjectProperty>
    


    <!-- http://purl.org/ai4se/ontology#isProperPartOfProcess -->

    <owl:ObjectProperty rdf:about="http://purl.org/ai4se/ontology#isProperPartOfProcess">
        <rdfs:subPropertyOf rdf:resource="http://purl.org/nemo/gufo#isEventProperPartOf"/>
        <rdfs:comment xml:lang="en">Represents activities being part of processes.</rdfs:comment>
        <rdfs:label>isPartOfProcess</rdfs:label>
    </owl:ObjectProperty>
    


    <!-- http://purl.org/ai4se/ontology#isSEActivityWithModels -->

    <owl:ObjectProperty rdf:about="http://purl.org/ai4se/ontology#isSEActivityWithModels">
        <rdfs:subPropertyOf rdf:resource="http://purl.org/nemo/gufo#mediates"/>
        <rdfs:range rdf:resource="http://purl.org/ai4se/ontology#Model"/>
    </owl:ObjectProperty>
    


    <!-- http://purl.org/ai4se/ontology#levelEnabledBy -->

    <owl:ObjectProperty rdf:about="http://purl.org/ai4se/ontology#levelEnabledBy">
        <rdfs:subPropertyOf rdf:resource="http://purl.org/ai4se/ontology#implementedIn"/>
        <rdfs:domain rdf:resource="http://purl.org/ai4se/ontology#AutomationLevel"/>
        <rdfs:range rdf:resource="http://purl.org/ai4se/ontology#ResearchPaper"/>
    </owl:ObjectProperty>
    


    <!-- http://purl.org/ai4se/ontology#purposeAdressedBy -->

    <owl:ObjectProperty rdf:about="http://purl.org/ai4se/ontology#purposeAdressedBy">
        <rdfs:subPropertyOf rdf:resource="http://purl.org/ai4se/ontology#implementedIn"/>
        <rdfs:domain rdf:resource="http://purl.org/ai4se/ontology#SolutionPurpose"/>
        <rdfs:range rdf:resource="http://purl.org/ai4se/ontology#ResearchPaper"/>
    </owl:ObjectProperty>
    


    <!-- http://purl.org/ai4se/ontology#targetFocussedBy -->

    <owl:ObjectProperty rdf:about="http://purl.org/ai4se/ontology#targetFocussedBy">
        <rdfs:subPropertyOf rdf:resource="http://purl.org/ai4se/ontology#implementedIn"/>
        <rdfs:domain rdf:resource="http://purl.org/ai4se/ontology#Target"/>
        <rdfs:range rdf:resource="http://purl.org/ai4se/ontology#ResearchPaper"/>
    </owl:ObjectProperty>
    


    <!-- http://purl.org/ai4se/ontology#topicAddressedBy -->

    <owl:ObjectProperty rdf:about="http://purl.org/ai4se/ontology#topicAddressedBy">
        <rdfs:subPropertyOf rdf:resource="http://purl.org/ai4se/ontology#implementedIn"/>
        <rdfs:domain rdf:resource="http://purl.org/ai4se/ontology#CSO:Topic"/>
        <rdfs:range rdf:resource="http://purl.org/ai4se/ontology#ResearchPaper"/>
    </owl:ObjectProperty>
    


    <!-- http://purl.org/ai4se/ontology#typeUsedBy -->

    <owl:ObjectProperty rdf:about="http://purl.org/ai4se/ontology#typeUsedBy">
        <rdfs:subPropertyOf rdf:resource="http://purl.org/ai4se/ontology#implementedIn"/>
        <rdfs:domain rdf:resource="http://purl.org/ai4se/ontology#AIType"/>
        <rdfs:range rdf:resource="http://purl.org/ai4se/ontology#ResearchPaper"/>
    </owl:ObjectProperty>
    


    <!-- 
    ///////////////////////////////////////////////////////////////////////////////////////
    //
    // Classes
    //
    ///////////////////////////////////////////////////////////////////////////////////////
     -->

    


    <!-- http://purl.org/ai4se/ontology#AIType -->

    <owl:Class rdf:about="http://purl.org/ai4se/ontology#AIType">
        <rdfs:subClassOf rdf:resource="http://purl.org/nemo/gufo#AbstractIndividualType"/>
        <rdfs:comment xml:lang="en">Represents the type of the artificial intelligence (AI) system being used.

According to ISO/IEC 22989:2022 Information technology - Artificial intelligence - Artificial intelligence concepts and terminology, artificial intelligence (AI) is

- &lt;discipline&gt; research and development of mechanisms and applications of AI systems.

and

artificial intelligence system (AI system) is

- engineered system that generates outputs such as content, forecasts, recommendations or decisions for a given set of human-defined objectives.</rdfs:comment>
        <rdfs:label>Type of AI system</rdfs:label>
    </owl:Class>
    


    <!-- http://purl.org/ai4se/ontology#AutomationLevel -->

    <owl:Class rdf:about="http://purl.org/ai4se/ontology#AutomationLevel">
        <rdfs:subClassOf rdf:resource="http://purl.org/nemo/gufo#AbstractIndividualType"/>
        <rdfs:label>Level of AI automation</rdfs:label>
        <rdfs:label xml:lang="en">Represents the level of automation provided / enabled by the AI system being used.

According to ISO/IEC 22989:2022 Information technology - Artificial intelligence - Artificial intelligence concepts and terminology, artificial intelligence (AI) is

- &lt;discipline&gt; research and development of mechanisms and applications of AI systems.

and

artificial intelligence system (AI system) is

- engineered system that generates outputs such as content, forecasts, recommendations or decisions for a given set of human-defined objectives.</rdfs:label>
    </owl:Class>
    


    <!-- http://purl.org/ai4se/ontology#Miscellaneous -->

    <owl:Class rdf:about="http://purl.org/ai4se/ontology#Miscellaneous">
        <rdfs:comment xml:lang="en">This is a collection of the fundamental concepts of the software development life cycle.

As no comprehensive, predefined ontology is available from SWEBOK, ISO, IEC, IEEE, or other sources, a lightweight approach was taken for the ai4se ontology: Fundamental concepts of SDLC needed for the understanding of ai4se are collected and definitions are referred to from selected sources.</rdfs:comment>
        <rdfs:isDefinedBy>610.12-1990 - IEEE Standard Glossary of Software Engineering Terminology:

https://ieeexplore.ieee.org/document/159342</rdfs:isDefinedBy>
        <rdfs:isDefinedBy>SWEBOK v4.0: Software Engineering Body of Knowledge 

https://www.computer.org/education/bodies-of-knowledge/software-engineering</rdfs:isDefinedBy>
        <rdfs:label>Misc</rdfs:label>
    </owl:Class>
    


    <!-- http://purl.org/ai4se/ontology#Model -->

    <owl:Class rdf:about="http://purl.org/ai4se/ontology#Model">
        <rdfs:subClassOf rdf:resource="http://purl.org/nemo/gufo#Mixin"/>
        <rdfs:comment xml:lang="en">Represents artifacts defining (semi-)formally (1) properties of one or more artefacts used by software engineering activities or processes or (2) properties of software engineering activities or processes.

According to ISO/IEC 22989:2022 Information technology - Artificial intelligence - Artificial intelligence concepts and terminology, model is

- physical, mathematical or otherwise logical representation of a system, entity, phenomenon, process or data.

Note: For the AI4SE ontology, only mathematical or logical representations are relevant.</rdfs:comment>
        <rdfs:label>Model</rdfs:label>
    </owl:Class>
    


    <!-- http://purl.org/ai4se/ontology#ResearchPaper -->

    <owl:Class rdf:about="http://purl.org/ai4se/ontology#ResearchPaper">
        <rdfs:subClassOf rdf:resource="http://purl.org/nemo/gufo#Mixin"/>
        <rdfs:comment xml:lang="en">Represents an artifact documenting research findings like new insights, methods, techniques, etc.</rdfs:comment>
        <rdfs:label>ResearchPaper</rdfs:label>
    </owl:Class>
    


    <!-- http://purl.org/ai4se/ontology#SolutionPurpose -->

    <owl:Class rdf:about="http://purl.org/ai4se/ontology#SolutionPurpose">
        <rdfs:subClassOf rdf:resource="http://purl.org/nemo/gufo#AbstractIndividualType"/>
        <rdfs:comment xml:lang="en">Represents the purpose of using the AI system in a software development / operation processes or activities.</rdfs:comment>
        <rdfs:label>Solution purpose</rdfs:label>
    </owl:Class>
    


    <!-- http://purl.org/ai4se/ontology#Target -->

    <owl:Class rdf:about="http://purl.org/ai4se/ontology#Target">
        <rdfs:subClassOf rdf:resource="http://purl.org/nemo/gufo#AbstractIndividualType"/>
        <rdfs:comment xml:lang="en">Represents the primary concept, issue, component, software, or process in a software engineering process or activitiy being addressed.</rdfs:comment>
        <rdfs:label>Solution target</rdfs:label>
    </owl:Class>
    


    <!-- http://purl.org/ai4se/ontology#CSO:Topic -->

    <owl:Class rdf:about="http://purl.org/ai4se/ontology#CSO:Topic">
        <rdfs:subClassOf rdf:resource="http://purl.org/ai4se/ontology#Miscellaneous"/>
        <rdfs:subClassOf rdf:resource="http://purl.org/nemo/gufo#AbstractIndividualType"/>
        <rdfs:isDefinedBy>https://cso.kmi.open.ac.uk/</rdfs:isDefinedBy>
        <rdfs:label>CSO:Topic</rdfs:label>
        <rdfs:label xml:lang="en">Represents the research topics in Computer Science as defined by the Computer Science Ontology CSO.</rdfs:label>
    </owl:Class>
    


    <!-- 
    ///////////////////////////////////////////////////////////////////////////////////////
    //
    // Individuals
    //
    ///////////////////////////////////////////////////////////////////////////////////////
     -->

    


    <!-- http://purl.org/ai4se/ontology#AI-assisted_options -->

    <owl:NamedIndividual rdf:about="http://purl.org/ai4se/ontology#AI-assisted_options">
        <rdf:type rdf:resource="http://purl.org/ai4se/ontology#AutomationLevel"/>
        <rdfs:comment xml:lang="en">Represents the case in which choices, recommendations, or decision-support outputs for the target SE processes or activities are generated or enhanced by an AI system, while retaining human control over the final choice, recommendation or decision, which may differ from the AI outputs.</rdfs:comment>
        <rdfs:label>AI-assisted options</rdfs:label>
    </owl:NamedIndividual>
    


    <!-- http://purl.org/ai4se/ontology#AI-assisted_selection -->

    <owl:NamedIndividual rdf:about="http://purl.org/ai4se/ontology#AI-assisted_selection">
        <rdf:type rdf:resource="http://purl.org/ai4se/ontology#AutomationLevel"/>
        <rdfs:comment xml:lang="en">Represents the case in which choices, recommendations, or decision-support outputs for the target SE processes or activities are generated or enhanced by an AI system, where the final choices, recommendations or decisions require human confirmation and do not differ from the AI outputs.</rdfs:comment>
        <rdfs:label>AI-assisted selection</rdfs:label>
    </owl:NamedIndividual>
    


    <!-- http://purl.org/ai4se/ontology#AI-driven_full_automation -->

    <owl:NamedIndividual rdf:about="http://purl.org/ai4se/ontology#AI-driven_full_automation">
        <rdf:type rdf:resource="http://purl.org/ai4se/ontology#AutomationLevel"/>
        <rdfs:comment xml:lang="en">Represents the case in which AI is used to automate all tasks or decision-making components within the target SE processes or activities, without requiring human intervention.</rdfs:comment>
        <rdfs:label>AI-driven full automation</rdfs:label>
    </owl:NamedIndividual>
    


    <!-- http://purl.org/ai4se/ontology#AI-driven_partial_automation -->

    <owl:NamedIndividual rdf:about="http://purl.org/ai4se/ontology#AI-driven_partial_automation">
        <rdf:type rdf:resource="http://purl.org/ai4se/ontology#AutomationLevel"/>
        <rdfs:comment xml:lang="en">Represents the case in which AI is used to automate specific tasks or decision-making components within the target SE processes or activities, while other parts of the process remain under human control or require human intervention.</rdfs:comment>
        <rdfs:label>AI-driven partial automation</rdfs:label>
    </owl:NamedIndividual>
    


    <!-- http://purl.org/ai4se/ontology#Agentic_AI -->

    <owl:NamedIndividual rdf:about="http://purl.org/ai4se/ontology#Agentic_AI">
        <rdf:type rdf:resource="http://purl.org/ai4se/ontology#AIType"/>
        <rdfs:comment xml:lang="en">Represents AI systems that rely on autonomous agents using AI techniques to plan, adapt, and execute multi-step objectives with minimal human control.</rdfs:comment>
        <rdfs:label>Agentic AI</rdfs:label>
    </owl:NamedIndividual>
    


    <!-- http://purl.org/ai4se/ontology#Architecture_and_Design -->

    <owl:NamedIndividual rdf:about="http://purl.org/ai4se/ontology#Architecture_and_Design">
        <rdf:type rdf:resource="http://purl.org/ai4se/ontology#Target"/>
        <belongsToSEActivity rdf:resource="http://purl.org/ai4se/ontology#Develop"/>
        <rdfs:comment xml:lang="en">Represents software architecture and design activities and processes. 

A software architecture defines its fundamental organization, its components, their relationships, and the principles guiding its design and evolution. 
 
According to ISO/IEC/IEEE 42010:2022: Software, systems and enterprise - Architecture description), a software architecture consists of the fundamental concepts or properties of an entity in its environment and governing principles for the realization and evolution of this entity and its related life cycle processes.

Software design is the process of defining the architecture, components, interfaces, and other characteristics of a software or a component.

According to ISO/IEC/IEEE 24765: Systems and software engineering - Vocabulary, software design is  

1. the use of scientific principles, technical information, and imagination in the definition of a software system to perform pre-specified functions with maximum economy and efficiency.</rdfs:comment>
        <rdfs:label>Software architecture and design</rdfs:label>
    </owl:NamedIndividual>
    


    <!-- http://purl.org/ai4se/ontology#Classical_machine_learning -->

    <owl:NamedIndividual rdf:about="http://purl.org/ai4se/ontology#Classical_machine_learning">
        <rdf:type rdf:resource="http://purl.org/ai4se/ontology#AIType"/>
        <belongsToAIType rdf:resource="http://purl.org/ai4se/ontology#Subsymbolic"/>
        <rdfs:comment xml:lang="en">Represents subsymbolic AI systems that rely on statistical and algorithmic learning techniques - such as decision trees, support vector machines, linear regression, and clustering - to learn patterns from structured data and make predictions or classifications. These models typically operate on explicitly defined features and do not involve deep neural networks.

This class of AI is used in contrast to deep learning AI.</rdfs:comment>
        <rdfs:label>Classical machine learning</rdfs:label>
    </owl:NamedIndividual>
    


    <!-- http://purl.org/ai4se/ontology#Coding -->

    <owl:NamedIndividual rdf:about="http://purl.org/ai4se/ontology#Coding">
        <rdf:type rdf:resource="http://purl.org/ai4se/ontology#Target"/>
        <belongsToSEActivity rdf:resource="http://purl.org/ai4se/ontology#Develop"/>
        <rdfs:comment xml:lang="en">Represents coding activities and processes. 

Coding (also known as programming) is the process of transforming the design of a software or a component into an executable computer program.

According to ISO/IEC/IEEE 24765: Systems and software engineering - Vocabulary, coding is

1. in software engineering, the process of expressing a computer program in a programming language

2. transforming of logic and data from design specifications (design descriptions) into a programming language.</rdfs:comment>
        <rdfs:label>Software coding</rdfs:label>
    </owl:NamedIndividual>
    


    <!-- http://purl.org/ai4se/ontology#Deep_learning -->

    <owl:NamedIndividual rdf:about="http://purl.org/ai4se/ontology#Deep_learning">
        <rdf:type rdf:resource="http://purl.org/ai4se/ontology#AIType"/>
        <belongsToAIType rdf:resource="http://purl.org/ai4se/ontology#Subsymbolic"/>
        <rdfs:comment xml:lang="en">Represents subsymbolic AI systems that rely on deep artificial neural networks to automatically learn features and perform tasks such as classification or prediction, especially from large and complex datasets. 

According to ISO/IEC 22989:2022 Information technology - Artificial intelligence - Artificial intelligence concepts and terminology, deep learning (deep neural network learning) is

- AI approach to creating rich hierarchical representations through the training of neural networks with many hidden layers.</rdfs:comment>
        <rdfs:label>Deep learning AI</rdfs:label>
    </owl:NamedIndividual>
    


    <!-- http://purl.org/ai4se/ontology#Deployment -->

    <owl:NamedIndividual rdf:about="http://purl.org/ai4se/ontology#Deployment">
        <rdf:type rdf:resource="http://purl.org/ai4se/ontology#Target"/>
        <belongsToSEActivity rdf:resource="http://purl.org/ai4se/ontology#Operate"/>
        <rdfs:comment xml:lang="en">Represents software deployment activities and processes.

Software deployment encompasses the processes and activities for placing a software or component into an operational environment.

According to ISO/IEC/IEEE 24765: Systems and software engineering - Vocabulary, deployment is 

1. a phase of a project in which a system is put into operation and cutover issues are resolved.</rdfs:comment>
        <rdfs:label>Software deployment</rdfs:label>
    </owl:NamedIndividual>
    


    <!-- http://purl.org/ai4se/ontology#Develop -->

    <owl:NamedIndividual rdf:about="http://purl.org/ai4se/ontology#Develop">
        <rdf:type rdf:resource="http://purl.org/ai4se/ontology#Target"/>
        <belongsToSEActivity rdf:resource="http://purl.org/ai4se/ontology#Software_Engineering"/>
        <rdfs:label>Develop</rdfs:label>
        <rdfs:label xml:lang="en">Represents software development activities and processes.

Software development is the set of activities that result in software products, including requirements analysis, design, coding, testing, and maintenance. It encompasses all the activities and processes involved in creating, implementing, and modifying software (artefacts), as well as ensuring that it satisfies stakeholder requirements throughout the software development life cycle.</rdfs:label>
    </owl:NamedIndividual>
    


    <!-- http://purl.org/ai4se/ontology#General_AI -->

    <owl:NamedIndividual rdf:about="http://purl.org/ai4se/ontology#General_AI">
        <rdf:type rdf:resource="http://purl.org/ai4se/ontology#AIType"/>
        <rdfs:comment xml:lang="en">Represents AI systems capable of performing a broad set of distinct tasks with satisfactory performance.

According to ISO/IEC 22989:2022 Information technology - Artificial intelligence - Artificial intelligence concepts and terminology, general AI (AGI, artificial general intelligence)

- type of AI system that addresses a broad range of tasks with a satisfactory level of performance 

Note 1: Compared to narrow AI.
Note 2: AGI is often used in a stronger sense, meaning systems that not only can perform a wide variety of tasks, but all tasks that a human can perform.</rdfs:comment>
        <rdfs:label>General AI</rdfs:label>
    </owl:NamedIndividual>
    


    <!-- http://purl.org/ai4se/ontology#Generate -->

    <owl:NamedIndividual rdf:about="http://purl.org/ai4se/ontology#Generate">
        <rdf:type rdf:resource="http://purl.org/ai4se/ontology#SolutionPurpose"/>
    </owl:NamedIndividual>
    


    <!-- http://purl.org/ai4se/ontology#Generative_AI -->

    <owl:NamedIndividual rdf:about="http://purl.org/ai4se/ontology#Generative_AI">
        <rdf:type rdf:resource="http://purl.org/ai4se/ontology#AIType"/>
        <rdfs:comment xml:lang="en">Represents AI systems that use learned or derived knowledge to produce original outputs, such as synthetic text, media, or other content types. It often uses subsymbolic AI like Convolutional Neural Networks (CNNs), Recurrent Neural Networks (RNNs), or Transformer-based models, but also symbolic AI.</rdfs:comment>
        <rdfs:label>Generative AI</rdfs:label>
    </owl:NamedIndividual>
    


    <!-- http://purl.org/ai4se/ontology#Improve -->

    <owl:NamedIndividual rdf:about="http://purl.org/ai4se/ontology#Improve">
        <rdf:type rdf:resource="http://purl.org/ai4se/ontology#SolutionPurpose"/>
        <rdfs:comment xml:lang="en">The purpose of using AI is to improve (parts of) artefacts used in software engineering.</rdfs:comment>
        <rdfs:label>Improve</rdfs:label>
    </owl:NamedIndividual>
    


    <!-- http://purl.org/ai4se/ontology#Improvement -->

    <owl:NamedIndividual rdf:about="http://purl.org/ai4se/ontology#Improvement">
        <rdf:type rdf:resource="http://purl.org/ai4se/ontology#Target"/>
        <belongsToSEActivity rdf:resource="http://purl.org/ai4se/ontology#Process"/>
    </owl:NamedIndividual>
    


    <!-- http://purl.org/ai4se/ontology#Maintenance -->

    <owl:NamedIndividual rdf:about="http://purl.org/ai4se/ontology#Maintenance">
        <rdf:type rdf:resource="http://purl.org/ai4se/ontology#Target"/>
        <belongsToSEActivity rdf:resource="http://purl.org/ai4se/ontology#Develop"/>
        <rdfs:comment xml:lang="en">Represents software maintenance activities and processes. 

Software maintenance is the process of modifying a software or component after delivery to correct faults, improve performance or other attributes, or adapt to a changed environment.

According to ISO/IEC/IEEE 24765: Systems and software engineering - Vocabulary, software maintenance is 

1. totality of activities required to provide cost-effective support to a software system 

2. entitlement of additional rights (such as additional
functionality, upgrade or support) for a previously granted software entitlement</rdfs:comment>
        <rdfs:label>Software maintenance</rdfs:label>
    </owl:NamedIndividual>
    


    <!-- http://purl.org/ai4se/ontology#Management -->

    <owl:NamedIndividual rdf:about="http://purl.org/ai4se/ontology#Management">
        <rdf:type rdf:resource="http://purl.org/ai4se/ontology#Target"/>
        <belongsToSEActivity rdf:resource="http://purl.org/ai4se/ontology#Process"/>
    </owl:NamedIndividual>
    


    <!-- http://purl.org/ai4se/ontology#Monitoring -->

    <owl:NamedIndividual rdf:about="http://purl.org/ai4se/ontology#Monitoring">
        <rdf:type rdf:resource="http://purl.org/ai4se/ontology#Target"/>
        <belongsToSEActivity rdf:resource="http://purl.org/ai4se/ontology#Operate"/>
        <rdfs:comment xml:lang="en">Represents software monitoring activities and processes.

Software monitoring is systematically observing, checking, or keeping track of the operations or performance of a software or component.</rdfs:comment>
        <rdfs:label>Software monitoring</rdfs:label>
    </owl:NamedIndividual>
    


    <!-- http://purl.org/ai4se/ontology#No_AI_support -->

    <owl:NamedIndividual rdf:about="http://purl.org/ai4se/ontology#No_AI_support">
        <rdf:type rdf:resource="http://purl.org/ai4se/ontology#AutomationLevel"/>
        <rdfs:comment xml:lang="en">Represents the case in which the target SE processes or activities are performed without the assistance of AI.</rdfs:comment>
        <rdfs:label>No AI-supported automation</rdfs:label>
    </owl:NamedIndividual>
    


    <!-- http://purl.org/ai4se/ontology#Operate -->

    <owl:NamedIndividual rdf:about="http://purl.org/ai4se/ontology#Operate">
        <rdf:type rdf:resource="http://purl.org/ai4se/ontology#Target"/>
        <belongsToSEActivity rdf:resource="http://purl.org/ai4se/ontology#Software_Engineering"/>
        <rdfs:comment xml:lang="en">Represents software operation activities and processs.</rdfs:comment>
        <rdfs:label>Operate</rdfs:label>
    </owl:NamedIndividual>
    


    <!-- http://purl.org/ai4se/ontology#Operation -->

    <owl:NamedIndividual rdf:about="http://purl.org/ai4se/ontology#Operation">
        <rdf:type rdf:resource="http://purl.org/ai4se/ontology#Target"/>
        <belongsToSEActivity rdf:resource="http://purl.org/ai4se/ontology#Operate"/>
        <rdfs:comment xml:lang="en">Represents software operation activities and processes.

Software operation refers to

1. The use and execution of software in its production environment to perform its intended functions.

2. Running a software to deliver services or perform tasks for users or other systems.</rdfs:comment>
        <rdfs:label>Software operation</rdfs:label>
    </owl:NamedIndividual>
    


    <!-- http://purl.org/ai4se/ontology#Process -->

    <owl:NamedIndividual rdf:about="http://purl.org/ai4se/ontology#Process">
        <rdf:type rdf:resource="http://purl.org/ai4se/ontology#Target"/>
        <belongsToSEActivity rdf:resource="http://purl.org/ai4se/ontology#Software_Engineering"/>
        <rdfs:label xml:lang="en">Represents processes for software engineering along the software lifecycle of software development and operation.</rdfs:label>
        <rdfs:label>Software Engineering Processes</rdfs:label>
    </owl:NamedIndividual>
    


    <!-- http://purl.org/ai4se/ontology#Requirements -->

    <owl:NamedIndividual rdf:about="http://purl.org/ai4se/ontology#Requirements">
        <rdf:type rdf:resource="http://purl.org/ai4se/ontology#Target"/>
        <belongsToSEActivity rdf:resource="http://purl.org/ai4se/ontology#Develop"/>
        <rdfs:comment xml:lang="en">Represents requirements engineering activities and processes. 

A software requirement is a condition or capability that must be met by a software or component.

According to ISO/IEC/IEEE 24765: Systems and software engineering - Vocabulary, software requirement is

1. software capability needed by a user to solve a problem or to achieve an objective

2. software capability that must be met or possessed by a system or system component to satisfy a contract, standard, specification, or other formally imposed document

According to ISO/IEC/IEEE 24765: Systems and software engineering - Vocabulary, software requirements engineering is

1. science and discipline concerned with analyzing and documenting software requirements 

2. software requirements elicitation, analysis, specification, verification, and management</rdfs:comment>
        <rdfs:label>Requirements engineering</rdfs:label>
    </owl:NamedIndividual>
    


    <!-- http://purl.org/ai4se/ontology#Software_Engineering -->

    <owl:NamedIndividual rdf:about="http://purl.org/ai4se/ontology#Software_Engineering">
        <rdf:type rdf:resource="http://purl.org/ai4se/ontology#Target"/>
    </owl:NamedIndividual>
    


    <!-- http://purl.org/ai4se/ontology#Statistical -->

    <owl:NamedIndividual rdf:about="http://purl.org/ai4se/ontology#Statistical">
        <rdf:type rdf:resource="http://purl.org/ai4se/ontology#AIType"/>
        <belongsToAIType rdf:resource="http://purl.org/ai4se/ontology#Subsymbolic"/>
        <rdfs:comment xml:lang="en">Represents subsymbolic AI systems that rely on data and statistical inference to identify patterns and make predictions.</rdfs:comment>
        <rdfs:label>Statistical AI</rdfs:label>
    </owl:NamedIndividual>
    


    <!-- http://purl.org/ai4se/ontology#Subsymbolic -->

    <owl:NamedIndividual rdf:about="http://purl.org/ai4se/ontology#Subsymbolic">
        <rdf:type rdf:resource="http://purl.org/ai4se/ontology#AIType"/>
        <rdfs:comment xml:lang="en">Represents AI systems that use numerical models to represent knowledge and computations, such as numerical optimisation and statistical learning, in order to model and solve problems.

According to ISO/IEC 22989:2022 Information technology - Artificial intelligence - Artificial intelligence concepts and terminology, subsymbolic AI is

- AI based on techniques and models that use an implicit encoding of information, that can be derived from experience or raw data.</rdfs:comment>
        <rdfs:label>Subsymbolic AI</rdfs:label>
    </owl:NamedIndividual>
    


    <!-- http://purl.org/ai4se/ontology#Symbolic -->

    <owl:NamedIndividual rdf:about="http://purl.org/ai4se/ontology#Symbolic">
        <rdf:type rdf:resource="http://purl.org/ai4se/ontology#AIType"/>
        <rdfs:comment xml:lang="en">Represents AI systems that use approaches relying on the explicit definition of symbols and rules representing knowledge and performing logical reasoning.

According to ISO/IEC 22989:2022 Information technology - Artificial intelligence - Artificial intelligence concepts and terminology, symbolic AI is

- AI based on techniques and models that manipulate symbols and structures according to explicitly defined rules to obtain inferences.</rdfs:comment>
        <rdfs:label>Symbolic AI</rdfs:label>
    </owl:NamedIndividual>
    


    <!-- http://purl.org/ai4se/ontology#Testing -->

    <owl:NamedIndividual rdf:about="http://purl.org/ai4se/ontology#Testing">
        <rdf:type rdf:resource="http://purl.org/ai4se/ontology#Target"/>
        <belongsToSEActivity rdf:resource="http://purl.org/ai4se/ontology#Develop"/>
        <rdfs:comment xml:lang="en">Represents software testing activities and processes.

Software testing encompasses the processes and activities used to evaluate the quality of a software or a component and of related artefacts.

According to ISO/IEC/IEEE 24765: Systems and software engineering - Vocabulary, software testing is

1. activity in which a system or component is executed under specified conditions, the results are observed or recorded, and an evaluation is made of some aspect of the system or component

2. dynamic verification that a program provides expected behaviors on a finite set of test cases, suitably selected from the usually infinite executions domain.</rdfs:comment>
        <rdfs:label>Software testing</rdfs:label>
    </owl:NamedIndividual>
    


    <!-- http://purl.org/ai4se/ontology#Understand -->

    <owl:NamedIndividual rdf:about="http://purl.org/ai4se/ontology#Understand">
        <rdf:type rdf:resource="http://purl.org/ai4se/ontology#SolutionPurpose"/>
        <rdfs:comment xml:lang="en">The purpose of using AI is to gain insight.</rdfs:comment>
        <rdfs:label>Understand</rdfs:label>
    </owl:NamedIndividual>
    


    <!-- http://purl.org/ai4se/ontology#ahmad_requirements_2023 -->

    <owl:NamedIndividual rdf:about="http://purl.org/ai4se/ontology#ahmad_requirements_2023">
        <rdf:type rdf:resource="http://purl.org/ai4se/ontology#ResearchPaper"/>
        <hasLevel rdf:resource="http://purl.org/ai4se/ontology#null"/>
        <hasPurpose rdf:resource="http://purl.org/ai4se/ontology#null"/>
        <hasTarget rdf:resource="http://purl.org/ai4se/ontology#null"/>
        <hasType rdf:resource="http://purl.org/ai4se/ontology#null"/>
        <isAboutResearchTopic rdf:resource="http://purl.org/ai4se/ontology#CSO:Testing_and_debugging"/>
        <rdfs:comment>@article{ahmad_requirements_2023,
 author = {Ahmad, Khlood and Abdelrazek, Mohamed and Arora, Chetan and Baniya, Arbind Agrahari and Bano, Muneera and Grundy, John},
 doi = {10.48550/ARXIV.2303.02920},
 journal = {CoRR},
 note = {arXiv: 2303.02920},
 title = {Requirements {Framework} for {Engineering} {Human}-centered {Artificial} {Intelligence}-{Based} {Software} {Systems}},
 url = {https://doi.org/10.48550/arXiv.2303.02920},
 volume = {abs/2303.02920},
 year = {2023}
}
</rdfs:comment>
        <rdfs:label>ahmad_requirements_2023</rdfs:label>
        <rdfs:seeAlso rdf:resource="https://doi.org/10.48550/arXiv.2303.02920"/>
    </owl:NamedIndividual>
    


    <!-- http://purl.org/ai4se/ontology#ahmad_towards_2023 -->

    <owl:NamedIndividual rdf:about="http://purl.org/ai4se/ontology#ahmad_towards_2023">
        <rdf:type rdf:resource="http://purl.org/ai4se/ontology#ResearchPaper"/>
        <hasLevel rdf:resource="http://purl.org/ai4se/ontology#null"/>
        <hasPurpose rdf:resource="http://purl.org/ai4se/ontology#null"/>
        <hasTarget rdf:resource="http://purl.org/ai4se/ontology#null"/>
        <hasType rdf:resource="http://purl.org/ai4se/ontology#null"/>
        <isAboutResearchTopic rdf:resource="http://purl.org/ai4se/ontology#CSO:Testing_and_debugging"/>
        <rdfs:comment>@inproceedings{ahmad_towards_2023,
 address = {Oulu Finland},
 author = {Ahmad, Aakash and Waseem, Muhammad and Liang, Peng and Fahmideh, Mahdi and Aktar, Mst Shamima and Mikkonen, Tommi},
 booktitle = {Proceedings of the 27th {International} {Conference} on {Evaluation} and {Assessment} in {Software} {Engineering}},
 doi = {10.1145/3593434.3593468},
  isbn = {979-8-4007-0044-6},
 language = {en},
 month = {June},
 pages = {279--285},
 publisher = {ACM},
 title = {Towards {Human}-{Bot} {Collaborative} {Software} {Architecting} with {ChatGPT}},
 url = {https://dl.acm.org/doi/10.1145/3593434.3593468},
 urldate = {2025-06-03},
 year = {2023}
}
</rdfs:comment>
        <rdfs:label>ahmad_towards_2023</rdfs:label>
        <rdfs:seeAlso rdf:resource="https://dl.acm.org/doi/10.1145/3593434.3593468"/>
    </owl:NamedIndividual>
    


    <!-- http://purl.org/ai4se/ontology#ajagbe_retraining_2022 -->

    <owl:NamedIndividual rdf:about="http://purl.org/ai4se/ontology#ajagbe_retraining_2022">
        <rdf:type rdf:resource="http://purl.org/ai4se/ontology#ResearchPaper"/>
        <hasLevel rdf:resource="http://purl.org/ai4se/ontology#null"/>
        <hasPurpose rdf:resource="http://purl.org/ai4se/ontology#null"/>
        <hasTarget rdf:resource="http://purl.org/ai4se/ontology#null"/>
        <hasType rdf:resource="http://purl.org/ai4se/ontology#null"/>
        <isAboutResearchTopic rdf:resource="http://purl.org/ai4se/ontology#CSO:Testing_and_debugging"/>
        <rdfs:comment>@inproceedings{ajagbe_retraining_2022,
 author = {Ajagbe, Muideen and Zhao, Liping},
 booktitle = {2022 {IEEE} 30th {International} {Requirements} {Engineering} {Conference} ({RE})},
 doi = {10.1109/RE54965.2022.00046},
  keywords = {Deep learning, Deep Learning, Machine Learning, BERT, Natural language processing, Requirements engineering, Transfer learning, Language Models, Task analysis, Natural Language Processing, Transfer Learning, Requirements Engineering, Bit error rate, Domain-Specific Language Models, Requirements Classification},
 month = {August},
 note = {ISSN: 2332-6441},
 pages = {309--315},
 shorttitle = {Retraining a {BERT} {Model} for {Transfer} {Learning} in {Requirements} {Engineering}},
 title = {Retraining a {BERT} {Model} for {Transfer} {Learning} in {Requirements} {Engineering}: {A} {Preliminary} {Study}},
 url = {https://ieeexplore.ieee.org/document/9920081},
 urldate = {2025-06-03},
 year = {2022}
}
</rdfs:comment>
        <rdfs:label>ajagbe_retraining_2022</rdfs:label>
        <rdfs:seeAlso rdf:resource="https://ieeexplore.ieee.org/document/9920081"/>
    </owl:NamedIndividual>
    


    <!-- http://purl.org/ai4se/ontology#akay_reading_2021 -->

    <owl:NamedIndividual rdf:about="http://purl.org/ai4se/ontology#akay_reading_2021">
        <rdf:type rdf:resource="http://purl.org/ai4se/ontology#ResearchPaper"/>
        <hasLevel rdf:resource="http://purl.org/ai4se/ontology#null"/>
        <hasPurpose rdf:resource="http://purl.org/ai4se/ontology#null"/>
        <hasTarget rdf:resource="http://purl.org/ai4se/ontology#null"/>
        <hasType rdf:resource="http://purl.org/ai4se/ontology#null"/>
        <isAboutResearchTopic rdf:resource="http://purl.org/ai4se/ontology#CSO:Testing_and_debugging"/>
        <rdfs:comment>@article{akay_reading_2021,
 author = {Akay, Haluk and Kim, Sang-Gook},
 doi = {10.1016/j.cirp.2021.04.021},
 issn = {00078506},
 journal = {CIRP Annals},
 language = {en},
 number = {1},
 pages = {139--142},
 title = {Reading functional requirements using machine learning-based language processing},
 url = {https://linkinghub.elsevier.com/retrieve/pii/S0007850621000457},
 urldate = {2025-06-03},
 volume = {70},
 year = {2021}
}
</rdfs:comment>
        <rdfs:label>akay_reading_2021</rdfs:label>
        <rdfs:seeAlso rdf:resource="https://linkinghub.elsevier.com/retrieve/pii/S0007850621000457"/>
    </owl:NamedIndividual>
    


    <!-- http://purl.org/ai4se/ontology#bader_getafix_2019 -->

    <owl:NamedIndividual rdf:about="http://purl.org/ai4se/ontology#bader_getafix_2019">
        <rdf:type rdf:resource="http://purl.org/ai4se/ontology#ResearchPaper"/>
        <hasLevel rdf:resource="http://purl.org/ai4se/ontology#AI-assisted_selection"/>
        <hasPurpose rdf:resource="http://purl.org/ai4se/ontology#Improve"/>
        <hasTarget rdf:resource="http://purl.org/ai4se/ontology#Coding"/>
        <hasTarget rdf:resource="http://purl.org/ai4se/ontology#Testing"/>
        <hasType rdf:resource="http://purl.org/ai4se/ontology#Classical_machine_learning"/>
        <isAboutResearchTopic rdf:resource="http://purl.org/ai4se/ontology#CSO:Testing_and_debugging"/>
        <rdfs:comment>@article{bader_getafix_2019,
 author = {Bader, Johannes and Scott, Andrew and Pradel, Michael and Chandra, Satish},
 doi = {10.1145/3360585},
 journal = {Proceedings of the ACM on Programming Languages},
 note = {Publisher: ACM New York, NY, USA},
 number = {OOPSLA},
 pages = {1--27},
 title = {Getafix: {Learning} to fix bugs automatically},
 volume = {3},
 year = {2019}
}
</rdfs:comment>
        <rdfs:label>bader_getafix_2019</rdfs:label>
        <rdfs:seeAlso rdf:resource="https://doi.org/10.1145/3360585"/>
    </owl:NamedIndividual>
    


    <!-- http://purl.org/ai4se/ontology#barstow_artificial_1987 -->

    <owl:NamedIndividual rdf:about="http://purl.org/ai4se/ontology#barstow_artificial_1987">
        <rdf:type rdf:resource="http://purl.org/ai4se/ontology#ResearchPaper"/>
        <hasLevel rdf:resource="http://purl.org/ai4se/ontology#null"/>
        <hasPurpose rdf:resource="http://purl.org/ai4se/ontology#null"/>
        <hasTarget rdf:resource="http://purl.org/ai4se/ontology#null"/>
        <hasType rdf:resource="http://purl.org/ai4se/ontology#null"/>
        <isAboutResearchTopic rdf:resource="http://purl.org/ai4se/ontology#CSO:Static_analysis"/>
        <rdfs:comment>@inproceedings{barstow_artificial_1987,
 author = {Barstow, David R.},
 booktitle = {Proceedings, 9th {International} {Conference} on {Software} {Engineering}, {Monterey}, {California}, {USA}, {March} 30 - {April} 2, 1987},
 editor = {Riddle, William E. and Balzer, Robert M. and Kishida, Kouichi},
 pages = {200--215},
 publisher = {ACM Press},
 title = {Artificial {Intelligence} and {Software} {Engineering}},
 url = {http://dl.acm.org/citation.cfm?id=41786},
 year = {1987}
}
</rdfs:comment>
        <rdfs:label>barstow_artificial_1987</rdfs:label>
        <rdfs:seeAlso rdf:resource="http://dl.acm.org/citation.cfm?id=41786"/>
    </owl:NamedIndividual>
    


    <!-- http://purl.org/ai4se/ontology#belli_coverage-oriented_2007 -->

    <owl:NamedIndividual rdf:about="http://purl.org/ai4se/ontology#belli_coverage-oriented_2007">
        <rdf:type rdf:resource="http://purl.org/ai4se/ontology#ResearchPaper"/>
        <hasLevel rdf:resource="http://purl.org/ai4se/ontology#null"/>
        <hasPurpose rdf:resource="http://purl.org/ai4se/ontology#null"/>
        <hasTarget rdf:resource="http://purl.org/ai4se/ontology#null"/>
        <hasType rdf:resource="http://purl.org/ai4se/ontology#null"/>
        <isAboutResearchTopic rdf:resource="http://purl.org/ai4se/ontology#CSO:Testing_and_debugging"/>
        <rdfs:comment>@article{belli_coverage-oriented_2007,
 author = {Belli, Fevzi and Belli, Fevzi and Eminov, Mübariz and Eminov, Mubariz and Eminov, Mubariz and Eminov, Mubariz and Gökçe, Nida and Gökçe, Nida},
 doi = {10.1007/978-3-540-75294-3_8},
 journal = {Latin-American Symposium on Dependable Computing},
 pmcid = {null},
 pmid = {null},
 title = {Coverage-oriented, prioritized testing: a fuzzy clustering approach and case study},
 year = {2007}
}
</rdfs:comment>
        <rdfs:label>belli_coverage-oriented_2007</rdfs:label>
        <rdfs:seeAlso rdf:resource="https://doi.org/10.1007/978-3-540-75294-3_8"/>
    </owl:NamedIndividual>
    


    <!-- http://purl.org/ai4se/ontology#bhat_adex_2019 -->

    <owl:NamedIndividual rdf:about="http://purl.org/ai4se/ontology#bhat_adex_2019">
        <rdf:type rdf:resource="http://purl.org/ai4se/ontology#ResearchPaper"/>
        <hasLevel rdf:resource="http://purl.org/ai4se/ontology#AI-assisted_selection"/>
        <hasPurpose rdf:resource="http://purl.org/ai4se/ontology#Improve"/>
        <hasPurpose rdf:resource="http://purl.org/ai4se/ontology#Understand"/>
        <hasTarget rdf:resource="http://purl.org/ai4se/ontology#Architecture_and_Design"/>
        <hasTarget rdf:resource="http://purl.org/ai4se/ontology#Deployment"/>
        <hasType rdf:resource="http://purl.org/ai4se/ontology#Classical_machine_learning"/>
        <isAboutResearchTopic rdf:resource="http://purl.org/ai4se/ontology#CSO:Traceability_management"/>
        <rdfs:comment>@inproceedings{bhat_adex_2019,
 author = {Bhat, Manoj and Tinnes, Christof and Shumaiev, Klym and Biesdorf, Andreas and Hohenstein, Uwe and Matthes, Florian},
 booktitle = {2019 {IEEE} {International} {Conference} on {Software} {Architecture} {Companion} ({ICSA}-{C})},
 doi = {10.1109/ICSA-C.2019.00035},
 pages = {158--161},
 publisher = {IEEE},
 title = {Adex: {A} tool for automatic curation of design decision knowledge for architectural decision recommendations},
 year = {2019}
}
</rdfs:comment>
        <rdfs:label>bhat_adex_2019</rdfs:label>
        <rdfs:seeAlso rdf:resource="https://doi.org/10.1109/ICSA-C.2019.00035"/>
    </owl:NamedIndividual>
    


    <!-- http://purl.org/ai4se/ontology#bhat_automatic_2017 -->

    <owl:NamedIndividual rdf:about="http://purl.org/ai4se/ontology#bhat_automatic_2017">
        <rdf:type rdf:resource="http://purl.org/ai4se/ontology#ResearchPaper"/>
        <hasLevel rdf:resource="http://purl.org/ai4se/ontology#null"/>
        <hasPurpose rdf:resource="http://purl.org/ai4se/ontology#null"/>
        <hasTarget rdf:resource="http://purl.org/ai4se/ontology#null"/>
        <hasType rdf:resource="http://purl.org/ai4se/ontology#null"/>
        <isAboutResearchTopic rdf:resource="http://purl.org/ai4se/ontology#CSO:Testing_and_debugging"/>
        <rdfs:comment>@article{bhat_automatic_2017,
 author = {Bhat, M. Seetharama and Bhat, Manoj and Shumaiev, Klym and Shumaiev, Klym and Biesdorf, Andreas and Biesdorf, Andreas and Hohenstein, Uwe and Hohenstein, Uwe and Matthes, Florian and Matthes, Florian},
 doi = {10.1007/978-3-319-65831-5_10},
 journal = {European Conference on Software Architecture},
 pmcid = {null},
 pmid = {null},
 title = {Automatic {Extraction} of {Design} {Decisions} from {Issue} {Management} {Systems}: {A} {Machine} {Learning} {Based} {Approach}},
 year = {2017}
}
</rdfs:comment>
        <rdfs:label>bhat_automatic_2017</rdfs:label>
        <rdfs:seeAlso rdf:resource="https://doi.org/10.1007/978-3-319-65831-5_10"/>
    </owl:NamedIndividual>
    


    <!-- http://purl.org/ai4se/ontology#bird_taking_2023 -->

    <owl:NamedIndividual rdf:about="http://purl.org/ai4se/ontology#bird_taking_2023">
        <rdf:type rdf:resource="http://purl.org/ai4se/ontology#ResearchPaper"/>
        <hasLevel rdf:resource="http://purl.org/ai4se/ontology#AI-assisted_selection"/>
        <hasPurpose rdf:resource="http://purl.org/ai4se/ontology#Generate"/>
        <hasPurpose rdf:resource="http://purl.org/ai4se/ontology#Understand"/>
        <hasTarget rdf:resource="http://purl.org/ai4se/ontology#Coding"/>
        <hasType rdf:resource="http://purl.org/ai4se/ontology#Generative_AI"/>
        <isAboutResearchTopic rdf:resource="http://purl.org/ai4se/ontology#CSO:Coding_technique"/>
        <rdfs:comment>@article{bird_taking_2023,
 author = {Bird, Christian and Ford, Denae and Zimmermann, Thomas and Forsgren, Nicole and Kalliamvakou, Eirini and Lowdermilk, Travis and Gazit, Idan},
 doi = {10.1145/3589996},
 issn = {0001-0782, 1557-7317},
 journal = {Communications of the ACM},
 language = {en},
 month = {June},
 number = {6},
 pages = {56--62},
 title = {Taking {Flight} with {Copilot}},
 url = {https://dl.acm.org/doi/10.1145/3589996},
 urldate = {2025-05-31},
 volume = {66},
 year = {2023}
}
</rdfs:comment>
        <rdfs:label>bird_taking_2023</rdfs:label>
        <rdfs:seeAlso rdf:resource="https://dl.acm.org/doi/10.1145/3589996"/>
    </owl:NamedIndividual>
    


    <!-- http://purl.org/ai4se/ontology#bouzenia_repairagent_2024 -->

    <owl:NamedIndividual rdf:about="http://purl.org/ai4se/ontology#bouzenia_repairagent_2024">
        <rdf:type rdf:resource="http://purl.org/ai4se/ontology#ResearchPaper"/>
        <hasLevel rdf:resource="http://purl.org/ai4se/ontology#AI-driven_partial_automation"/>
        <hasPurpose rdf:resource="http://purl.org/ai4se/ontology#Improve"/>
        <hasTarget rdf:resource="http://purl.org/ai4se/ontology#Coding"/>
        <hasType rdf:resource="http://purl.org/ai4se/ontology#Agentic_AI"/>
        <isAboutResearchTopic rdf:resource="http://purl.org/ai4se/ontology#CSO:Static_analysis"/>
        <rdfs:comment>@article{bouzenia_repairagent_2024,
 author = {Bouzenia, Islem and Devanbu, Premkumar and Pradel, Michael},
 doi = {10.48550/arXiv.2403.17134},
 journal = {arXiv preprint arXiv:2403.17134},
 title = {Repairagent: {An} autonomous, llm-based agent for program repair},
 year = {2024}
}
</rdfs:comment>
        <rdfs:label>bouzenia_repairagent_2024</rdfs:label>
        <rdfs:seeAlso rdf:resource="https://doi.org/10.48550/arXiv.2403.17134"/>
    </owl:NamedIndividual>
    


    <!-- http://purl.org/ai4se/ontology#burson_program_1990 -->

    <owl:NamedIndividual rdf:about="http://purl.org/ai4se/ontology#burson_program_1990">
        <rdf:type rdf:resource="http://purl.org/ai4se/ontology#ResearchPaper"/>
        <hasLevel rdf:resource="http://purl.org/ai4se/ontology#null"/>
        <hasPurpose rdf:resource="http://purl.org/ai4se/ontology#null"/>
        <hasTarget rdf:resource="http://purl.org/ai4se/ontology#null"/>
        <hasType rdf:resource="http://purl.org/ai4se/ontology#null"/>
        <isAboutResearchTopic rdf:resource="http://purl.org/ai4se/ontology#CSO:Testing_and_debugging"/>
        <rdfs:comment>@inproceedings{burson_program_1990,
 author = {Burson, S and Kotik, GB and Markosian, LZ},
 booktitle = {Proceedings., {Fourteenth} {Annual} {International} {Computer} {Software} and {Applications} {Conference}},
 doi = {10.1109/CMPSAC.1990.139375},
 pages = {314--322},
 publisher = {IEEE},
 title = {A program transformation approach to automating software re-engineering},
 year = {1990}
}
</rdfs:comment>
        <rdfs:label>burson_program_1990</rdfs:label>
        <rdfs:seeAlso rdf:resource="https://doi.org/10.1109/CMPSAC.1990.139375"/>
    </owl:NamedIndividual>
    


    <!-- http://purl.org/ai4se/ontology#ceran_prediction_2023 -->

    <owl:NamedIndividual rdf:about="http://purl.org/ai4se/ontology#ceran_prediction_2023">
        <rdf:type rdf:resource="http://purl.org/ai4se/ontology#ResearchPaper"/>
        <hasLevel rdf:resource="http://purl.org/ai4se/ontology#AI-driven_partial_automation"/>
        <hasPurpose rdf:resource="http://purl.org/ai4se/ontology#Understand"/>
        <hasTarget rdf:resource="http://purl.org/ai4se/ontology#Develop"/>
        <hasTarget rdf:resource="http://purl.org/ai4se/ontology#Operate"/>
        <hasType rdf:resource="http://purl.org/ai4se/ontology#Classical_machine_learning"/>
        <isAboutResearchTopic rdf:resource="http://purl.org/ai4se/ontology#CSO:Software_quality"/>
        <rdfs:comment>@article{ceran_prediction_2023,
 author = {Ceran, A Ayberk and Ar, Yilmaz and Tanrıöver, Ö Özgür and Ceran, Sinem Seyrek},
 doi = {10.1016/j.matpr.2022.11.229},
 journal = {Materials Today: Proceedings},
 note = {Publisher: Elsevier},
 pages = {18--25},
 title = {Prediction of software quality with {Machine} {Learning}-{Based} ensemble methods},
 volume = {81},
 year = {2023}
}
</rdfs:comment>
        <rdfs:label>ceran_prediction_2023</rdfs:label>
        <rdfs:seeAlso rdf:resource="https://doi.org/10.1016/j.matpr.2022.11.229"/>
    </owl:NamedIndividual>
    


    <!-- http://purl.org/ai4se/ontology#chen_design_2024 -->

    <owl:NamedIndividual rdf:about="http://purl.org/ai4se/ontology#chen_design_2024">
        <rdf:type rdf:resource="http://purl.org/ai4se/ontology#ResearchPaper"/>
        <hasLevel rdf:resource="http://purl.org/ai4se/ontology#null"/>
        <hasPurpose rdf:resource="http://purl.org/ai4se/ontology#null"/>
        <hasTarget rdf:resource="http://purl.org/ai4se/ontology#null"/>
        <hasType rdf:resource="http://purl.org/ai4se/ontology#null"/>
        <isAboutResearchTopic rdf:resource="http://purl.org/ai4se/ontology#CSO:Testing_and_debugging"/>
        <rdfs:comment>@inproceedings{chen_design_2024,
 author = {Chen, Jing and Wang, Yufan},
 booktitle = {2024 {International} {Conference} on {Advances} in {Electrical} {Engineering} and {Computer} {Applications} ({AEECA})},
 doi = {10.1109/AEECA62331.2024.00116},
 keywords = {Software engineering, Software algorithms, Heuristic algorithms, Reinforcement learning, Adaptation models, agent, reinforcement learning, Object oriented modeling, Adaptive learning, adaptive mechanism, adaptive systems, Adaptive systems, Dogs, Robots},
 month = {August},
 pages = {655--661},
 publisher = {2024 International Conference on Advances in Electrical Engineering and Computer Applications (AEECA)},
 title = {Design of {Software} {Engineering} {Adaptive} {Learning} {System} {Based} on {Artificial} {Intelligence}},
 url = {https://ieeexplore.ieee.org/document/10898656/},
 year = {2024}
}
</rdfs:comment>
        <rdfs:label>chen_design_2024</rdfs:label>
        <rdfs:seeAlso rdf:resource="https://ieeexplore.ieee.org/document/10898656/"/>
    </owl:NamedIndividual>
    


    <!-- http://purl.org/ai4se/ontology#chen_incorporating_2023 -->

    <owl:NamedIndividual rdf:about="http://purl.org/ai4se/ontology#chen_incorporating_2023">
        <rdf:type rdf:resource="http://purl.org/ai4se/ontology#ResearchPaper"/>
        <hasLevel rdf:resource="http://purl.org/ai4se/ontology#null"/>
        <hasPurpose rdf:resource="http://purl.org/ai4se/ontology#null"/>
        <hasTarget rdf:resource="http://purl.org/ai4se/ontology#null"/>
        <hasType rdf:resource="http://purl.org/ai4se/ontology#null"/>
        <isAboutResearchTopic rdf:resource="http://purl.org/ai4se/ontology#CSO:Testing_and_debugging"/>
        <rdfs:comment>@article{chen_incorporating_2023,
 author = {{Chen}},
 doi = {null},
 journal = {Journal of Information Systems Education},
 title = {Incorporating {AI} and {LLMs} into {Software} {Engineering} {Capstone} {Projects}: {A} {Comprehensive} {Analysis}},
 year = {2023}
}
</rdfs:comment>
        <rdfs:label>chen_incorporating_2023</rdfs:label>
        <rdfs:seeAlso rdf:resource="https://doi.org/null"/>
    </owl:NamedIndividual>
    


    <!-- http://purl.org/ai4se/ontology#dakhel_github_2023 -->

    <owl:NamedIndividual rdf:about="http://purl.org/ai4se/ontology#dakhel_github_2023">
        <rdf:type rdf:resource="http://purl.org/ai4se/ontology#ResearchPaper"/>
        <hasLevel rdf:resource="http://purl.org/ai4se/ontology#null"/>
        <hasPurpose rdf:resource="http://purl.org/ai4se/ontology#null"/>
        <hasTarget rdf:resource="http://purl.org/ai4se/ontology#null"/>
        <hasType rdf:resource="http://purl.org/ai4se/ontology#null"/>
        <isAboutResearchTopic rdf:resource="http://purl.org/ai4se/ontology#CSO:Testing_and_debugging"/>
        <rdfs:comment>@article{dakhel_github_2023,
 author = {Dakhel, Arghavan Moradi and Majdinasab, Vahid and Nikanjam, Amin and Khomh, Foutse and Desmarais, Michel C and Jiang, Zhen Ming Jack},
 doi = {10.1016/j.jss.2023.111734},
 journal = {Journal of Systems and Software},
 note = {Publisher: Elsevier},
 pages = {111734},
 title = {Github copilot ai pair programmer: {Asset} or liability?},
 volume = {203},
 year = {2023}
}
</rdfs:comment>
        <rdfs:label>dakhel_github_2023</rdfs:label>
        <rdfs:seeAlso rdf:resource="https://doi.org/10.1016/j.jss.2023.111734"/>
    </owl:NamedIndividual>
    


    <!-- http://purl.org/ai4se/ontology#dhruv_leveraging_2024 -->

    <owl:NamedIndividual rdf:about="http://purl.org/ai4se/ontology#dhruv_leveraging_2024">
        <rdf:type rdf:resource="http://purl.org/ai4se/ontology#ResearchPaper"/>
        <hasLevel rdf:resource="http://purl.org/ai4se/ontology#null"/>
        <hasPurpose rdf:resource="http://purl.org/ai4se/ontology#null"/>
        <hasTarget rdf:resource="http://purl.org/ai4se/ontology#null"/>
        <hasType rdf:resource="http://purl.org/ai4se/ontology#null"/>
        <isAboutResearchTopic rdf:resource="http://purl.org/ai4se/ontology#CSO:Testing_and_debugging"/>
        <rdfs:comment>@misc{dhruv_leveraging_2024,
 author = {Dhruv, Akash and Dubey, Anshu},
 copyright = {Creative Commons Attribution 4.0 International},
 doi = {10.48550/ARXIV.2410.24119},
 keywords = {FOS: Computer and information sciences, Software Engineering (cs.SE), Artificial Intelligence (cs.AI)},
 note = {Version Number: 2},
 publisher = {arXiv},
 title = {Leveraging {Large} {Language} {Models} for {Code} {Translation} and {Software} {Development} in {Scientific} {Computing}},
 url = {https://arxiv.org/abs/2410.24119},
 urldate = {2025-06-03},
 year = {2024}
}
</rdfs:comment>
        <rdfs:label>dhruv_leveraging_2024</rdfs:label>
        <rdfs:seeAlso rdf:resource="https://arxiv.org/abs/2410.24119"/>
    </owl:NamedIndividual>
    


    <!-- http://purl.org/ai4se/ontology#drain_generating_2021 -->

    <owl:NamedIndividual rdf:about="http://purl.org/ai4se/ontology#drain_generating_2021">
        <rdf:type rdf:resource="http://purl.org/ai4se/ontology#ResearchPaper"/>
        <hasLevel rdf:resource="http://purl.org/ai4se/ontology#AI-driven_partial_automation"/>
        <hasPurpose rdf:resource="http://purl.org/ai4se/ontology#Improve"/>
        <hasTarget rdf:resource="http://purl.org/ai4se/ontology#Coding"/>
        <hasTarget rdf:resource="http://purl.org/ai4se/ontology#Maintenance"/>
        <hasType rdf:resource="http://purl.org/ai4se/ontology#Deep_learning"/>
        <isAboutResearchTopic rdf:resource="http://purl.org/ai4se/ontology#CSO:Static_analysis"/>
        <rdfs:comment>@inproceedings{drain_generating_2021,
 author = {Drain, Dawn and Wu, Chen and Svyatkovskiy, Alexey and Sundaresan, Neel},
 booktitle = {Proceedings of the 5th {ACM} {SIGPLAN} {International} {Symposium} on {Machine} {Programming}},
 doi = {10.1145/3460945.3464951},
 pages = {1--8},
 title = {Generating bug-fixes using pretrained transformers},
 year = {2021}
}
</rdfs:comment>
        <rdfs:label>drain_generating_2021</rdfs:label>
        <rdfs:seeAlso rdf:resource="https://doi.org/10.1145/3460945.3464951"/>
    </owl:NamedIndividual>
    


    <!-- http://purl.org/ai4se/ontology#durrani_decade_2024 -->

    <owl:NamedIndividual rdf:about="http://purl.org/ai4se/ontology#durrani_decade_2024">
        <rdf:type rdf:resource="http://purl.org/ai4se/ontology#ResearchPaper"/>
        <hasLevel rdf:resource="http://purl.org/ai4se/ontology#null"/>
        <hasPurpose rdf:resource="http://purl.org/ai4se/ontology#null"/>
        <hasTarget rdf:resource="http://purl.org/ai4se/ontology#null"/>
        <hasType rdf:resource="http://purl.org/ai4se/ontology#null"/>
        <isAboutResearchTopic rdf:resource="http://purl.org/ai4se/ontology#CSO:Testing_and_debugging"/>
        <rdfs:comment>@article{durrani_decade_2024,
 author = {Durrani, Usman Khan and Akpinar, Mustafa and Fatih Adak, Muhammed and Talha Kabakus, Abdullah and Maruf Öztürk, Muhammed and Saleh, Mohammed},
 copyright = {https://creativecommons.org/licenses/by-nc-nd/4.0/},
 doi = {10.1109/ACCESS.2024.3488904},
  issn = {2169-3536},
 journal = {IEEE Access},
 pages = {171185--171204},
 shorttitle = {A {Decade} of {Progress}},
 title = {A {Decade} of {Progress}: {A} {Systematic} {Literature} {Review} on the {Integration} of {AI} in {Software} {Engineering} {Phases} and {Activities} (2013-2023)},
 url = {https://ieeexplore.ieee.org/document/10740293/},
 urldate = {2025-06-02},
 volume = {12},
 year = {2024}
}
</rdfs:comment>
        <rdfs:label>durrani_decade_2024</rdfs:label>
        <rdfs:seeAlso rdf:resource="https://ieeexplore.ieee.org/document/10740293/"/>
    </owl:NamedIndividual>
    


    <!-- http://purl.org/ai4se/ontology#ebert_generative_2023 -->

    <owl:NamedIndividual rdf:about="http://purl.org/ai4se/ontology#ebert_generative_2023">
        <rdf:type rdf:resource="http://purl.org/ai4se/ontology#ResearchPaper"/>
        <hasLevel rdf:resource="http://purl.org/ai4se/ontology#null"/>
        <hasPurpose rdf:resource="http://purl.org/ai4se/ontology#null"/>
        <hasTarget rdf:resource="http://purl.org/ai4se/ontology#null"/>
        <hasType rdf:resource="http://purl.org/ai4se/ontology#null"/>
        <isAboutResearchTopic rdf:resource="http://purl.org/ai4se/ontology#CSO:Testing_and_debugging"/>
        <rdfs:comment>@article{ebert_generative_2023,
 author = {Ebert, Christof and Λουρίδας, Πάνος},
 doi = {10.1109/ms.2023.3265877},
 journal = {IEEE Software},
 pmcid = {null},
 pmid = {null},
 title = {Generative {AI} for {Software} {Practitioners}},
 year = {2023}
}
</rdfs:comment>
        <rdfs:label>ebert_generative_2023</rdfs:label>
        <rdfs:seeAlso rdf:resource="https://doi.org/10.1109/ms.2023.3265877"/>
    </owl:NamedIndividual>
    


    <!-- http://purl.org/ai4se/ontology#eisenreich_requirements_2024 -->

    <owl:NamedIndividual rdf:about="http://purl.org/ai4se/ontology#eisenreich_requirements_2024">
        <rdf:type rdf:resource="http://purl.org/ai4se/ontology#ResearchPaper"/>
        <hasLevel rdf:resource="http://purl.org/ai4se/ontology#null"/>
        <hasPurpose rdf:resource="http://purl.org/ai4se/ontology#null"/>
        <hasTarget rdf:resource="http://purl.org/ai4se/ontology#null"/>
        <hasType rdf:resource="http://purl.org/ai4se/ontology#null"/>
        <isAboutResearchTopic rdf:resource="http://purl.org/ai4se/ontology#CSO:Testing_and_debugging"/>
        <rdfs:comment>@inproceedings{eisenreich_requirements_2024,
 author = {Eisenreich, Tobias and Speth, Sandro and Wagner, Stefan},
 booktitle = {Proceedings of the 1st {International} {Workshop} on {Designing} {Software}},
 doi = {10.1145/3643660.3643942},
 pages = {52--55},
 title = {From requirements to architecture: {An} ai-based journey to semi-automatically generate software architectures},
 year = {2024}
}
</rdfs:comment>
        <rdfs:label>eisenreich_requirements_2024</rdfs:label>
        <rdfs:seeAlso rdf:resource="https://doi.org/10.1145/3643660.3643942"/>
    </owl:NamedIndividual>
    


    <!-- http://purl.org/ai4se/ontology#fan_automated_2023 -->

    <owl:NamedIndividual rdf:about="http://purl.org/ai4se/ontology#fan_automated_2023">
        <rdf:type rdf:resource="http://purl.org/ai4se/ontology#ResearchPaper"/>
        <hasLevel rdf:resource="http://purl.org/ai4se/ontology#null"/>
        <hasPurpose rdf:resource="http://purl.org/ai4se/ontology#null"/>
        <hasTarget rdf:resource="http://purl.org/ai4se/ontology#null"/>
        <hasType rdf:resource="http://purl.org/ai4se/ontology#null"/>
        <isAboutResearchTopic rdf:resource="http://purl.org/ai4se/ontology#CSO:Testing_and_debugging"/>
        <rdfs:comment>@inproceedings{fan_automated_2023,
 address = {Melbourne, Australia},
 author = {Fan, Zhiyu and Gao, Xiang and Mirchev, Martin and Roychoudhury, Abhik and Tan, Shin Hwei},
 booktitle = {2023 {IEEE}/{ACM} 45th {International} {Conference} on {Software} {Engineering} ({ICSE})},
 copyright = {https://doi.org/10.15223/policy-029},
 doi = {10.1109/ICSE48619.2023.00128},
  isbn = {978-1-6654-5701-9},
 month = {May},
 pages = {1469--1481},
 publisher = {IEEE},
 title = {Automated {Repair} of {Programs} from {Large} {Language} {Models}},
 url = {https://ieeexplore.ieee.org/document/10172854/},
 urldate = {2025-06-03},
 year = {2023}
}
</rdfs:comment>
        <rdfs:label>fan_automated_2023</rdfs:label>
        <rdfs:seeAlso rdf:resource="https://ieeexplore.ieee.org/document/10172854/"/>
    </owl:NamedIndividual>
    


    <!-- http://purl.org/ai4se/ontology#ford_artificial_1987 -->

    <owl:NamedIndividual rdf:about="http://purl.org/ai4se/ontology#ford_artificial_1987">
        <rdf:type rdf:resource="http://purl.org/ai4se/ontology#ResearchPaper"/>
        <hasLevel rdf:resource="http://purl.org/ai4se/ontology#null"/>
        <hasPurpose rdf:resource="http://purl.org/ai4se/ontology#null"/>
        <hasTarget rdf:resource="http://purl.org/ai4se/ontology#null"/>
        <hasType rdf:resource="http://purl.org/ai4se/ontology#null"/>
        <isAboutResearchTopic rdf:resource="http://purl.org/ai4se/ontology#CSO:Testing_and_debugging"/>
        <rdfs:comment>@article{ford_artificial_1987,
 author = {Ford, L.},
 copyright = {http://www.springer.com/tdm},
 doi = {10.1007/BF00142926},
 issn = {0269-2821, 1573-7462},
 journal = {Artificial Intelligence Review},
 language = {en},
 number = {4},
 pages = {255--273},
 shorttitle = {Artificial intelligence and software engineering},
 title = {Artificial intelligence and software engineering: a tutorial introduction to their relationship},
 url = {http://link.springer.com/10.1007/BF00142926},
 urldate = {2025-06-03},
 volume = {1},
 year = {1987}
}
</rdfs:comment>
        <rdfs:label>ford_artificial_1987</rdfs:label>
        <rdfs:seeAlso rdf:resource="http://link.springer.com/10.1007/BF00142926"/>
    </owl:NamedIndividual>
    


    <!-- http://purl.org/ai4se/ontology#ghai_artificial_2024 -->

    <owl:NamedIndividual rdf:about="http://purl.org/ai4se/ontology#ghai_artificial_2024">
        <rdf:type rdf:resource="http://purl.org/ai4se/ontology#ResearchPaper"/>
        <hasLevel rdf:resource="http://purl.org/ai4se/ontology#null"/>
        <hasPurpose rdf:resource="http://purl.org/ai4se/ontology#null"/>
        <hasTarget rdf:resource="http://purl.org/ai4se/ontology#null"/>
        <hasType rdf:resource="http://purl.org/ai4se/ontology#null"/>
        <isAboutResearchTopic rdf:resource="http://purl.org/ai4se/ontology#CSO:Testing_and_debugging"/>
        <rdfs:comment>@inproceedings{ghai_artificial_2024,
 author = {Ghai, Anupriya Sharma and Rawat, Vandna and Gupta, Vishan Kumar and Ghai, Kapil},
 booktitle = {2024 {International} {Conference} on {Electrical} {Electronics} and {Computing} {Technologies} ({ICEECT})},
 doi = {10.1109/ICEECT61758.2024.10738945},
 keywords = {Software, Codes, Software engineering, Manuals, Encoding, Software algorithms, Transforms, Ethics, Artificial intelligence, ai code generation, Error analysis, manual code, system and software engineering},
 month = {August},
 pages = {01. Mai},
 publisher = {2024 International Conference on Electrical Electronics and Computing Technologies (ICEECT)},
 title = {Artificial {Intelligence} in {System} and {Software} {Engineering} for {Auto} {Code} {Generation}},
 url = {https://ieeexplore.ieee.org/document/10738945/},
 volume = {1},
 year = {2024}
}
</rdfs:comment>
        <rdfs:label>ghai_artificial_2024</rdfs:label>
        <rdfs:seeAlso rdf:resource="https://ieeexplore.ieee.org/document/10738945/"/>
    </owl:NamedIndividual>
    


    <!-- http://purl.org/ai4se/ontology#gokce_coverage-based_2006 -->

    <owl:NamedIndividual rdf:about="http://purl.org/ai4se/ontology#gokce_coverage-based_2006">
        <rdf:type rdf:resource="http://purl.org/ai4se/ontology#ResearchPaper"/>
        <hasLevel rdf:resource="http://purl.org/ai4se/ontology#null"/>
        <hasPurpose rdf:resource="http://purl.org/ai4se/ontology#null"/>
        <hasTarget rdf:resource="http://purl.org/ai4se/ontology#null"/>
        <hasType rdf:resource="http://purl.org/ai4se/ontology#null"/>
        <isAboutResearchTopic rdf:resource="http://purl.org/ai4se/ontology#CSO:Testing_and_debugging"/>
        <rdfs:comment>@inproceedings{gokce_coverage-based_2006,
 author = {Gökçe, Nida and Eminov, Mubariz and Belli, Fevzi},
 booktitle = {Computer and {Information} {Sciences}–{ISCIS} 2006: 21th {International} {Symposium}, {Istanbul}, {Turkey}, {November} 1-3, 2006. {Proceedings} 21},
 doi = {10.1007/11902140_110},
 pages = {1060--1071},
 publisher = {Springer},
 title = {Coverage-based, prioritized testing using neural network clustering},
 year = {2006}
}
</rdfs:comment>
        <rdfs:label>gokce_coverage-based_2006</rdfs:label>
        <rdfs:seeAlso rdf:resource="https://doi.org/10.1007/11902140_110"/>
    </owl:NamedIndividual>
    


    <!-- http://purl.org/ai4se/ontology#gui_cross-language_2022 -->

    <owl:NamedIndividual rdf:about="http://purl.org/ai4se/ontology#gui_cross-language_2022">
        <rdf:type rdf:resource="http://purl.org/ai4se/ontology#ResearchPaper"/>
        <hasLevel rdf:resource="http://purl.org/ai4se/ontology#null"/>
        <hasPurpose rdf:resource="http://purl.org/ai4se/ontology#null"/>
        <hasTarget rdf:resource="http://purl.org/ai4se/ontology#null"/>
        <hasType rdf:resource="http://purl.org/ai4se/ontology#null"/>
        <isAboutResearchTopic rdf:resource="http://purl.org/ai4se/ontology#CSO:Testing_and_debugging"/>
        <rdfs:comment>@inproceedings{gui_cross-language_2022,
 address = {Honolulu, HI, USA},
 author = {Gui, Yi and Wan, Yao and Zhang, Hongyu and Huang, Huifang and Sui, Yulei and Xu, Guandong and Shao, Zhiyuan and Jin, Hai},
 booktitle = {2022 {IEEE} {International} {Conference} on {Software} {Analysis}, {Evolution} and {Reengineering} ({SANER})},
 copyright = {https://doi.org/10.15223/policy-029},
 doi = {10.1109/SANER53432.2022.00077},
  isbn = {978-1-6654-3786-8},
 month = {March},
 pages = {601--612},
 publisher = {IEEE},
 title = {Cross-{Language} {Binary}-{Source} {Code} {Matching} with {Intermediate} {Representations}},
 url = {https://ieeexplore.ieee.org/document/9825768/},
 urldate = {2025-06-03},
 year = {2022}
}
</rdfs:comment>
        <rdfs:label>gui_cross-language_2022</rdfs:label>
        <rdfs:seeAlso rdf:resource="https://ieeexplore.ieee.org/document/9825768/"/>
    </owl:NamedIndividual>
    


    <!-- http://purl.org/ai4se/ontology#guo_deepseek-coder_2024 -->

    <owl:NamedIndividual rdf:about="http://purl.org/ai4se/ontology#guo_deepseek-coder_2024">
        <rdf:type rdf:resource="http://purl.org/ai4se/ontology#ResearchPaper"/>
        <hasLevel rdf:resource="http://purl.org/ai4se/ontology#null"/>
        <hasPurpose rdf:resource="http://purl.org/ai4se/ontology#null"/>
        <hasTarget rdf:resource="http://purl.org/ai4se/ontology#null"/>
        <hasType rdf:resource="http://purl.org/ai4se/ontology#null"/>
        <isAboutResearchTopic rdf:resource="http://purl.org/ai4se/ontology#CSO:Testing_and_debugging"/>
        <rdfs:comment>@misc{guo_deepseek-coder_2024,
 author = {Guo, Daya and Zhu, Qihao and Yang, Dejian and Xie, Zhenda and Dong, Kai and Zhang, Wentao and Chen, Guanting and Bi, Xiao and Wu, Y. and Li, Y. K. and Luo, Fuli and Xiong, Yingfei and Liang, Wenfeng},
 copyright = {arXiv.org perpetual, non-exclusive license},
 doi = {10.48550/ARXIV.2401.14196},
 keywords = {FOS: Computer and information sciences, Machine Learning (cs.LG), Software Engineering (cs.SE), Computation and Language (cs.CL)},
 note = {Version Number: 2},
 publisher = {arXiv},
 shorttitle = {{DeepSeek}-{Coder}},
 title = {{DeepSeek}-{Coder}: {When} the {Large} {Language} {Model} {Meets} {Programming} -- {The} {Rise} of {Code} {Intelligence}},
 url = {https://arxiv.org/abs/2401.14196},
 urldate = {2025-06-02},
 year = {2024}
}
</rdfs:comment>
        <rdfs:label>guo_deepseek-coder_2024</rdfs:label>
        <rdfs:seeAlso rdf:resource="https://arxiv.org/abs/2401.14196"/>
    </owl:NamedIndividual>
    


    <!-- http://purl.org/ai4se/ontology#guo_graphcodebert_2020 -->

    <owl:NamedIndividual rdf:about="http://purl.org/ai4se/ontology#guo_graphcodebert_2020">
        <rdf:type rdf:resource="http://purl.org/ai4se/ontology#ResearchPaper"/>
        <hasLevel rdf:resource="http://purl.org/ai4se/ontology#AI-assisted_options"/>
        <hasPurpose rdf:resource="http://purl.org/ai4se/ontology#Understand"/>
        <hasTarget rdf:resource="http://purl.org/ai4se/ontology#Coding"/>
        <hasTarget rdf:resource="http://purl.org/ai4se/ontology#Maintenance"/>
        <hasType rdf:resource="http://purl.org/ai4se/ontology#Deep_learning"/>
        <isAboutResearchTopic rdf:resource="http://purl.org/ai4se/ontology#CSO:Deep_learning"/>
        <rdfs:comment>@article{guo_graphcodebert_2020,
 author = {Guo, Daya and Ren, Shuo and Lu, Shuai and Feng, Zhangyin and Tang, Duyu and Liu, Shujie and Zhou, Long and Duan, Nan and Svyatkovskiy, Alexey and Fu, Shengyu and {others}},
 doi = {10.48550/arXiv.2009.08366},
 journal = {arXiv preprint arXiv:2009.08366},
 title = {Graphcodebert: {Pre}-training code representations with data flow},
 year = {2020}
}
</rdfs:comment>
        <rdfs:label>guo_graphcodebert_2020</rdfs:label>
        <rdfs:seeAlso rdf:resource="https://doi.org/10.48550/arXiv.2009.08366"/>
    </owl:NamedIndividual>
    


    <!-- http://purl.org/ai4se/ontology#gupta_intelligent_2018 -->

    <owl:NamedIndividual rdf:about="http://purl.org/ai4se/ontology#gupta_intelligent_2018">
        <rdf:type rdf:resource="http://purl.org/ai4se/ontology#ResearchPaper"/>
        <hasLevel rdf:resource="http://purl.org/ai4se/ontology#AI-assisted_selection"/>
        <hasPurpose rdf:resource="http://purl.org/ai4se/ontology#Improve"/>
        <hasTarget rdf:resource="http://purl.org/ai4se/ontology#Coding"/>
        <hasTarget rdf:resource="http://purl.org/ai4se/ontology#Deployment"/>
        <hasType rdf:resource="http://purl.org/ai4se/ontology#Deep_learning"/>
        <isAboutResearchTopic rdf:resource="http://purl.org/ai4se/ontology#CSO:Static_analysis"/>
        <rdfs:comment>@inproceedings{gupta_intelligent_2018,
 author = {Gupta, Anshul and Sundaresan, Neel},
 booktitle = {Proceedings of the 24th {ACM} {SIGKDD} {International} {Conference} on {Knowledge} {Discovery} and {Data} {Mining} ({KDD}’18) {Deep} {Learning} {Day}},
 title = {Intelligent code reviews using deep learning},
 year = {2018},
 url = {https://www.kdd.org/kdd2018/files/deep-learning-day/DLDay18_paper_40.pdf}
}
</rdfs:comment>
        <rdfs:label>gupta_intelligent_2018</rdfs:label>
        <rdfs:seeAlso rdf:resource="https://www.kdd.org/kdd2018/files/deep-learning-day/DLDay18_paper_40.pdf"/>
    </owl:NamedIndividual>
    


    <!-- http://purl.org/ai4se/ontology#harman_role_2012 -->

    <owl:NamedIndividual rdf:about="http://purl.org/ai4se/ontology#harman_role_2012">
        <rdf:type rdf:resource="http://purl.org/ai4se/ontology#ResearchPaper"/>
        <hasLevel rdf:resource="http://purl.org/ai4se/ontology#null"/>
        <hasPurpose rdf:resource="http://purl.org/ai4se/ontology#null"/>
        <hasTarget rdf:resource="http://purl.org/ai4se/ontology#null"/>
        <hasType rdf:resource="http://purl.org/ai4se/ontology#null"/>
        <isAboutResearchTopic rdf:resource="http://purl.org/ai4se/ontology#CSO:Testing_and_debugging"/>
        <rdfs:comment>@inproceedings{harman_role_2012,
 author = {Harman, Mark},
 booktitle = {Proceedings of the {First} {International} {Workshop} on {Realizing} {AI} {Synergies} in {Software} {Engineering}, {RAISE} 2012, {Zurich}, {Switzerland}, {June} 5, 2012},
 doi = {10.1109/RAISE.2012.6227961},
 editor = {Harrison, Rachel},
 pages = {1--6},
 publisher = {IEEE},
 title = {The role of artificial intelligence in software engineering},
 url = {https://doi.org/10.1109/RAISE.2012.6227961},
 year = {2012}
}
</rdfs:comment>
        <rdfs:label>harman_role_2012</rdfs:label>
        <rdfs:seeAlso rdf:resource="https://doi.org/10.1109/RAISE.2012.6227961"/>
    </owl:NamedIndividual>
    


    <!-- http://purl.org/ai4se/ontology#hu_practitioners_2022 -->

    <owl:NamedIndividual rdf:about="http://purl.org/ai4se/ontology#hu_practitioners_2022">
        <rdf:type rdf:resource="http://purl.org/ai4se/ontology#ResearchPaper"/>
        <hasLevel rdf:resource="http://purl.org/ai4se/ontology#null"/>
        <hasPurpose rdf:resource="http://purl.org/ai4se/ontology#null"/>
        <hasTarget rdf:resource="http://purl.org/ai4se/ontology#null"/>
        <hasType rdf:resource="http://purl.org/ai4se/ontology#null"/>
        <isAboutResearchTopic rdf:resource="http://purl.org/ai4se/ontology#CSO:Testing_and_debugging"/>
        <rdfs:comment>@inproceedings{hu_practitioners_2022,
 address = {Pittsburgh Pennsylvania},
 author = {Hu, Xing and Xia, Xin and Lo, David and Wan, Zhiyuan and Chen, Qiuyuan and Zimmermann, Thomas},
 booktitle = {Proceedings of the 44th {International} {Conference} on {Software} {Engineering}},
 doi = {10.1145/3510003.3510152},
 isbn = {978-1-4503-9221-1},
 language = {en},
 month = {May},
 pages = {1693--1705},
 publisher = {ACM},
 title = {Practitioners&apos; expectations on automated code comment generation},
 url = {https://dl.acm.org/doi/10.1145/3510003.3510152},
 urldate = {2025-06-03},
 year = {2022}
}
</rdfs:comment>
        <rdfs:label>hu_practitioners_2022</rdfs:label>
        <rdfs:seeAlso rdf:resource="https://dl.acm.org/doi/10.1145/3510003.3510152"/>
    </owl:NamedIndividual>
    


    <!-- http://purl.org/ai4se/ontology#iqbal_measuring_2021 -->

    <owl:NamedIndividual rdf:about="http://purl.org/ai4se/ontology#iqbal_measuring_2021">
        <rdf:type rdf:resource="http://purl.org/ai4se/ontology#ResearchPaper"/>
        <hasLevel rdf:resource="http://purl.org/ai4se/ontology#null"/>
        <hasPurpose rdf:resource="http://purl.org/ai4se/ontology#null"/>
        <hasTarget rdf:resource="http://purl.org/ai4se/ontology#null"/>
        <hasType rdf:resource="http://purl.org/ai4se/ontology#null"/>
        <isAboutResearchTopic rdf:resource="http://purl.org/ai4se/ontology#CSO:Testing_and_debugging"/>
        <rdfs:comment>@article{iqbal_measuring_2021,
 author = {Iqbal, Nayyar and Sang, Jun and Chen, Jing and Xia, Xiaofeng},
 copyright = {https://creativecommons.org/licenses/by/4.0/},
 doi = {10.3390/e23020136},
  issn = {1099-4300},
 journal = {Entropy},
 language = {en},
 month = {January},
 number = {2},
 pages = {136},
 title = {Measuring {Software} {Maintainability} with {Naïve} {Bayes} {Classifier}},
 url = {https://www.mdpi.com/1099-4300/23/2/136},
 urldate = {2025-06-03},
 volume = {23},
 year = {2021}
}
</rdfs:comment>
        <rdfs:label>iqbal_measuring_2021</rdfs:label>
        <rdfs:seeAlso rdf:resource="https://www.mdpi.com/1099-4300/23/2/136"/>
    </owl:NamedIndividual>
    


    <!-- http://purl.org/ai4se/ontology#joshi_repair_2023 -->

    <owl:NamedIndividual rdf:about="http://purl.org/ai4se/ontology#joshi_repair_2023">
        <rdf:type rdf:resource="http://purl.org/ai4se/ontology#ResearchPaper"/>
        <hasLevel rdf:resource="http://purl.org/ai4se/ontology#null"/>
        <hasPurpose rdf:resource="http://purl.org/ai4se/ontology#null"/>
        <hasTarget rdf:resource="http://purl.org/ai4se/ontology#null"/>
        <hasType rdf:resource="http://purl.org/ai4se/ontology#null"/>
        <isAboutResearchTopic rdf:resource="http://purl.org/ai4se/ontology#CSO:Testing_and_debugging"/>
        <rdfs:comment>@article{joshi_repair_2023,
 author = {Joshi, Harshit and Cambronero Sanchez, José and Gulwani, Sumit and Le, Vu and Verbruggen, Gust and Radiček, Ivan},
 doi = {10.1609/aaai.v37i4.25642},
  issn = {2374-3468, 2159-5399},
 journal = {Proceedings of the AAAI Conference on Artificial Intelligence},
 month = {June},
 number = {4},
 pages = {5131--5140},
 shorttitle = {Repair {Is} {Nearly} {Generation}},
 title = {Repair {Is} {Nearly} {Generation}: {Multilingual} {Program} {Repair} with {LLMs}},
 url = {https://ojs.aaai.org/index.php/AAAI/article/view/25642},
 urldate = {2025-06-03},
 volume = {37},
 year = {2023}
}
</rdfs:comment>
        <rdfs:label>joshi_repair_2023</rdfs:label>
        <rdfs:seeAlso rdf:resource="https://ojs.aaai.org/index.php/AAAI/article/view/25642"/>
    </owl:NamedIndividual>
    


    <!-- http://purl.org/ai4se/ontology#kalech_artificial_2021 -->

    <owl:NamedIndividual rdf:about="http://purl.org/ai4se/ontology#kalech_artificial_2021">
        <rdf:type rdf:resource="http://purl.org/ai4se/ontology#ResearchPaper"/>
        <hasLevel rdf:resource="http://purl.org/ai4se/ontology#null"/>
        <hasPurpose rdf:resource="http://purl.org/ai4se/ontology#null"/>
        <hasTarget rdf:resource="http://purl.org/ai4se/ontology#null"/>
        <hasType rdf:resource="http://purl.org/ai4se/ontology#null"/>
        <isAboutResearchTopic rdf:resource="http://purl.org/ai4se/ontology#CSO:Testing_and_debugging"/>
        <rdfs:comment>@book{kalech_artificial_2021,
 author = {Kalech, Meir and Abreu, Rui and Last, Mark},
 doi = {10.1142/12360},
 isbn = {978-981-12-3991-5},
 publisher = {WorldScientific},
 title = {Artificial {Intelligence} {Methods} for {Software} {Engineering}},
 url = {https://doi.org/10.1142/12360},
 year = {2021}
}
</rdfs:comment>
        <rdfs:label>kalech_artificial_2021</rdfs:label>
        <rdfs:seeAlso rdf:resource="https://doi.org/10.1142/12360"/>
    </owl:NamedIndividual>
    


    <!-- http://purl.org/ai4se/ontology#korner_transferring_2014 -->

    <owl:NamedIndividual rdf:about="http://purl.org/ai4se/ontology#korner_transferring_2014">
        <rdf:type rdf:resource="http://purl.org/ai4se/ontology#ResearchPaper"/>
        <hasLevel rdf:resource="http://purl.org/ai4se/ontology#AI-assisted_selection"/>
        <hasPurpose rdf:resource="http://purl.org/ai4se/ontology#Improve"/>
        <hasType rdf:resource="http://purl.org/ai4se/ontology#Symbolic"/>
        <isAboutResearchTopic rdf:resource="http://purl.org/ai4se/ontology#CSO:Requirements_engineering"/>
        <rdfs:comment>@inproceedings{korner_transferring_2014,
 author = {Körner, Sven J and Landhäußer, Mathias and Tichy, Walter F},
 booktitle = {2014 {IEEE} 1st {International} {Workshop} on {Artificial} {Intelligence} for {Requirements} {Engineering} ({AIRE})},
 doi = {10.1109/AIRE.2014.6894851},
 pages = {13--18},
 publisher = {IEEE},
 title = {Transferring research into the real world: {How} to improve {RE} with {AI} in the automotive industry},
 year = {2014}
}
</rdfs:comment>
        <rdfs:label>korner_transferring_2014</rdfs:label>
        <rdfs:seeAlso rdf:resource="https://doi.org/10.1109/AIRE.2014.6894851"/>
    </owl:NamedIndividual>
    


    <!-- http://purl.org/ai4se/ontology#kumari_intelligent_2025 -->

    <owl:NamedIndividual rdf:about="http://purl.org/ai4se/ontology#kumari_intelligent_2025">
        <rdf:type rdf:resource="http://purl.org/ai4se/ontology#ResearchPaper"/>
        <hasLevel rdf:resource="http://purl.org/ai4se/ontology#null"/>
        <hasPurpose rdf:resource="http://purl.org/ai4se/ontology#null"/>
        <hasTarget rdf:resource="http://purl.org/ai4se/ontology#null"/>
        <hasType rdf:resource="http://purl.org/ai4se/ontology#null"/>
        <isAboutResearchTopic rdf:resource="http://purl.org/ai4se/ontology#CSO:Testing_and_debugging"/>
        <rdfs:comment>@article{kumari_intelligent_2025,
 author = {Kumari, Pragati},
 journal = {International Journal on Science and Technology},
 title = {Intelligent {Test} {Automation}: {A} {Multi}-{Agent} {LLM} {Framework} for {Dynamic} {Test} {Case} {Generation} and {Validation}},
 url = {https://api.semanticscholar.org/CorpusID:276753846},
 year = {2025}
}
</rdfs:comment>
        <rdfs:label>kumari_intelligent_2025</rdfs:label>
        <rdfs:seeAlso rdf:resource="https://api.semanticscholar.org/CorpusID:276753846"/>
    </owl:NamedIndividual>
    


    <!-- http://purl.org/ai4se/ontology#lenz_linking_2013 -->

    <owl:NamedIndividual rdf:about="http://purl.org/ai4se/ontology#lenz_linking_2013">
        <rdf:type rdf:resource="http://purl.org/ai4se/ontology#ResearchPaper"/>
        <hasLevel rdf:resource="http://purl.org/ai4se/ontology#AI-assisted_selection"/>
        <hasPurpose rdf:resource="http://purl.org/ai4se/ontology#Generate"/>
        <hasTarget rdf:resource="http://purl.org/ai4se/ontology#Testing"/>
        <hasType rdf:resource="http://purl.org/ai4se/ontology#Classical_machine_learning"/>
        <isAboutResearchTopic rdf:resource="http://purl.org/ai4se/ontology#CSO:Testing_and_debugging"/>
        <rdfs:comment>@article{lenz_linking_2013,
 author = {Lenz, Alexandre Rafael and Pozo, Aurora and Vergilio, Silvia Regina},
 doi = {10.1016/j.engappai.2013.01.008},
 journal = {Engineering Applications of Artificial Intelligence},
 note = {Publisher: Elsevier},
 number = {5-6},
 pages = {1631--1640},
 title = {Linking software testing results with a machine learning approach},
 volume = {26},
 year = {2013}
}
</rdfs:comment>
        <rdfs:label>lenz_linking_2013</rdfs:label>
        <rdfs:seeAlso rdf:resource="https://doi.org/10.1016/j.engappai.2013.01.008"/>
    </owl:NamedIndividual>
    


    <!-- http://purl.org/ai4se/ontology#li_starcoder_2023 -->

    <owl:NamedIndividual rdf:about="http://purl.org/ai4se/ontology#li_starcoder_2023">
        <rdf:type rdf:resource="http://purl.org/ai4se/ontology#ResearchPaper"/>
        <hasLevel rdf:resource="http://purl.org/ai4se/ontology#null"/>
        <hasPurpose rdf:resource="http://purl.org/ai4se/ontology#null"/>
        <hasTarget rdf:resource="http://purl.org/ai4se/ontology#null"/>
        <hasType rdf:resource="http://purl.org/ai4se/ontology#null"/>
        <isAboutResearchTopic rdf:resource="http://purl.org/ai4se/ontology#CSO:Testing_and_debugging"/>
        <rdfs:comment>@article{li_starcoder_2023,
 author = {Li, Raymond and Allal, Loubna Ben and Zi, Yangtian and Muennighoff, Niklas and Kocetkov, Denis and Mou, Chenghao and Marone, M. and Akiki, Christopher and Li, Jia and Chim, Jenny and Liu, Qian and Zheltonozhskii, Evgenii and Zhuo, Terry Yue and Wang, Thomas J. and Dehaene, Olivier and Davaadorj, Mishig and Lamy-Poirier, Joël and Monteiro, João L. and Shliazhko, Oleh and Gontier, Nicolas and Meade, Nicholas and Zebaze, Armel and Yee, Ming-Ho and Umapathi, Logesh Kumar and Zhu, Jun and Lipkin, Benjamin and Oblokulov, Muhtasham and Wang, Zhiruo and Murthy, Ravindra and Stillerman, Jason and Patel, Siva Sankalp and Abulkhanov, Dmitry and Zocca, Marco and Dey, Manan and Zhang, Zhihan and Fahmy, Nour and Bhattacharyya, Urvashi and Yu, Wenhao and Singh, Surjit and Luccioni, Sasha and Villegas, Paulo and Kunakov, Maxim and Zhdanov, Fedor and Romero, Manuel and Lee, Tong and Timor, Nadav and Ding, Jennifer and Schlesinger, Cole and Schoelkopf, Hailey and Ebert, Jürgen and Dao, Tri and Mishra, Mayank and Gu, Alex and Robinson, Jennifer G. and Anderson, Carolyn J. and Dolan-Gavitt, Brendan and Contractor, Danish and Reddy, Siva and Fried, Daniel and Bahdanau, Dzmitry and Jernite, Yacine and Ferrandis, Carlos Muñoz and Hughes, Sean and Wolf, Thomas and Guha, Arjun and Werra, Leandro von and Vries, Harm de},
 doi = {10.48550/arxiv.2305.06161},
 journal = {arXiv preprint arXiv:2305.06161},
 pmcid = {null},
 pmid = {null},
 title = {{StarCoder}: may the source be with you!},
 year = {2023}
}
</rdfs:comment>
        <rdfs:label>li_starcoder_2023</rdfs:label>
        <rdfs:seeAlso rdf:resource="https://doi.org/10.48550/arxiv.2305.06161"/>
    </owl:NamedIndividual>
    


    <!-- http://purl.org/ai4se/ontology#li_vulanalyzer_2023 -->

    <owl:NamedIndividual rdf:about="http://purl.org/ai4se/ontology#li_vulanalyzer_2023">
        <rdf:type rdf:resource="http://purl.org/ai4se/ontology#ResearchPaper"/>
        <hasLevel rdf:resource="http://purl.org/ai4se/ontology#null"/>
        <hasPurpose rdf:resource="http://purl.org/ai4se/ontology#null"/>
        <hasTarget rdf:resource="http://purl.org/ai4se/ontology#null"/>
        <hasType rdf:resource="http://purl.org/ai4se/ontology#null"/>
        <isAboutResearchTopic rdf:resource="http://purl.org/ai4se/ontology#CSO:Testing_and_debugging"/>
        <rdfs:comment>@article{li_vulanalyzer_2023,
 author = {Li, Litao and Ding, Steven H. H. and Tian, Yuan and Fung, Benjamin C. M. and Charland, Philippe and Ou, Weihan and Song, Leo and Chen, Congwei},
 doi = {10.1145/3585386},
 issn = {2471-2566, 2471-2574},
 journal = {ACM Transactions on Privacy and Security},
 language = {en},
 month = {August},
 number = {3},
 pages = {1--25},
 shorttitle = {{VulANalyzeR}},
 title = {{VulANalyzeR}: {Explainable} {Binary} {Vulnerability} {Detection} with {Multi}-task {Learning} and {Attentional} {Graph} {Convolution}},
 url = {https://dl.acm.org/doi/10.1145/3585386},
 urldate = {2025-06-03},
 volume = {26},
 year = {2023}
}
</rdfs:comment>
        <rdfs:label>li_vulanalyzer_2023</rdfs:label>
        <rdfs:seeAlso rdf:resource="https://dl.acm.org/doi/10.1145/3585386"/>
    </owl:NamedIndividual>
    


    <!-- http://purl.org/ai4se/ontology#liang_large-scale_2023 -->

    <owl:NamedIndividual rdf:about="http://purl.org/ai4se/ontology#liang_large-scale_2023">
        <rdf:type rdf:resource="http://purl.org/ai4se/ontology#ResearchPaper"/>
        <hasLevel rdf:resource="http://purl.org/ai4se/ontology#null"/>
        <hasPurpose rdf:resource="http://purl.org/ai4se/ontology#null"/>
        <hasTarget rdf:resource="http://purl.org/ai4se/ontology#null"/>
        <hasType rdf:resource="http://purl.org/ai4se/ontology#null"/>
        <isAboutResearchTopic rdf:resource="http://purl.org/ai4se/ontology#CSO:Testing_and_debugging"/>
        <rdfs:comment>@article{liang_large-scale_2023,
 author = {Liang, Jenny T. and Yang, Chenyang and Myers, B.},
 doi = {10.1145/3597503.3608128},
 journal = {International Conference on Software Engineering},
 pmcid = {null},
 pmid = {null},
 title = {A {Large}-{Scale} {Survey} on the {Usability} of {AI} {Programming} {Assistants}: {Successes} and {Challenges}},
 year = {2023}
}
</rdfs:comment>
        <rdfs:label>liang_large-scale_2023</rdfs:label>
        <rdfs:seeAlso rdf:resource="https://doi.org/10.1145/3597503.3608128"/>
    </owl:NamedIndividual>
    


    <!-- http://purl.org/ai4se/ontology#lin_traceability_2021 -->

    <owl:NamedIndividual rdf:about="http://purl.org/ai4se/ontology#lin_traceability_2021">
        <rdf:type rdf:resource="http://purl.org/ai4se/ontology#ResearchPaper"/>
        <hasLevel rdf:resource="http://purl.org/ai4se/ontology#AI-driven_partial_automation"/>
        <hasPurpose rdf:resource="http://purl.org/ai4se/ontology#Generate"/>
        <hasTarget rdf:resource="http://purl.org/ai4se/ontology#Develop"/>
        <hasType rdf:resource="http://purl.org/ai4se/ontology#Deep_learning"/>
        <isAboutResearchTopic rdf:resource="http://purl.org/ai4se/ontology#CSO:Software_traceability"/>
        <rdfs:comment>@inproceedings{lin_traceability_2021,
 author = {Lin, Jinfeng and Liu, Yalin and Zeng, Qingkai and Jiang, Meng and Cleland-Huang, Jane},
 booktitle = {2021 {IEEE}/{ACM} 43rd {International} {Conference} on {Software} {Engineering} ({ICSE})},
 doi = {10.1109/ICSE43902.2021.00040},
 pages = {324--335},
 publisher = {IEEE},
 title = {Traceability transformed: {Generating} more accurate links with pre-trained bert models},
 year = {2021}
}
</rdfs:comment>
        <rdfs:label>lin_traceability_2021</rdfs:label>
        <rdfs:seeAlso rdf:resource="https://doi.org/10.1109/ICSE43902.2021.00040"/>
    </owl:NamedIndividual>
    


    <!-- http://purl.org/ai4se/ontology#liu_generating_2022 -->

    <owl:NamedIndividual rdf:about="http://purl.org/ai4se/ontology#liu_generating_2022">
        <rdf:type rdf:resource="http://purl.org/ai4se/ontology#ResearchPaper"/>
        <hasLevel rdf:resource="http://purl.org/ai4se/ontology#null"/>
        <hasPurpose rdf:resource="http://purl.org/ai4se/ontology#null"/>
        <hasTarget rdf:resource="http://purl.org/ai4se/ontology#null"/>
        <hasType rdf:resource="http://purl.org/ai4se/ontology#null"/>
        <isAboutResearchTopic rdf:resource="http://purl.org/ai4se/ontology#CSO:Testing_and_debugging"/>
        <rdfs:comment>@inproceedings{liu_generating_2022,
 address = {Pittsburgh Pennsylvania},
 author = {Liu, Yalin and Lin, Jinfeng and Anuyah, Oghenemaro and Metoyer, Ronald and Cleland-Huang, Jane},
 booktitle = {Proceedings of the 44th {International} {Conference} on {Software} {Engineering}},
 doi = {10.1145/3510003.3510129},
  isbn = {978-1-4503-9221-1},
 language = {en},
 month = {May},
 pages = {1033--1044},
 publisher = {ACM},
 title = {Generating and visualizing trace link explanations},
 url = {https://dl.acm.org/doi/10.1145/3510003.3510129},
 urldate = {2025-06-03},
 year = {2022}
}
</rdfs:comment>
        <rdfs:label>liu_generating_2022</rdfs:label>
        <rdfs:seeAlso rdf:resource="https://dl.acm.org/doi/10.1145/3510003.3510129"/>
    </owl:NamedIndividual>
    


    <!-- http://purl.org/ai4se/ontology#lu_codexglue_2021 -->

    <owl:NamedIndividual rdf:about="http://purl.org/ai4se/ontology#lu_codexglue_2021">
        <rdf:type rdf:resource="http://purl.org/ai4se/ontology#ResearchPaper"/>
        <hasLevel rdf:resource="http://purl.org/ai4se/ontology#null"/>
        <hasPurpose rdf:resource="http://purl.org/ai4se/ontology#null"/>
        <hasTarget rdf:resource="http://purl.org/ai4se/ontology#null"/>
        <hasType rdf:resource="http://purl.org/ai4se/ontology#null"/>
        <isAboutResearchTopic rdf:resource="http://purl.org/ai4se/ontology#CSO:Testing_and_debugging"/>
        <rdfs:comment>@misc{lu_codexglue_2021,
 author = {Lu, Shuai and Guo, Daya and Ren, Shuo and Huang, Junjie and Svyatkovskiy, Alexey and Blanco, Ambrosio and Clement, Colin and Drain, Dawn and Jiang, Daxin and Tang, Duyu and Li, Ge and Zhou, Lidong and Shou, Linjun and Zhou, Long and Tufano, Michele and Gong, Ming and Zhou, Ming and Duan, Nan and Sundaresan, Neel and Deng, Shao Kun and Fu, Shengyu and Liu, Shujie},
 copyright = {arXiv.org perpetual, non-exclusive license},
 doi = {10.48550/ARXIV.2102.04664},
 keywords = {FOS: Computer and information sciences, Software Engineering (cs.SE), Computation and Language (cs.CL)},
 note = {Version Number: 2},
 publisher = {arXiv},
 shorttitle = {{CodeXGLUE}},
 title = {{CodeXGLUE}: {A} {Machine} {Learning} {Benchmark} {Dataset} for {Code} {Understanding} and {Generation}},
 url = {https://arxiv.org/abs/2102.04664},
 urldate = {2025-06-03},
 year = {2021}
}
</rdfs:comment>
        <rdfs:label>lu_codexglue_2021</rdfs:label>
        <rdfs:seeAlso rdf:resource="https://arxiv.org/abs/2102.04664"/>
    </owl:NamedIndividual>
    


    <!-- http://purl.org/ai4se/ontology#mahbub_explaining_2023 -->

    <owl:NamedIndividual rdf:about="http://purl.org/ai4se/ontology#mahbub_explaining_2023">
        <rdf:type rdf:resource="http://purl.org/ai4se/ontology#ResearchPaper"/>
        <hasLevel rdf:resource="http://purl.org/ai4se/ontology#null"/>
        <hasPurpose rdf:resource="http://purl.org/ai4se/ontology#null"/>
        <hasTarget rdf:resource="http://purl.org/ai4se/ontology#null"/>
        <hasType rdf:resource="http://purl.org/ai4se/ontology#null"/>
        <isAboutResearchTopic rdf:resource="http://purl.org/ai4se/ontology#CSO:Testing_and_debugging"/>
        <rdfs:comment>@inproceedings{mahbub_explaining_2023,
 address = {Melbourne, Australia},
 author = {Mahbub, Parvez and Shuvo, Ohiduzzaman and Rahman, Mohammad Masudur},
 booktitle = {2023 {IEEE}/{ACM} 45th {International} {Conference} on {Software} {Engineering} ({ICSE})},
 copyright = {https://doi.org/10.15223/policy-029},
 doi = {10.1109/ICSE48619.2023.00063},
  isbn = {978-1-6654-5701-9},
 month = {May},
 pages = {640--652},
 publisher = {IEEE},
 title = {Explaining {Software} {Bugs} {Leveraging} {Code} {Structures} in {Neural} {Machine} {Translation}},
 url = {https://ieeexplore.ieee.org/document/10172643/},
 urldate = {2025-06-03},
 year = {2023}
}
</rdfs:comment>
        <rdfs:label>mahbub_explaining_2023</rdfs:label>
        <rdfs:seeAlso rdf:resource="https://ieeexplore.ieee.org/document/10172643/"/>
    </owl:NamedIndividual>
    


    <!-- http://purl.org/ai4se/ontology#mastropaolo_robustness_2023 -->

    <owl:NamedIndividual rdf:about="http://purl.org/ai4se/ontology#mastropaolo_robustness_2023">
        <rdf:type rdf:resource="http://purl.org/ai4se/ontology#ResearchPaper"/>
        <hasLevel rdf:resource="http://purl.org/ai4se/ontology#null"/>
        <hasPurpose rdf:resource="http://purl.org/ai4se/ontology#null"/>
        <hasTarget rdf:resource="http://purl.org/ai4se/ontology#null"/>
        <hasType rdf:resource="http://purl.org/ai4se/ontology#null"/>
        <isAboutResearchTopic rdf:resource="http://purl.org/ai4se/ontology#CSO:Testing_and_debugging"/>
        <rdfs:comment>@inproceedings{mastropaolo_robustness_2023,
 address = {Melbourne, Australia},
 author = {Mastropaolo, Antonio and Pascarella, Luca and Guglielmi, Emanuela and Ciniselli, Matteo and Scalabrino, Simone and Oliveto, Rocco and Bavota, Gabriele},
 booktitle = {2023 {IEEE}/{ACM} 45th {International} {Conference} on {Software} {Engineering} ({ICSE})},
 copyright = {https://doi.org/10.15223/policy-029},
 doi = {10.1109/ICSE48619.2023.00181},
  isbn = {978-1-6654-5701-9},
 month = {May},
 pages = {2149--2160},
 publisher = {IEEE},
 shorttitle = {On the {Robustness} of {Code} {Generation} {Techniques}},
 title = {On the {Robustness} of {Code} {Generation} {Techniques}: {An} {Empirical} {Study} on {GitHub} {Copilot}},
 url = {https://ieeexplore.ieee.org/document/10172792/},
 urldate = {2025-06-03},
 year = {2023}
}
</rdfs:comment>
        <rdfs:label>mastropaolo_robustness_2023</rdfs:label>
        <rdfs:seeAlso rdf:resource="https://ieeexplore.ieee.org/document/10172792/"/>
    </owl:NamedIndividual>
    


    <!-- http://purl.org/ai4se/ontology#nguyen-duc_transforming_2024 -->

    <owl:NamedIndividual rdf:about="http://purl.org/ai4se/ontology#nguyen-duc_transforming_2024">
        <rdf:type rdf:resource="http://purl.org/ai4se/ontology#ResearchPaper"/>
        <hasLevel rdf:resource="http://purl.org/ai4se/ontology#null"/>
        <hasPurpose rdf:resource="http://purl.org/ai4se/ontology#null"/>
        <hasTarget rdf:resource="http://purl.org/ai4se/ontology#null"/>
        <hasType rdf:resource="http://purl.org/ai4se/ontology#null"/>
        <isAboutResearchTopic rdf:resource="http://purl.org/ai4se/ontology#CSO:Testing_and_debugging"/>
        <rdfs:comment>@incollection{nguyen-duc_transforming_2024,
 address = {Cham},
 author = {Ulfsnes, Rasmus and Moe, Nils Brede and Stray, Viktoria and Skarpen, Marianne},
 booktitle = {Generative {AI} for {Effective} {Software} {Development}},
 doi = {10.1007/978-3-031-55642-5_10},
 editor = {Nguyen-Duc, Anh and Abrahamsson, Pekka and Khomh, Foutse},
 isbn = {978-3-031-55641-8 978-3-031-55642-5},
 language = {en},
 pages = {219--234},
 publisher = {Springer Nature Switzerland},
 shorttitle = {Transforming {Software} {Development} with {Generative} {AI}},
 title = {Transforming {Software} {Development} with {Generative} {AI}: {Empirical} {Insights} on {Collaboration} and {Workflow}},
 url = {https://link.springer.com/10.1007/978-3-031-55642-5_10},
 urldate = {2025-06-03},
 year = {2024}
}
</rdfs:comment>
        <rdfs:label>nguyen-duc_transforming_2024</rdfs:label>
        <rdfs:seeAlso rdf:resource="https://link.springer.com/10.1007/978-3-031-55642-5_10"/>
    </owl:NamedIndividual>
    


    <!-- http://purl.org/ai4se/ontology#niu_crosscodebench_2023 -->

    <owl:NamedIndividual rdf:about="http://purl.org/ai4se/ontology#niu_crosscodebench_2023">
        <rdf:type rdf:resource="http://purl.org/ai4se/ontology#ResearchPaper"/>
        <hasLevel rdf:resource="http://purl.org/ai4se/ontology#null"/>
        <hasPurpose rdf:resource="http://purl.org/ai4se/ontology#null"/>
        <hasTarget rdf:resource="http://purl.org/ai4se/ontology#null"/>
        <hasType rdf:resource="http://purl.org/ai4se/ontology#null"/>
        <isAboutResearchTopic rdf:resource="http://purl.org/ai4se/ontology#CSO:Testing_and_debugging"/>
        <rdfs:comment>@inproceedings{niu_crosscodebench_2023,
 address = {Melbourne, Australia},
 author = {Niu, Changan and Li, Chuanyi and Ng, Vincent and Luo, Bin},
 booktitle = {2023 {IEEE}/{ACM} 45th {International} {Conference} on {Software} {Engineering} ({ICSE})},
 copyright = {https://doi.org/10.15223/policy-029},
 doi = {10.1109/ICSE48619.2023.00055},
  isbn = {978-1-6654-5701-9},
 month = {May},
 pages = {537--549},
 publisher = {IEEE},
 shorttitle = {{CrossCodeBench}},
 title = {{CrossCodeBench}: {Benchmarking} {Cross}-{Task} {Generalization} of {Source} {Code} {Models}},
 url = {https://ieeexplore.ieee.org/document/10172565/},
 urldate = {2025-06-03},
 year = {2023}
}
</rdfs:comment>
        <rdfs:label>niu_crosscodebench_2023</rdfs:label>
        <rdfs:seeAlso rdf:resource="https://ieeexplore.ieee.org/document/10172565/"/>
    </owl:NamedIndividual>
    


    <!-- http://purl.org/ai4se/ontology#null -->

    <owl:Thing rdf:about="http://purl.org/ai4se/ontology#null">
        <rdf:type rdf:resource="http://www.w3.org/2002/07/owl#NamedIndividual"/>
    </owl:Thing>
    


    <!-- http://purl.org/ai4se/ontology#ortin_big_2016 -->

    <owl:NamedIndividual rdf:about="http://purl.org/ai4se/ontology#ortin_big_2016">
        <rdf:type rdf:resource="http://purl.org/ai4se/ontology#ResearchPaper"/>
        <hasLevel rdf:resource="http://purl.org/ai4se/ontology#null"/>
        <hasPurpose rdf:resource="http://purl.org/ai4se/ontology#null"/>
        <hasTarget rdf:resource="http://purl.org/ai4se/ontology#null"/>
        <hasType rdf:resource="http://purl.org/ai4se/ontology#null"/>
        <isAboutResearchTopic rdf:resource="http://purl.org/ai4se/ontology#CSO:Testing_and_debugging"/>
        <rdfs:comment>@article{ortin_big_2016,
 author = {Ortin, Francisco and Escalada, Javier and Rodriguez-Prieto, Oscar},
 journal = {J. Softw.},
 number = {11},
 pages = {1083--1088},
 title = {Big {Code}: {New} {Opportunities} for {Improving} {Software} {Construction}},
 volume = {11},
 year = {2016}
}
</rdfs:comment>
        <rdfs:label>ortin_big_2016</rdfs:label>
    </owl:NamedIndividual>
    


    <!-- http://purl.org/ai4se/ontology#palomba_predicting_2021 -->

    <owl:NamedIndividual rdf:about="http://purl.org/ai4se/ontology#palomba_predicting_2021">
        <rdf:type rdf:resource="http://purl.org/ai4se/ontology#ResearchPaper"/>
        <hasLevel rdf:resource="http://purl.org/ai4se/ontology#null"/>
        <hasPurpose rdf:resource="http://purl.org/ai4se/ontology#null"/>
        <hasTarget rdf:resource="http://purl.org/ai4se/ontology#null"/>
        <hasType rdf:resource="http://purl.org/ai4se/ontology#null"/>
        <isAboutResearchTopic rdf:resource="http://purl.org/ai4se/ontology#CSO:Testing_and_debugging"/>
        <rdfs:comment>@article{palomba_predicting_2021,
 author = {Palomba, Fabio and Tamburri, Damian Andrew},
 doi = {10.1016/j.jss.2020.110847},
 issn = {01641212},
 journal = {Journal of Systems and Software},
 language = {en},
 month = {January},
 pages = {110847},
 shorttitle = {Predicting the emergence of community smells using socio-technical metrics},
 title = {Predicting the emergence of community smells using socio-technical metrics: {A} machine-learning approach},
 url = {https://linkinghub.elsevier.com/retrieve/pii/S0164121220302375},
 urldate = {2025-06-03},
 volume = {171},
 year = {2021}
}
</rdfs:comment>
        <rdfs:label>palomba_predicting_2021</rdfs:label>
        <rdfs:seeAlso rdf:resource="https://linkinghub.elsevier.com/retrieve/pii/S0164121220302375"/>
    </owl:NamedIndividual>
    


    <!-- http://purl.org/ai4se/ontology#peng_impact_2023 -->

    <owl:NamedIndividual rdf:about="http://purl.org/ai4se/ontology#peng_impact_2023">
        <rdf:type rdf:resource="http://purl.org/ai4se/ontology#ResearchPaper"/>
        <hasLevel rdf:resource="http://purl.org/ai4se/ontology#null"/>
        <hasPurpose rdf:resource="http://purl.org/ai4se/ontology#null"/>
        <hasTarget rdf:resource="http://purl.org/ai4se/ontology#null"/>
        <hasType rdf:resource="http://purl.org/ai4se/ontology#null"/>
        <isAboutResearchTopic rdf:resource="http://purl.org/ai4se/ontology#CSO:Testing_and_debugging"/>
        <rdfs:comment>@misc{peng_impact_2023,
 author = {Peng, Sida and Kalliamvakou, Eirini and Cihon, Peter and Demirer, Mert},
 copyright = {arXiv.org perpetual, non-exclusive license},
 doi = {10.48550/ARXIV.2302.06590},
 keywords = {FOS: Computer and information sciences, Software Engineering (cs.SE)},
 note = {Version Number: 1},
 publisher = {arXiv},
 shorttitle = {The {Impact} of {AI} on {Developer} {Productivity}},
 title = {The {Impact} of {AI} on {Developer} {Productivity}: {Evidence} from {GitHub} {Copilot}},
 url = {https://arxiv.org/abs/2302.06590},
 urldate = {2025-06-03},
 year = {2023}
}
</rdfs:comment>
        <rdfs:label>peng_impact_2023</rdfs:label>
        <rdfs:seeAlso rdf:resource="https://arxiv.org/abs/2302.06590"/>
    </owl:NamedIndividual>
    


    <!-- http://purl.org/ai4se/ontology#perini_machine_2012 -->

    <owl:NamedIndividual rdf:about="http://purl.org/ai4se/ontology#perini_machine_2012">
        <rdf:type rdf:resource="http://purl.org/ai4se/ontology#ResearchPaper"/>
        <hasLevel rdf:resource="http://purl.org/ai4se/ontology#AI-assisted_selection"/>
        <hasPurpose rdf:resource="http://purl.org/ai4se/ontology#Improve"/>
        <hasTarget rdf:resource="http://purl.org/ai4se/ontology#Deployment"/>
        <hasTarget rdf:resource="http://purl.org/ai4se/ontology#Management"/>
        <hasTarget rdf:resource="http://purl.org/ai4se/ontology#Requirements"/>
        <hasType rdf:resource="http://purl.org/ai4se/ontology#Classical_machine_learning"/>
        <isAboutResearchTopic rdf:resource="http://purl.org/ai4se/ontology#CSO:Requirements_engineering"/>
        <rdfs:comment>@article{perini_machine_2012,
 author = {Perini, Anna and Susi, Angelo and Avesani, Paolo},
 doi = {10.1109/TSE.2012.52},
 journal = {IEEE Transactions on Software Engineering},
 note = {Publisher: IEEE},
 number = {4},
 pages = {445--461},
 title = {A machine learning approach to software requirements prioritization},
 volume = {39},
 year = {2012}
}
</rdfs:comment>
        <rdfs:label>perini_machine_2012</rdfs:label>
        <rdfs:seeAlso rdf:resource="https://doi.org/10.1109/TSE.2012.52"/>
    </owl:NamedIndividual>
    


    <!-- http://purl.org/ai4se/ontology#pudari_copilot_2023 -->

    <owl:NamedIndividual rdf:about="http://purl.org/ai4se/ontology#pudari_copilot_2023">
        <rdf:type rdf:resource="http://purl.org/ai4se/ontology#ResearchPaper"/>
        <hasLevel rdf:resource="http://purl.org/ai4se/ontology#null"/>
        <hasPurpose rdf:resource="http://purl.org/ai4se/ontology#null"/>
        <hasTarget rdf:resource="http://purl.org/ai4se/ontology#null"/>
        <hasType rdf:resource="http://purl.org/ai4se/ontology#null"/>
        <isAboutResearchTopic rdf:resource="http://purl.org/ai4se/ontology#CSO:Testing_and_debugging"/>
        <rdfs:comment>@article{pudari_copilot_2023,
 author = {Pudari, Rohith and Ernst, Neil A.},
 doi = {10.48550/arxiv.2303.04142},
 journal = {arXiv preprint arXiv:2303.04142},
 pmcid = {null},
 pmid = {null},
 title = {From {Copilot} to {Pilot}: {Towards} {AI} {Supported} {Software} {Development}},
 year = {2023}
}
</rdfs:comment>
        <rdfs:label>pudari_copilot_2023</rdfs:label>
        <rdfs:seeAlso rdf:resource="https://doi.org/10.48550/arxiv.2303.04142"/>
    </owl:NamedIndividual>
    


    <!-- http://purl.org/ai4se/ontology#roziere_leveraging_2021 -->

    <owl:NamedIndividual rdf:about="http://purl.org/ai4se/ontology#roziere_leveraging_2021">
        <rdf:type rdf:resource="http://purl.org/ai4se/ontology#ResearchPaper"/>
        <hasLevel rdf:resource="http://purl.org/ai4se/ontology#null"/>
        <hasPurpose rdf:resource="http://purl.org/ai4se/ontology#null"/>
        <hasTarget rdf:resource="http://purl.org/ai4se/ontology#null"/>
        <hasType rdf:resource="http://purl.org/ai4se/ontology#null"/>
        <isAboutResearchTopic rdf:resource="http://purl.org/ai4se/ontology#CSO:Testing_and_debugging"/>
        <rdfs:comment>@misc{roziere_leveraging_2021,
 author = {Roziere, Baptiste and Zhang, Jie M. and Charton, Francois and Harman, Mark and Synnaeve, Gabriel and Lample, Guillaume},
 copyright = {arXiv.org perpetual, non-exclusive license},
 doi = {10.48550/ARXIV.2110.06773},
 keywords = {FOS: Computer and information sciences, Machine Learning (cs.LG), Software Engineering (cs.SE), Computation and Language (cs.CL)},
 note = {Version Number: 2},
 publisher = {arXiv},
 title = {Leveraging {Automated} {Unit} {Tests} for {Unsupervised} {Code} {Translation}},
 url = {https://arxiv.org/abs/2110.06773},
 urldate = {2025-06-03},
 year = {2021}
}
</rdfs:comment>
        <rdfs:label>roziere_leveraging_2021</rdfs:label>
        <rdfs:seeAlso rdf:resource="https://arxiv.org/abs/2110.06773"/>
    </owl:NamedIndividual>
    


    <!-- http://purl.org/ai4se/ontology#samplePaper -->

    <owl:NamedIndividual rdf:about="http://purl.org/ai4se/ontology#samplePaper">
        <rdf:type rdf:resource="http://purl.org/ai4se/ontology#ResearchPaper"/>
        <hasLevel rdf:resource="http://purl.org/ai4se/ontology#AI-assisted_selection"/>
        <hasPurpose rdf:resource="http://purl.org/ai4se/ontology#Improve"/>
        <hasPurpose rdf:resource="http://purl.org/ai4se/ontology#Understand"/>
        <hasTarget rdf:resource="http://purl.org/ai4se/ontology#Testing"/>
        <hasType rdf:resource="http://purl.org/ai4se/ontology#Deep_learning"/>
        <isAboutResearchTopic rdf:resource="http://purl.org/ai4se/ontology#CSO:Testing_and_debugging"/>
    </owl:NamedIndividual>
    


    <!-- http://purl.org/ai4se/ontology#shafiq_nlp4ip_2021 -->

    <owl:NamedIndividual rdf:about="http://purl.org/ai4se/ontology#shafiq_nlp4ip_2021">
        <rdf:type rdf:resource="http://purl.org/ai4se/ontology#ResearchPaper"/>
        <hasLevel rdf:resource="http://purl.org/ai4se/ontology#null"/>
        <hasPurpose rdf:resource="http://purl.org/ai4se/ontology#null"/>
        <hasTarget rdf:resource="http://purl.org/ai4se/ontology#null"/>
        <hasType rdf:resource="http://purl.org/ai4se/ontology#null"/>
        <isAboutResearchTopic rdf:resource="http://purl.org/ai4se/ontology#CSO:Testing_and_debugging"/>
        <rdfs:comment>@inproceedings{shafiq_nlp4ip_2021,
 address = {Palermo, Italy},
 author = {Shafiq, Saad and Mashkoor, Atif and Mayr-Dorn, Christoph and Egyed, Alexander},
 booktitle = {2021 47th {Euromicro} {Conference} on {Software} {Engineering} and {Advanced} {Applications} ({SEAA})},
 copyright = {https://ieeexplore.ieee.org/Xplorehelp/downloads/license-information/IEEE.html},
 doi = {10.1109/SEAA53835.2021.00022},
 isbn = {978-1-6654-2705-0},
 month = {September},
 pages = {99--108},
 publisher = {IEEE},
 shorttitle = {{NLP4IP}},
 title = {{NLP4IP}: {Natural} {Language} {Processing}-based {Recommendation} {Approach} for {Issues} {Prioritization}},
 url = {https://ieeexplore.ieee.org/document/9582582/},
 urldate = {2025-06-03},
 year = {2021}
}
</rdfs:comment>
        <rdfs:label>shafiq_nlp4ip_2021</rdfs:label>
        <rdfs:seeAlso rdf:resource="https://ieeexplore.ieee.org/document/9582582/"/>
    </owl:NamedIndividual>
    


    <!-- http://purl.org/ai4se/ontology#siavvas_technical_2022 -->

    <owl:NamedIndividual rdf:about="http://purl.org/ai4se/ontology#siavvas_technical_2022">
        <rdf:type rdf:resource="http://purl.org/ai4se/ontology#ResearchPaper"/>
        <hasLevel rdf:resource="http://purl.org/ai4se/ontology#null"/>
        <hasPurpose rdf:resource="http://purl.org/ai4se/ontology#null"/>
        <hasTarget rdf:resource="http://purl.org/ai4se/ontology#null"/>
        <hasType rdf:resource="http://purl.org/ai4se/ontology#null"/>
        <isAboutResearchTopic rdf:resource="http://purl.org/ai4se/ontology#CSO:Testing_and_debugging"/>
        <rdfs:comment>@article{siavvas_technical_2022,
 author = {Siavvas, Miltiadis and Tsoukalas, Dimitrios and Jankovic, Marija and Kehagias, Dionysios and Tzovaras, Dimitrios},
 doi = {10.1080/17517575.2020.1824017},
 issn = {1751-7575, 1751-7583},
 journal = {Enterprise Information Systems},
 language = {en},
 month = {May},
 number = {5},
 pages = {1824017},
 shorttitle = {Technical debt as an indicator of software security risk},
 title = {Technical debt as an indicator of software security risk: a machine learning approach for software development enterprises},
 url = {https://www.tandfonline.com/doi/full/10.1080/17517575.2020.1824017},
 urldate = {2025-06-03},
 volume = {16},
 year = {2022}
}
</rdfs:comment>
        <rdfs:label>siavvas_technical_2022</rdfs:label>
        <rdfs:seeAlso rdf:resource="https://www.tandfonline.com/doi/full/10.1080/17517575.2020.1824017"/>
    </owl:NamedIndividual>
    


    <!-- http://purl.org/ai4se/ontology#singh_study_2021 -->

    <owl:NamedIndividual rdf:about="http://purl.org/ai4se/ontology#singh_study_2021">
        <rdf:type rdf:resource="http://purl.org/ai4se/ontology#ResearchPaper"/>
        <hasLevel rdf:resource="http://purl.org/ai4se/ontology#null"/>
        <hasPurpose rdf:resource="http://purl.org/ai4se/ontology#null"/>
        <hasTarget rdf:resource="http://purl.org/ai4se/ontology#null"/>
        <hasType rdf:resource="http://purl.org/ai4se/ontology#null"/>
        <isAboutResearchTopic rdf:resource="http://purl.org/ai4se/ontology#CSO:Testing_and_debugging"/>
        <rdfs:comment>@inproceedings{singh_study_2021,
 address = {Coimbatore, India},
 author = {Singh, Shilpi and Saikia, L P and Baruah, Sunandan},
 booktitle = {2021 {Second} {International} {Conference} on {Electronics} and {Sustainable} {Communication} {Systems} ({ICESC})},
 copyright = {https://ieeexplore.ieee.org/Xplorehelp/downloads/license-information/IEEE.html},
 doi = {10.1109/ICESC51422.2021.9532736},
 isbn = {978-1-6654-2867-5},
 month = {August},
 pages = {1541--1548},
 publisher = {IEEE},
 title = {A study on {Quality} {Assessment} of {Requirement} {Engineering} {Document} using {Text} {Classification} {Technique}},
 url = {https://ieeexplore.ieee.org/document/9532736/},
 urldate = {2025-06-03},
 year = {2021}
}
</rdfs:comment>
        <rdfs:label>singh_study_2021</rdfs:label>
        <rdfs:seeAlso rdf:resource="https://ieeexplore.ieee.org/document/9532736/"/>
    </owl:NamedIndividual>
    


    <!-- http://purl.org/ai4se/ontology#soeken_assisted_2012 -->

    <owl:NamedIndividual rdf:about="http://purl.org/ai4se/ontology#soeken_assisted_2012">
        <rdf:type rdf:resource="http://purl.org/ai4se/ontology#ResearchPaper"/>
        <hasLevel rdf:resource="http://purl.org/ai4se/ontology#null"/>
        <hasPurpose rdf:resource="http://purl.org/ai4se/ontology#null"/>
        <hasTarget rdf:resource="http://purl.org/ai4se/ontology#null"/>
        <hasType rdf:resource="http://purl.org/ai4se/ontology#null"/>
        <isAboutResearchTopic rdf:resource="http://purl.org/ai4se/ontology#CSO:Testing_and_debugging"/>
        <rdfs:comment>@inproceedings{soeken_assisted_2012,
 author = {Soeken, Mathias and Wille, Robert and Drechsler, Rolf},
 booktitle = {Objects, {Models}, {Components}, {Patterns}: 50th {International} {Conference}, {TOOLS} 2012, {Prague}, {Czech} {Republic}, {May} 29-31, 2012. {Proceedings} 50},
 doi = {10.1007/978-3-642-30561-0_19},
 pages = {269--287},
 publisher = {Springer},
 title = {Assisted behavior driven development using natural language processing},
 year = {2012}
}
</rdfs:comment>
        <rdfs:label>soeken_assisted_2012</rdfs:label>
        <rdfs:seeAlso rdf:resource="https://doi.org/10.1007/978-3-642-30561-0_19"/>
    </owl:NamedIndividual>
    


    <!-- http://purl.org/ai4se/ontology#spieker_reinforcement_2017 -->

    <owl:NamedIndividual rdf:about="http://purl.org/ai4se/ontology#spieker_reinforcement_2017">
        <rdf:type rdf:resource="http://purl.org/ai4se/ontology#ResearchPaper"/>
        <hasLevel rdf:resource="http://purl.org/ai4se/ontology#AI-driven_partial_automation"/>
        <hasPurpose rdf:resource="http://purl.org/ai4se/ontology#Improve"/>
        <hasTarget rdf:resource="http://purl.org/ai4se/ontology#Testing"/>
        <hasType rdf:resource="http://purl.org/ai4se/ontology#Deep_learning"/>
        <isAboutResearchTopic rdf:resource="http://purl.org/ai4se/ontology#CSO:Testing_and_debugging"/>
        <rdfs:comment>@inproceedings{spieker_reinforcement_2017,
 author = {Spieker, Helge and Gotlieb, Arnaud and Marijan, Dusica and Mossige, Morten},
 booktitle = {Proceedings of the 26th {ACM} {SIGSOFT} international symposium on software testing and analysis},
 doi = {10.1145/3092703.3092709},
 pages = {12--22},
 title = {Reinforcement learning for automatic test case prioritization and selection in continuous integration},
 year = {2017}
}
</rdfs:comment>
        <rdfs:label>spieker_reinforcement_2017</rdfs:label>
        <rdfs:seeAlso rdf:resource="https://doi.org/10.1145/3092703.3092709"/>
    </owl:NamedIndividual>
    


    <!-- http://purl.org/ai4se/ontology#svyatkovskiy_intellicode_2020 -->

    <owl:NamedIndividual rdf:about="http://purl.org/ai4se/ontology#svyatkovskiy_intellicode_2020">
        <rdf:type rdf:resource="http://purl.org/ai4se/ontology#ResearchPaper"/>
        <hasLevel rdf:resource="http://purl.org/ai4se/ontology#AI-driven_partial_automation"/>
        <hasPurpose rdf:resource="http://purl.org/ai4se/ontology#Generate"/>
        <hasPurpose rdf:resource="http://purl.org/ai4se/ontology#Improve"/>
        <hasTarget rdf:resource="http://purl.org/ai4se/ontology#Coding"/>
        <hasType rdf:resource="http://purl.org/ai4se/ontology#Generative_AI"/>
        <isAboutResearchTopic rdf:resource="http://purl.org/ai4se/ontology#CSO:Traceability_management"/>
        <rdfs:comment>@inproceedings{svyatkovskiy_intellicode_2020,
 author = {Svyatkovskiy, Alexey and Deng, Shao Kun and Fu, Shengyu and Sundaresan, Neel},
 booktitle = {Proceedings of the 28th {ACM} joint meeting on {European} software engineering conference and symposium on the foundations of software engineering},
 doi = {10.1145/3368089.3417058},
 pages = {1433--1443},
 title = {Intellicode compose: {Code} generation using transformer},
 year = {2020}
}
</rdfs:comment>
        <rdfs:label>svyatkovskiy_intellicode_2020</rdfs:label>
        <rdfs:seeAlso rdf:resource="https://doi.org/10.1145/3368089.3417058"/>
    </owl:NamedIndividual>
    


    <!-- http://purl.org/ai4se/ontology#tamizharasi_novel_2024 -->

    <owl:NamedIndividual rdf:about="http://purl.org/ai4se/ontology#tamizharasi_novel_2024">
        <rdf:type rdf:resource="http://purl.org/ai4se/ontology#ResearchPaper"/>
        <hasLevel rdf:resource="http://purl.org/ai4se/ontology#null"/>
        <hasPurpose rdf:resource="http://purl.org/ai4se/ontology#null"/>
        <hasTarget rdf:resource="http://purl.org/ai4se/ontology#null"/>
        <hasType rdf:resource="http://purl.org/ai4se/ontology#null"/>
        <isAboutResearchTopic rdf:resource="http://purl.org/ai4se/ontology#CSO:Testing_and_debugging"/>
        <rdfs:comment>@article{tamizharasi_novel_2024,
 author = {Tamizharasi, A and Ezhumalai, P},
 doi = {10.1007/s10836-024-06121-x},
 journal = {Journal of Electronic Testing},
 note = {Publisher: Springer},
 pages = {1--24},
 title = {A {Novel} {Framework} {For} {Optimal} {Test} {Case} {Generation} and {Prioritization} {Using} {Ent}-{LSOA} {And} {IMTRNN} {Techniques}},
 year = {2024}
}
</rdfs:comment>
        <rdfs:label>tamizharasi_novel_2024</rdfs:label>
        <rdfs:seeAlso rdf:resource="https://doi.org/10.1007/s10836-024-06121-x"/>
    </owl:NamedIndividual>
    


    <!-- http://purl.org/ai4se/ontology#tatineni_integrating_2024 -->

    <owl:NamedIndividual rdf:about="http://purl.org/ai4se/ontology#tatineni_integrating_2024">
        <rdf:type rdf:resource="http://purl.org/ai4se/ontology#ResearchPaper"/>
        <hasLevel rdf:resource="http://purl.org/ai4se/ontology#AI-driven_partial_automation"/>
        <hasPurpose rdf:resource="http://purl.org/ai4se/ontology#Improve"/>
        <hasPurpose rdf:resource="http://purl.org/ai4se/ontology#Understand"/>
        <hasTarget rdf:resource="http://purl.org/ai4se/ontology#Improvement"/>
        <hasTarget rdf:resource="http://purl.org/ai4se/ontology#Maintenance"/>
        <hasTarget rdf:resource="http://purl.org/ai4se/ontology#Monitoring"/>
        <hasType rdf:resource="http://purl.org/ai4se/ontology#null"/>
        <isAboutResearchTopic rdf:resource="http://purl.org/ai4se/ontology#CSO:DevOps"/>
        <rdfs:comment>@book{tatineni_integrating_2024,
 author = {Tatineni, Sumanth},
 publisher = {Libertatem Media Private Limited},
 title = {Integrating {Artificial} {Intelligence} with {DevOps}: {Advanced} {Techniques}, {Predictive} {Analytics}, and {Automation} for {Real}-{Time} {Optimization} and {Security} in {Modern} {Software} {Development}},
 year = {2024}
}
</rdfs:comment>
        <rdfs:label>tatineni_integrating_2024</rdfs:label>
    </owl:NamedIndividual>
    


    <!-- http://purl.org/ai4se/ontology#tufano_autodev_2024 -->

    <owl:NamedIndividual rdf:about="http://purl.org/ai4se/ontology#tufano_autodev_2024">
        <rdf:type rdf:resource="http://purl.org/ai4se/ontology#ResearchPaper"/>
        <hasLevel rdf:resource="http://purl.org/ai4se/ontology#null"/>
        <hasPurpose rdf:resource="http://purl.org/ai4se/ontology#null"/>
        <hasTarget rdf:resource="http://purl.org/ai4se/ontology#null"/>
        <hasType rdf:resource="http://purl.org/ai4se/ontology#null"/>
        <isAboutResearchTopic rdf:resource="http://purl.org/ai4se/ontology#CSO:Testing_and_debugging"/>
        <rdfs:comment>@misc{tufano_autodev_2024,
 author = {Tufano, Michele and Agarwal, Anisha and Jang, Jinu and Moghaddam, Roshanak Zilouchian and Sundaresan, Neel},
 copyright = {Creative Commons Attribution 4.0 International},
 doi = {10.48550/ARXIV.2403.08299},
 keywords = {FOS: Computer and information sciences, Software Engineering (cs.SE), Artificial Intelligence (cs.AI)},
 note = {Version Number: 1},
 publisher = {arXiv},
 shorttitle = {{AutoDev}},
 title = {{AutoDev}: {Automated} {AI}-{Driven} {Development}},
 url = {https://arxiv.org/abs/2403.08299},
 urldate = {2025-06-03},
 year = {2024}
}
</rdfs:comment>
        <rdfs:label>tufano_autodev_2024</rdfs:label>
        <rdfs:seeAlso rdf:resource="https://arxiv.org/abs/2403.08299"/>
    </owl:NamedIndividual>
    


    <!-- http://purl.org/ai4se/ontology#tufano_generating_2022 -->

    <owl:NamedIndividual rdf:about="http://purl.org/ai4se/ontology#tufano_generating_2022">
        <rdf:type rdf:resource="http://purl.org/ai4se/ontology#ResearchPaper"/>
        <hasLevel rdf:resource="http://purl.org/ai4se/ontology#AI-assisted_selection"/>
        <hasPurpose rdf:resource="http://purl.org/ai4se/ontology#Improve"/>
        <hasTarget rdf:resource="http://purl.org/ai4se/ontology#Coding"/>
        <hasTarget rdf:resource="http://purl.org/ai4se/ontology#Testing"/>
        <hasType rdf:resource="http://purl.org/ai4se/ontology#Generative_AI"/>
        <isAboutResearchTopic rdf:resource="http://purl.org/ai4se/ontology#CSO:Testing_and_debugging"/>
        <rdfs:comment>@inproceedings{tufano_generating_2022,
 address = {Pittsburgh Pennsylvania},
 author = {Tufano, Michele and Drain, Dawn and Svyatkovskiy, Alexey and Sundaresan, Neel},
 booktitle = {Proceedings of the 3rd {ACM}/{IEEE} {International} {Conference} on {Automation} of {Software} {Test}},
 doi = {10.1145/3524481.3527220},
  isbn = {978-1-4503-9286-0},
 language = {en},
 month = {May},
 pages = {54--64},
 publisher = {ACM},
 title = {Generating accurate assert statements for unit test cases using pretrained transformers},
 url = {https://dl.acm.org/doi/10.1145/3524481.3527220},
 urldate = {2025-06-03},
 year = {2022}
}
</rdfs:comment>
        <rdfs:label>tufano_generating_2022</rdfs:label>
        <rdfs:seeAlso rdf:resource="https://dl.acm.org/doi/10.1145/3524481.3527220"/>
    </owl:NamedIndividual>
    


    <!-- http://purl.org/ai4se/ontology#widyasari_xai4fl_2022 -->

    <owl:NamedIndividual rdf:about="http://purl.org/ai4se/ontology#widyasari_xai4fl_2022">
        <rdf:type rdf:resource="http://purl.org/ai4se/ontology#ResearchPaper"/>
        <hasLevel rdf:resource="http://purl.org/ai4se/ontology#null"/>
        <hasPurpose rdf:resource="http://purl.org/ai4se/ontology#null"/>
        <hasTarget rdf:resource="http://purl.org/ai4se/ontology#null"/>
        <hasType rdf:resource="http://purl.org/ai4se/ontology#null"/>
        <isAboutResearchTopic rdf:resource="http://purl.org/ai4se/ontology#CSO:Testing_and_debugging"/>
        <rdfs:comment>@inproceedings{widyasari_xai4fl_2022,
 address = {Virtual Event},
 author = {Widyasari, Ratnadira and Prana, Gede Artha Azriadi and Haryono, Stefanus A. and Tian, Yuan and Zachiary, Hafil Noer and Lo, David},
 booktitle = {Proceedings of the 30th {IEEE}/{ACM} {International} {Conference} on {Program} {Comprehension}},
 doi = {10.1145/3524610.3527902},
 isbn = {978-1-4503-9298-3},
 language = {en},
 month = {May},
 pages = {499--510},
 publisher = {ACM},
 shorttitle = {{XAI4FL}},
 title = {{XAI4FL}: enhancing spectrum-based fault localization with explainable artificial intelligence},
 url = {https://dl.acm.org/doi/10.1145/3524610.3527902},
 urldate = {2025-06-03},
 year = {2022}
}
</rdfs:comment>
        <rdfs:label>widyasari_xai4fl_2022</rdfs:label>
        <rdfs:seeAlso rdf:resource="https://dl.acm.org/doi/10.1145/3524610.3527902"/>
    </owl:NamedIndividual>
    


    <!-- http://purl.org/ai4se/ontology#xia_sequential_2022 -->

    <owl:NamedIndividual rdf:about="http://purl.org/ai4se/ontology#xia_sequential_2022">
        <rdf:type rdf:resource="http://purl.org/ai4se/ontology#ResearchPaper"/>
        <hasLevel rdf:resource="http://purl.org/ai4se/ontology#null"/>
        <hasPurpose rdf:resource="http://purl.org/ai4se/ontology#null"/>
        <hasTarget rdf:resource="http://purl.org/ai4se/ontology#null"/>
        <hasType rdf:resource="http://purl.org/ai4se/ontology#null"/>
        <isAboutResearchTopic rdf:resource="http://purl.org/ai4se/ontology#CSO:Testing_and_debugging"/>
        <rdfs:comment>@article{xia_sequential_2022,
 author = {Xia, Tianpei and Shu, Rui and Shen, Xipeng and Menzies, Tim},
 copyright = {https://ieeexplore.ieee.org/Xplorehelp/downloads/license-information/IEEE.html},
 doi = {10.1109/TSE.2020.3047072},
 issn = {0098-5589, 1939-3520, 2326-3881},
 journal = {IEEE Transactions on Software Engineering},
 month = {June},
 number = {6},
 pages = {1994--2009},
 title = {Sequential {Model} {Optimization} for {Software} {Effort} {Estimation}},
 url = {https://ieeexplore.ieee.org/document/9307246/},
 urldate = {2025-06-03},
 volume = {48},
 year = {2022}
}
</rdfs:comment>
        <rdfs:label>xia_sequential_2022</rdfs:label>
        <rdfs:seeAlso rdf:resource="https://ieeexplore.ieee.org/document/9307246/"/>
    </owl:NamedIndividual>
    


    <!-- http://purl.org/ai4se/ontology#xie_synergy_2013 -->

    <owl:NamedIndividual rdf:about="http://purl.org/ai4se/ontology#xie_synergy_2013">
        <rdf:type rdf:resource="http://purl.org/ai4se/ontology#ResearchPaper"/>
        <hasLevel rdf:resource="http://purl.org/ai4se/ontology#null"/>
        <hasPurpose rdf:resource="http://purl.org/ai4se/ontology#null"/>
        <hasTarget rdf:resource="http://purl.org/ai4se/ontology#null"/>
        <hasType rdf:resource="http://purl.org/ai4se/ontology#null"/>
        <isAboutResearchTopic rdf:resource="http://purl.org/ai4se/ontology#CSO:Testing_and_debugging"/>
        <rdfs:comment>@inproceedings{xie_synergy_2013,
 author = {Xie, Tao},
 booktitle = {2nd {International} {Workshop} on {Realizing} {Artificial} {Intelligence} {Synergies} in {Software} {Engineering}, {RAISE} 2013, {San} {Francisco}, {CA}, {USA}, {May} 25-26, 2013},
 doi = {10.1109/RAISE.2013.6615197},
 pages = {4--6},
 publisher = {IEEE Computer Society},
 title = {The synergy of human and artificial intelligence in software engineering},
 url = {https://doi.org/10.1109/RAISE.2013.6615197},
 year = {2013}
}
</rdfs:comment>
        <rdfs:label>xie_synergy_2013</rdfs:label>
        <rdfs:seeAlso rdf:resource="https://doi.org/10.1109/RAISE.2013.6615197"/>
    </owl:NamedIndividual>
    


    <!-- http://purl.org/ai4se/ontology#zhang_context-aware_2023 -->

    <owl:NamedIndividual rdf:about="http://purl.org/ai4se/ontology#zhang_context-aware_2023">
        <rdf:type rdf:resource="http://purl.org/ai4se/ontology#ResearchPaper"/>
        <hasLevel rdf:resource="http://purl.org/ai4se/ontology#null"/>
        <hasPurpose rdf:resource="http://purl.org/ai4se/ontology#null"/>
        <hasTarget rdf:resource="http://purl.org/ai4se/ontology#null"/>
        <hasType rdf:resource="http://purl.org/ai4se/ontology#null"/>
        <isAboutResearchTopic rdf:resource="http://purl.org/ai4se/ontology#CSO:Testing_and_debugging"/>
        <rdfs:comment>@article{zhang_context-aware_2023,
 author = {Zhang, Zhuo and Lei, Yan and Mao, Xiaoguang and Yan, Meng and Xia, Xin and Lo, David},
 copyright = {https://ieeexplore.ieee.org/Xplorehelp/downloads/license-information/IEEE.html},
 doi = {10.1109/TSE.2023.3279125},
 issn = {0098-5589, 1939-3520, 2326-3881},
 journal = {IEEE Transactions on Software Engineering},
 month = {July},
 number = {7},
 pages = {3939--3954},
 title = {Context-{Aware} {Neural} {Fault} {Localization}},
 url = {https://ieeexplore.ieee.org/document/10132088/},
 urldate = {2025-06-03},
 volume = {49},
 year = {2023}
}
</rdfs:comment>
        <rdfs:label>zhang_context-aware_2023</rdfs:label>
        <rdfs:seeAlso rdf:resource="https://ieeexplore.ieee.org/document/10132088/"/>
    </owl:NamedIndividual>
    


    <!-- http://purl.org/ai4se/ontology#zhang_survey_2024 -->

    <owl:NamedIndividual rdf:about="http://purl.org/ai4se/ontology#zhang_survey_2024">
        <rdf:type rdf:resource="http://purl.org/ai4se/ontology#ResearchPaper"/>
        <hasLevel rdf:resource="http://purl.org/ai4se/ontology#null"/>
        <hasPurpose rdf:resource="http://purl.org/ai4se/ontology#null"/>
        <hasTarget rdf:resource="http://purl.org/ai4se/ontology#null"/>
        <hasType rdf:resource="http://purl.org/ai4se/ontology#null"/>
        <isAboutResearchTopic rdf:resource="http://purl.org/ai4se/ontology#CSO:Testing_and_debugging"/>
        <rdfs:comment>@article{zhang_survey_2024,
 author = {Zhang, Quanjun and Fang, Chunrong and Ma, Yuxiang and Sun, Weisong and Chen, Zhenyu},
 doi = {10.1145/3631974},
  issn = {1049-331X, 1557-7392},
 journal = {ACM Transactions on Software Engineering and Methodology},
 language = {en},
 month = {February},
 number = {2},
 pages = {1--69},
 title = {A {Survey} of {Learning}-based {Automated} {Program} {Repair}},
 url = {https://dl.acm.org/doi/10.1145/3631974},
 urldate = {2025-06-02},
 volume = {33},
 year = {2024}
}
</rdfs:comment>
        <rdfs:label>zhang_survey_2024</rdfs:label>
        <rdfs:seeAlso rdf:resource="https://dl.acm.org/doi/10.1145/3631974"/>
    </owl:NamedIndividual>
    


    <!-- http://purl.org/ai4se/ontology#zhao_clustering-bayesian_2015 -->

    <owl:NamedIndividual rdf:about="http://purl.org/ai4se/ontology#zhao_clustering-bayesian_2015">
        <rdf:type rdf:resource="http://purl.org/ai4se/ontology#ResearchPaper"/>
        <hasLevel rdf:resource="http://purl.org/ai4se/ontology#AI-assisted_options"/>
        <hasPurpose rdf:resource="http://purl.org/ai4se/ontology#Improve"/>
        <hasTarget rdf:resource="http://purl.org/ai4se/ontology#Testing"/>
        <hasType rdf:resource="http://purl.org/ai4se/ontology#Statistical"/>
        <isAboutResearchTopic rdf:resource="http://purl.org/ai4se/ontology#CSO:Testing_and_debugging"/>
        <rdfs:comment>@inproceedings{zhao_clustering-bayesian_2015,
 author = {Zhao, Xiaobin and Wang, Zan and Fan, Xiangyu and Wang, Zhenhua},
 booktitle = {2015 {IEEE} 39th {Annual} {Computer} {Software} and {Applications} {Conference}},
 doi = {10.1109/COMPSAC.2015.154},
 pages = {542--547},
 publisher = {IEEE},
 title = {A clustering-{Bayesian} network based approach for test case prioritization},
 volume = {3},
 year = {2015}
}
</rdfs:comment>
        <rdfs:label>zhao_clustering-bayesian_2015</rdfs:label>
        <rdfs:seeAlso rdf:resource="https://doi.org/10.1109/COMPSAC.2015.154"/>
    </owl:NamedIndividual>
    


    <!-- http://purl.org/ai4se/ontology#CSO:Coding_technique -->

    <owl:NamedIndividual rdf:about="http://purl.org/ai4se/ontology#CSO:Coding_technique">
        <rdf:type rdf:resource="http://purl.org/ai4se/ontology#CSO:Topic"/>
    </owl:NamedIndividual>
    


    <!-- http://purl.org/ai4se/ontology#CSO:Deep_learning -->

    <owl:NamedIndividual rdf:about="http://purl.org/ai4se/ontology#CSO:Deep_learning">
        <rdf:type rdf:resource="http://purl.org/ai4se/ontology#CSO:Topic"/>
    </owl:NamedIndividual>
    


    <!-- http://purl.org/ai4se/ontology#CSO:DevOps -->

    <owl:NamedIndividual rdf:about="http://purl.org/ai4se/ontology#CSO:DevOps">
        <rdf:type rdf:resource="http://purl.org/ai4se/ontology#CSO:Topic"/>
    </owl:NamedIndividual>
    


    <!-- http://purl.org/ai4se/ontology#CSO:Requirements_engineering -->

    <owl:NamedIndividual rdf:about="http://purl.org/ai4se/ontology#CSO:Requirements_engineering">
        <rdf:type rdf:resource="http://purl.org/ai4se/ontology#CSO:Topic"/>
    </owl:NamedIndividual>
    


    <!-- http://purl.org/ai4se/ontology#CSO:Software_quality -->

    <owl:NamedIndividual rdf:about="http://purl.org/ai4se/ontology#CSO:Software_quality">
        <rdf:type rdf:resource="http://purl.org/ai4se/ontology#CSO:Topic"/>
    </owl:NamedIndividual>
    


    <!-- http://purl.org/ai4se/ontology#CSO:Software_traceability -->

    <owl:NamedIndividual rdf:about="http://purl.org/ai4se/ontology#CSO:Software_traceability">
        <rdf:type rdf:resource="http://purl.org/ai4se/ontology#CSO:Topic"/>
    </owl:NamedIndividual>
    


    <!-- http://purl.org/ai4se/ontology#CSO:Static_analysis -->

    <owl:NamedIndividual rdf:about="http://purl.org/ai4se/ontology#CSO:Static_analysis">
        <rdf:type rdf:resource="http://purl.org/ai4se/ontology#CSO:Topic"/>
    </owl:NamedIndividual>
    


    <!-- http://purl.org/ai4se/ontology#CSO:Testing_and_debugging -->

    <owl:NamedIndividual rdf:about="http://purl.org/ai4se/ontology#CSO:Testing_and_debugging">
        <rdf:type rdf:resource="http://purl.org/ai4se/ontology#CSO:Topic"/>
    </owl:NamedIndividual>
    


    <!-- http://purl.org/ai4se/ontology#CSO:Traceability_management -->

    <owl:NamedIndividual rdf:about="http://purl.org/ai4se/ontology#CSO:Traceability_management">
        <rdf:type rdf:resource="http://purl.org/ai4se/ontology#CSO:Topic"/>
    </owl:NamedIndividual>
</rdf:RDF>



<!-- Generated by the OWL API (version 4.5.29.2024-05-13T12:11:03Z) https://github.com/owlcs/owlapi -->

