<?xml version="1.0"?>
<rdf:RDF xmlns="http://purl.org/ai4se/owl#"
     xml:base="http://purl.org/ai4se/owl"
     xmlns:dc="http://purl.org/dc/elements/1.1/"
     xmlns:owl="http://www.w3.org/2002/07/owl#"
     xmlns:rdf="http://www.w3.org/1999/02/22-rdf-syntax-ns#"
     xmlns:xml="http://www.w3.org/XML/1998/namespace"
     xmlns:xsd="http://www.w3.org/2001/XMLSchema#"
     xmlns:gufo="http://purl.org/nemo/gufo#"
     xmlns:rdfs="http://www.w3.org/2000/01/rdf-schema#"
     xmlns:vann="http://purl.org/vocab/vann/"
     xmlns:ai4se="http://purl.org/ai4se/owl#"
     xmlns:terms="http://purl.org/dc/terms/"
     xmlns:papers="http://purl.org/ai4se/papers#">
    <owl:Ontology rdf:about="http://purl.org/ai4se/owl#">
        <owl:versionIRI rdf:resource="http://purl.org/ai4se/owl#/1.0.3"/>
        <dc:creator>Schieferdecker, Ina K.</dc:creator>
        <dc:title xml:lang="en">ai4se: The AI for SE taxonomy</dc:title>
        <terms:bibliographicCitation xml:lang="en">Schieferdecker, I.K.: &quot;ai4se: A taxonomy of research papers on the support of software engineering (SE) through the use of artificial intelligence (AI) methods and techniques&quot;, 2025, http://purl.org/ai4se/doc</terms:bibliographicCitation>
        <terms:license>https://creativecommons.org/licenses/by/4.0/legalcode.en</terms:license>
        <vann:preferredNamespacePrefix xml:lang="en">ai4se</vann:preferredNamespacePrefix>
        <vann:preferredNamespaceUri rdf:datatype="http://www.w3.org/2001/XMLSchema#anyURI">http://purl.org/ai4se/owl/</vann:preferredNamespaceUri>
        <rdfs:comment xml:lang="en">ai4se is a taxonomy for research papers on the use of artificial intelligence (AI) methods and techniques to support software engineering (SE).  It relates papers to their topics and contributions. These contributions are categorised by the purpose of the solution aimed for, the SE activity or process targeted, the type of AI used and the level of automation supported.</rdfs:comment>
        <owl:versionInfo rdf:datatype="http://www.w3.org/2001/XMLSchema#integer">3</owl:versionInfo>
    </owl:Ontology>
    


    <!-- 
    ///////////////////////////////////////////////////////////////////////////////////////
    //
    // Annotation properties
    //
    ///////////////////////////////////////////////////////////////////////////////////////
     -->

    


    <!-- http://purl.org/dc/elements/1.1/creator -->

    <owl:AnnotationProperty rdf:about="http://purl.org/dc/elements/1.1/creator"/>
    


    <!-- http://purl.org/dc/elements/1.1/title -->

    <owl:AnnotationProperty rdf:about="http://purl.org/dc/elements/1.1/title"/>
    


    <!-- http://purl.org/dc/terms/bibliographicCitation -->

    <owl:AnnotationProperty rdf:about="http://purl.org/dc/terms/bibliographicCitation"/>
    


    <!-- http://purl.org/dc/terms/license -->

    <owl:AnnotationProperty rdf:about="http://purl.org/dc/terms/license"/>
    


    <!-- http://purl.org/vocab/vann/preferredNamespacePrefix -->

    <owl:AnnotationProperty rdf:about="http://purl.org/vocab/vann/preferredNamespacePrefix"/>
    


    <!-- http://purl.org/vocab/vann/preferredNamespaceUri -->

    <owl:AnnotationProperty rdf:about="http://purl.org/vocab/vann/preferredNamespaceUri"/>
    


    <!-- 
    ///////////////////////////////////////////////////////////////////////////////////////
    //
    // Object Properties
    //
    ///////////////////////////////////////////////////////////////////////////////////////
     -->

    


    <!-- http://purl.org/ai4se/owl#hasClassification -->

    <owl:ObjectProperty rdf:about="http://purl.org/ai4se/owl#hasClassification">
        <rdfs:subPropertyOf rdf:resource="http://www.w3.org/2002/07/owl#topObjectProperty"/>
        <rdf:type rdf:resource="http://www.w3.org/2002/07/owl#AsymmetricProperty"/>
        <rdf:type rdf:resource="http://www.w3.org/2002/07/owl#IrreflexiveProperty"/>
        <rdfs:domain rdf:resource="http://purl.org/ai4se/owl#Research_contribution"/>
        <rdfs:range rdf:resource="http://purl.org/ai4se/owl#Taxonomy"/>
        <rdfs:comment xml:lang="en">A general property to link a research contribution to its classification values across different dimensions (e.g., Solution purpose, Solution target, AI type, Automation level).</rdfs:comment>
        <rdfs:label xml:lang="en">has classification</rdfs:label>
    </owl:ObjectProperty>
    


    <!-- http://purl.org/ai4se/owl#isAboutResearchTopic -->

    <owl:ObjectProperty rdf:about="http://purl.org/ai4se/owl#isAboutResearchTopic">
        <rdfs:subPropertyOf rdf:resource="http://www.w3.org/2002/07/owl#topObjectProperty"/>
        <rdf:type rdf:resource="http://www.w3.org/2002/07/owl#AsymmetricProperty"/>
        <rdf:type rdf:resource="http://www.w3.org/2002/07/owl#IrreflexiveProperty"/>
        <rdfs:domain rdf:resource="http://purl.org/ai4se/owl#Research_paper"/>
        <rdfs:range rdf:resource="http://purl.org/ai4se/owl#CSO:Topic"/>
        <rdfs:comment xml:lang="en">Property to link a research paper to its research topic(s).</rdfs:comment>
        <rdfs:label>isAboutResearchTopic</rdfs:label>
    </owl:ObjectProperty>
    


    <!-- http://purl.org/ai4se/owl#isInResearchCollection -->

    <owl:ObjectProperty rdf:about="http://purl.org/ai4se/owl#isInResearchCollection">
        <rdfs:subPropertyOf rdf:resource="http://www.w3.org/2002/07/owl#topObjectProperty"/>
        <rdf:type rdf:resource="http://www.w3.org/2002/07/owl#AsymmetricProperty"/>
        <rdf:type rdf:resource="http://www.w3.org/2002/07/owl#IrreflexiveProperty"/>
        <rdfs:domain rdf:resource="http://purl.org/ai4se/owl#Research_paper"/>
        <rdfs:range rdf:resource="http://purl.org/ai4se/owl#Research_paper_collection"/>
        <rdfs:comment xml:lang="en">Represents the membership of a research paper or research paper collection to a research paper collection.</rdfs:comment>
        <rdfs:label>isInResearchCollection</rdfs:label>
    </owl:ObjectProperty>
    


    <!-- http://purl.org/ai4se/papers#belongsToAIType -->

    <owl:ObjectProperty rdf:about="http://purl.org/ai4se/papers#belongsToAIType">
        <rdfs:subPropertyOf rdf:resource="http://www.w3.org/2002/07/owl#topObjectProperty"/>
        <rdf:type rdf:resource="http://www.w3.org/2002/07/owl#TransitiveProperty"/>
        <rdfs:domain rdf:resource="http://purl.org/ai4se/owl#AI_Type"/>
        <rdfs:range rdf:resource="http://purl.org/ai4se/owl#AI_Type"/>
        <rdfs:comment xml:lang="en">Property to group AI types.</rdfs:comment>
        <rdfs:label>belongsToAIType</rdfs:label>
    </owl:ObjectProperty>
    


    <!-- http://purl.org/ai4se/papers#belongsToSEActivity -->

    <owl:ObjectProperty rdf:about="http://purl.org/ai4se/papers#belongsToSEActivity">
        <rdfs:subPropertyOf rdf:resource="http://www.w3.org/2002/07/owl#topObjectProperty"/>
        <rdf:type rdf:resource="http://www.w3.org/2002/07/owl#TransitiveProperty"/>
        <rdfs:domain rdf:resource="http://purl.org/ai4se/papers#SE_target"/>
        <rdfs:range rdf:resource="http://purl.org/ai4se/papers#SE_target"/>
        <rdfs:comment xml:lang="en">Property to group SE activities/processes.</rdfs:comment>
        <rdfs:label>belongsToSEActivity</rdfs:label>
    </owl:ObjectProperty>
    


    <!-- http://purl.org/ai4se/papers#hasClassificationAIType -->

    <owl:ObjectProperty rdf:about="http://purl.org/ai4se/papers#hasClassificationAIType">
        <rdfs:subPropertyOf rdf:resource="http://purl.org/ai4se/owl#hasClassification"/>
        <rdf:type rdf:resource="http://www.w3.org/2002/07/owl#AsymmetricProperty"/>
        <rdf:type rdf:resource="http://www.w3.org/2002/07/owl#IrreflexiveProperty"/>
        <rdfs:domain rdf:resource="http://purl.org/ai4se/owl#Research_contribution"/>
        <rdfs:range rdf:resource="http://purl.org/ai4se/owl#AI_Type"/>
        <rdfs:comment>Property to link a research contribution to the AI type(s) being used.</rdfs:comment>
        <rdfs:label>hasClassificationAIType</rdfs:label>
    </owl:ObjectProperty>
    


    <!-- http://purl.org/ai4se/papers#hasClassificationAutomationLevel -->

    <owl:ObjectProperty rdf:about="http://purl.org/ai4se/papers#hasClassificationAutomationLevel">
        <rdfs:subPropertyOf rdf:resource="http://purl.org/ai4se/owl#hasClassification"/>
        <rdf:type rdf:resource="http://www.w3.org/2002/07/owl#AsymmetricProperty"/>
        <rdf:type rdf:resource="http://www.w3.org/2002/07/owl#IrreflexiveProperty"/>
        <rdfs:domain rdf:resource="http://purl.org/ai4se/owl#Research_contribution"/>
        <rdfs:range rdf:resource="http://purl.org/ai4se/owl#Automation_level"/>
        <rdfs:comment xml:lang="en">Property to link a research contribution to the automation level(s) being supported.</rdfs:comment>
        <rdfs:label>hasClassificationAutomationLevel</rdfs:label>
    </owl:ObjectProperty>
    


    <!-- http://purl.org/ai4se/papers#hasClassificationSolutionPurpose -->

    <owl:ObjectProperty rdf:about="http://purl.org/ai4se/papers#hasClassificationSolutionPurpose">
        <rdfs:subPropertyOf rdf:resource="http://purl.org/ai4se/owl#hasClassification"/>
        <rdf:type rdf:resource="http://www.w3.org/2002/07/owl#AsymmetricProperty"/>
        <rdf:type rdf:resource="http://www.w3.org/2002/07/owl#IrreflexiveProperty"/>
        <rdfs:domain rdf:resource="http://purl.org/ai4se/owl#Research_contribution"/>
        <rdfs:range rdf:resource="http://purl.org/ai4se/owl#Solution_purpose"/>
        <rdfs:comment xml:lang="en">Property to link a research contribution to the solution purpose(s) being aimed at.</rdfs:comment>
        <rdfs:label>hasClassificationSolutionPurpose</rdfs:label>
    </owl:ObjectProperty>
    


    <!-- http://purl.org/ai4se/papers#hasClassificationSolutionTarget -->

    <owl:ObjectProperty rdf:about="http://purl.org/ai4se/papers#hasClassificationSolutionTarget">
        <rdfs:subPropertyOf rdf:resource="http://purl.org/ai4se/owl#hasClassification"/>
        <rdf:type rdf:resource="http://www.w3.org/2002/07/owl#AsymmetricProperty"/>
        <rdf:type rdf:resource="http://www.w3.org/2002/07/owl#IrreflexiveProperty"/>
        <rdfs:domain rdf:resource="http://purl.org/ai4se/owl#Research_contribution"/>
        <rdfs:range rdf:resource="http://purl.org/ai4se/papers#SE_target"/>
        <rdfs:comment xml:lang="en">Property to link a research contribution to the SE activities/processes being addressed.</rdfs:comment>
        <rdfs:label>hasClassificationSolutionTarget</rdfs:label>
    </owl:ObjectProperty>
    


    <!-- http://purl.org/ai4se/papers#hasContribution -->

    <owl:ObjectProperty rdf:about="http://purl.org/ai4se/papers#hasContribution">
        <rdfs:subPropertyOf rdf:resource="http://www.w3.org/2002/07/owl#topObjectProperty"/>
        <rdf:type rdf:resource="http://www.w3.org/2002/07/owl#InverseFunctionalProperty"/>
        <rdf:type rdf:resource="http://www.w3.org/2002/07/owl#IrreflexiveProperty"/>
        <rdfs:domain rdf:resource="http://purl.org/ai4se/owl#Research_paper"/>
        <rdfs:range rdf:resource="http://purl.org/ai4se/owl#Research_contribution"/>
        <rdfs:comment xml:lang="en">Property to link a research paper to its research contribution(s).</rdfs:comment>
        <rdfs:label>hasContribution</rdfs:label>
    </owl:ObjectProperty>
    


    <!-- http://purl.org/ai4se/papers#usesModel -->

    <owl:ObjectProperty rdf:about="http://purl.org/ai4se/papers#usesModel">
        <rdfs:domain rdf:resource="http://purl.org/ai4se/papers#SE_target"/>
        <rdfs:range rdf:resource="http://purl.org/ai4se/owl#Model"/>
        <rdfs:comment xml:lang="en">Property to link SE activities/processes to models being used, in particular in Model-Driven Software Engineering (MDSE).</rdfs:comment>
        <rdfs:label>usesModel</rdfs:label>
    </owl:ObjectProperty>
    


    <!-- 
    ///////////////////////////////////////////////////////////////////////////////////////
    //
    // Classes
    //
    ///////////////////////////////////////////////////////////////////////////////////////
     -->

    


    <!-- http://purl.org/ai4se/owl#AI_Type -->

    <owl:Class rdf:about="http://purl.org/ai4se/owl#AI_Type">
        <rdfs:subClassOf rdf:resource="http://purl.org/ai4se/owl#Taxonomy"/>
        <owl:disjointWith rdf:resource="http://purl.org/ai4se/owl#Automation_level"/>
        <owl:disjointWith rdf:resource="http://purl.org/ai4se/owl#Solution_purpose"/>
        <rdfs:comment xml:lang="en">Represents the type of the artificial intelligence (AI) system being used.

According to ISO/IEC 22989:2022 Information technology - Artificial intelligence - Artificial intelligence concepts and terminology, artificial intelligence (AI) is

- &lt;discipline&gt; research and development of mechanisms and applications of AI systems.

and

artificial intelligence system (AI system) is

- engineered system that generates outputs such as content, forecasts, recommendations or decisions for a given set of human-defined objectives.</rdfs:comment>
        <rdfs:label>Type of AI system</rdfs:label>
    </owl:Class>
    


    <!-- http://purl.org/ai4se/owl#Automation_level -->

    <owl:Class rdf:about="http://purl.org/ai4se/owl#Automation_level">
        <rdfs:subClassOf rdf:resource="http://purl.org/ai4se/owl#Taxonomy"/>
        <owl:disjointWith rdf:resource="http://purl.org/ai4se/owl#Solution_purpose"/>
        <rdfs:comment xml:lang="en">Represents the level of automation provided / enabled by the AI system being used.

According to ISO/IEC 22989:2022 Information technology - Artificial intelligence - Artificial intelligence concepts and terminology, artificial intelligence (AI) is

- &lt;discipline&gt; research and development of mechanisms and applications of AI systems.

and

artificial intelligence system (AI system) is

- engineered system that generates outputs such as content, forecasts, recommendations or decisions for a given set of human-defined objectives.</rdfs:comment>
        <rdfs:label>Level of AI automation</rdfs:label>
    </owl:Class>
    


    <!-- http://purl.org/ai4se/owl#Model -->

    <owl:Class rdf:about="http://purl.org/ai4se/owl#Model">
        <rdfs:comment xml:lang="en">Represents artifacts defining (semi-)formally (1) properties of one or more artefacts used by software engineering activities or processes or (2) properties of software engineering activities or processes.

According to ISO/IEC 22989:2022 Information technology - Artificial intelligence - Artificial intelligence concepts and terminology, model is

- physical, mathematical or otherwise logical representation of a system, entity, phenomenon, process or data.

Note: For the AI4SE ontology, only mathematical or logical representations are relevant.</rdfs:comment>
        <rdfs:label>Model</rdfs:label>
    </owl:Class>
    


    <!-- http://purl.org/ai4se/owl#Model-Driven_Software_Engineering -->

    <owl:Class rdf:about="http://purl.org/ai4se/owl#Model-Driven_Software_Engineering">
        <rdfs:subClassOf rdf:resource="http://purl.org/ai4se/papers#SE_target"/>
        <rdfs:comment xml:lang="en">Relates software activities and processes to models used for model-driven software engineering.

Model-driven software engineering (MDSE) refers to software engineering methodologies that focus on creating and exploiting (domain-specific) models. These are conceptual models that describe various aspects of software, its components and/or environment, and the processes and/or activities used to develop and operate it. Rather than just focusing on programming and code, MDSE emphasises the use of models as the primary artefacts in software engineering processes.</rdfs:comment>
        <rdfs:label>Model-Driven Software Engineering</rdfs:label>
    </owl:Class>
    


    <!-- http://purl.org/ai4se/owl#Research_contribution -->

    <owl:Class rdf:about="http://purl.org/ai4se/owl#Research_contribution">
        <rdfs:comment xml:lang="en">Represents the specific research contribution(s) made by a specific research paper.</rdfs:comment>
        <rdfs:label>Research contribution</rdfs:label>
    </owl:Class>
    


    <!-- http://purl.org/ai4se/owl#Research_paper -->

    <owl:Class rdf:about="http://purl.org/ai4se/owl#Research_paper">
        <rdfs:comment xml:lang="en">Represents an artefact that documents research findings, such as new insights, methods or techniques. It has been reviewed, published and is digitally accessible.</rdfs:comment>
        <rdfs:label>Research paper</rdfs:label>
    </owl:Class>
    


    <!-- http://purl.org/ai4se/owl#Research_paper_collection -->

    <owl:Class rdf:about="http://purl.org/ai4se/owl#Research_paper_collection">
        <rdfs:comment xml:lang="en">A collection of research papers contributing to the body of knowledge in a given field, for a research topic, research question(s) or a given problem statement.</rdfs:comment>
        <rdfs:label>Research paper collection</rdfs:label>
    </owl:Class>
    


    <!-- http://purl.org/ai4se/owl#Solution_purpose -->

    <owl:Class rdf:about="http://purl.org/ai4se/owl#Solution_purpose">
        <rdfs:subClassOf rdf:resource="http://purl.org/ai4se/owl#Taxonomy"/>
        <rdfs:comment xml:lang="en">Represents the purpose of using the AI system in a software development / operation processes or activities.</rdfs:comment>
        <rdfs:label>Solution purpose</rdfs:label>
    </owl:Class>
    


    <!-- http://purl.org/ai4se/owl#Taxonomy -->

    <owl:Class rdf:about="http://purl.org/ai4se/owl#Taxonomy">
        <rdfs:comment xml:lang="en">The superclass for all specific values used to classify the qualities of research contributions, such as &apos;Symbolic AI&apos; or &apos;Generate&apos;. As a subclass of gufo:QualityValue, it represents a value within a certain quality space (e.g., AI type, automation level, solution purpose).</rdfs:comment>
        <rdfs:label xml:lang="en">Classification Value</rdfs:label>
    </owl:Class>
    


    <!-- http://purl.org/ai4se/owl#CSO:Topic -->

    <owl:Class rdf:about="http://purl.org/ai4se/owl#CSO:Topic">
        <rdfs:comment xml:lang="en">Represents the research topics in Computer Science as defined by the Computer Science Ontology CSO.</rdfs:comment>
        <rdfs:label>CSO:Topic</rdfs:label>
        <rdfs:seeAlso>https://cso.kmi.open.ac.uk/</rdfs:seeAlso>
    </owl:Class>
    


    <!-- http://purl.org/ai4se/owl#PrMO:Activity -->

    <owl:Class rdf:about="http://purl.org/ai4se/owl#PrMO:Activity">
        <rdfs:comment xml:lang="en">Represents a set of tasks used to produce, operate or maintain software-based products or services as well as to achieve the objectives of the process it belongs to. The activity includes the procedures, standards, policies, and objectives to create and modify a set of work products. 

Adapted to software-related activities from PrMO: an ontology of process-reference models.</rdfs:comment>
        <rdfs:label>PrMO:Activity</rdfs:label>
        <rdfs:seeAlso>https://www.redalyc.org/articulo.oa?id=43032606003</rdfs:seeAlso>
    </owl:Class>
    


    <!-- http://purl.org/ai4se/owl#PrMO:Process -->

    <owl:Class rdf:about="http://purl.org/ai4se/owl#PrMO:Process">
        <rdfs:subClassOf rdf:resource="http://purl.org/ai4se/owl#PrMO:Activity"/>
        <rdfs:comment xml:lang="en">Represents a coherent set of policies, organizational structures, technologies; procedures, purposes, objectives, and work products that are needed to design, develop, deploy and maintain a software product.

Defined by PrMO: an ontology of process-reference models</rdfs:comment>
        <rdfs:label>PrMO:Process</rdfs:label>
        <rdfs:seeAlso>https://www.redalyc.org/articulo.oa?id=43032606003</rdfs:seeAlso>
    </owl:Class>
    


    <!-- http://purl.org/ai4se/papers#SE_target -->

    <owl:Class rdf:about="http://purl.org/ai4se/papers#SE_target">
        <rdfs:subClassOf rdf:resource="http://purl.org/ai4se/owl#Taxonomy"/>
        <rdfs:subClassOf rdf:resource="http://purl.org/ai4se/owl#PrMO:Activity"/>
        <rdfs:subClassOf rdf:resource="http://purl.org/ai4se/owl#PrMO:Process"/>
        <rdfs:comment xml:lang="en">Represents the primary software engineering process or activitiy being addressed.

According to  ISO/IEC/IEEE 24765: Systems and software engineering - Vocabulary, software engineering is

1. systematic application of scientific and technological knowledge, methods, and experience to the design, implementation, testing, and documentation of software.

2. application of a systematic, disciplined, quantifiable approach to the development, operation, and maintenance of software; that is, the application of engineering to software.</rdfs:comment>
        <rdfs:label>Software Engineering target</rdfs:label>
        <rdfs:seeAlso>https://www.computer.org/education/bodies-of-knowledge/software-engineering</rdfs:seeAlso>
    </owl:Class>
    


    <!-- 
    ///////////////////////////////////////////////////////////////////////////////////////
    //
    // Individuals
    //
    ///////////////////////////////////////////////////////////////////////////////////////
     -->

    


    <!-- http://purl.org/ai4se/owl#AI-assisted_options -->

    <owl:NamedIndividual rdf:about="http://purl.org/ai4se/owl#AI-assisted_options">
        <rdf:type rdf:resource="http://purl.org/ai4se/owl#Automation_level"/>
        <rdfs:comment xml:lang="en">Represents the case in which choices, recommendations, or decision-support outputs for the target SE processes or activities are generated or enhanced by an AI system, while retaining human control over the final choice, recommendation or decision, which may differ from the AI outputs.</rdfs:comment>
        <rdfs:label>AI-assisted options</rdfs:label>
    </owl:NamedIndividual>
    


    <!-- http://purl.org/ai4se/owl#AI-assisted_selection -->

    <owl:NamedIndividual rdf:about="http://purl.org/ai4se/owl#AI-assisted_selection">
        <rdf:type rdf:resource="http://purl.org/ai4se/owl#Automation_level"/>
        <rdfs:comment xml:lang="en">Represents the case in which choices, recommendations, or decision-support outputs for the target SE processes or activities are generated or enhanced by an AI system, where the final choices, recommendations or decisions require human confirmation and do not differ from the AI outputs.</rdfs:comment>
        <rdfs:label>AI-assisted selection</rdfs:label>
    </owl:NamedIndividual>
    


    <!-- http://purl.org/ai4se/owl#AI-driven_full_automation -->

    <owl:NamedIndividual rdf:about="http://purl.org/ai4se/owl#AI-driven_full_automation">
        <rdf:type rdf:resource="http://purl.org/ai4se/owl#Automation_level"/>
        <rdfs:comment xml:lang="en">Represents the case in which AI is used to automate all tasks or decision-making components within the target SE processes or activities, without requiring human intervention.</rdfs:comment>
        <rdfs:label>AI-driven full automation</rdfs:label>
    </owl:NamedIndividual>
    


    <!-- http://purl.org/ai4se/owl#AI-driven_partial_automation -->

    <owl:NamedIndividual rdf:about="http://purl.org/ai4se/owl#AI-driven_partial_automation">
        <rdf:type rdf:resource="http://purl.org/ai4se/owl#Automation_level"/>
        <rdfs:comment xml:lang="en">Represents the case in which AI is used to automate specific tasks or decision-making components within the target SE processes or activities, while other parts of the process remain under human control or require human intervention.</rdfs:comment>
        <rdfs:label>AI-driven partial automation</rdfs:label>
    </owl:NamedIndividual>
    


    <!-- http://purl.org/ai4se/owl#Agentic_AI -->

    <owl:NamedIndividual rdf:about="http://purl.org/ai4se/owl#Agentic_AI">
        <rdf:type rdf:resource="http://purl.org/ai4se/owl#AI_Type"/>
        <rdfs:comment xml:lang="en">Represents AI systems that rely on autonomous agents using AI techniques to plan, adapt, and execute multi-step objectives with minimal human control.</rdfs:comment>
        <rdfs:label>Agentic AI</rdfs:label>
    </owl:NamedIndividual>
    


    <!-- http://purl.org/ai4se/owl#Architecture_and_design -->

    <owl:NamedIndividual rdf:about="http://purl.org/ai4se/owl#Architecture_and_design">
        <rdf:type rdf:resource="http://purl.org/ai4se/papers#SE_target"/>
        <papers:belongsToSEActivity rdf:resource="http://purl.org/ai4se/owl#Develop"/>
        <rdfs:comment xml:lang="en">Represents software architecture and design activities and processes. 

A software architecture defines its fundamental organization, its components, their relationships, and the principles guiding its design and evolution. 
 
According to ISO/IEC/IEEE 42010:2022: Software, systems and enterprise - Architecture description), a software architecture consists of the fundamental concepts or properties of an entity in its environment and governing principles for the realization and evolution of this entity and its related life cycle processes.

Software design is the process of defining the architecture, components, interfaces, and other characteristics of a software or a component.

According to ISO/IEC/IEEE 24765: Systems and software engineering - Vocabulary, software design is  

1. the use of scientific principles, technical information, and imagination in the definition of a software system to perform pre-specified functions with maximum economy and efficiency.</rdfs:comment>
        <rdfs:label>Software architecture and design</rdfs:label>
    </owl:NamedIndividual>
    


    <!-- http://purl.org/ai4se/owl#Classical_machine_learning -->

    <owl:NamedIndividual rdf:about="http://purl.org/ai4se/owl#Classical_machine_learning">
        <rdf:type rdf:resource="http://purl.org/ai4se/owl#AI_Type"/>
        <papers:belongsToAIType rdf:resource="http://purl.org/ai4se/owl#Subsymbolic"/>
        <rdfs:comment xml:lang="en">Represents subsymbolic AI systems that rely on statistical and algorithmic learning techniques - such as decision trees, support vector machines, linear regression, and clustering - to learn patterns from structured data and make predictions or classifications. These models typically operate on explicitly defined features and do not involve deep neural networks.

This class of AI is used in contrast to deep learning AI.</rdfs:comment>
        <rdfs:label>Classical machine learning</rdfs:label>
    </owl:NamedIndividual>
    


    <!-- http://purl.org/ai4se/owl#Coding -->

    <owl:NamedIndividual rdf:about="http://purl.org/ai4se/owl#Coding">
        <rdf:type rdf:resource="http://purl.org/ai4se/papers#SE_target"/>
        <papers:belongsToSEActivity rdf:resource="http://purl.org/ai4se/owl#Develop"/>
        <rdfs:comment xml:lang="en">Represents coding activities and processes. 

Coding (also known as programming) is the process of transforming the design of a software or a component into an executable computer program.

According to ISO/IEC/IEEE 24765: Systems and software engineering - Vocabulary, coding is

1. in software engineering, the process of expressing a computer program in a programming language

2. transforming of logic and data from design specifications (design descriptions) into a programming language.</rdfs:comment>
        <rdfs:label>Software coding</rdfs:label>
    </owl:NamedIndividual>
    


    <!-- http://purl.org/ai4se/owl#Deep_learning -->

    <owl:NamedIndividual rdf:about="http://purl.org/ai4se/owl#Deep_learning">
        <rdf:type rdf:resource="http://purl.org/ai4se/owl#AI_Type"/>
        <papers:belongsToAIType rdf:resource="http://purl.org/ai4se/owl#Subsymbolic"/>
        <rdfs:comment xml:lang="en">Represents subsymbolic AI systems that rely on deep artificial neural networks to automatically learn features and perform tasks such as classification or prediction, especially from large and complex datasets. 

According to ISO/IEC 22989:2022 Information technology - Artificial intelligence - Artificial intelligence concepts and terminology, deep learning (deep neural network learning) is

- AI approach to creating rich hierarchical representations through the training of neural networks with many hidden layers.</rdfs:comment>
        <rdfs:label>Deep learning AI</rdfs:label>
    </owl:NamedIndividual>
    


    <!-- http://purl.org/ai4se/owl#Deployment -->

    <owl:NamedIndividual rdf:about="http://purl.org/ai4se/owl#Deployment">
        <rdf:type rdf:resource="http://purl.org/ai4se/papers#SE_target"/>
        <papers:belongsToSEActivity rdf:resource="http://purl.org/ai4se/owl#Operate"/>
        <rdfs:comment xml:lang="en">Represents software deployment activities and processes.

Software deployment encompasses the processes and activities for placing a software or component into an operational environment.

According to ISO/IEC/IEEE 24765: Systems and software engineering - Vocabulary, deployment is 

1. a phase of a project in which a system is put into operation and cutover issues are resolved.</rdfs:comment>
        <rdfs:label>Software deployment</rdfs:label>
    </owl:NamedIndividual>
    


    <!-- http://purl.org/ai4se/owl#Develop -->

    <owl:NamedIndividual rdf:about="http://purl.org/ai4se/owl#Develop">
        <rdf:type rdf:resource="http://purl.org/ai4se/papers#SE_target"/>
        <rdfs:comment xml:lang="en">Represents software development activities and processes.

Software development is the set of activities that result in software products, including requirements analysis, design, coding, testing, and maintenance. It encompasses all the activities and processes involved in creating, implementing, and modifying software (artefacts), as well as ensuring that it satisfies stakeholder requirements throughout the software development life cycle.</rdfs:comment>
        <rdfs:label>Develop</rdfs:label>
    </owl:NamedIndividual>
    


    <!-- http://purl.org/ai4se/owl#General_AI -->

    <owl:NamedIndividual rdf:about="http://purl.org/ai4se/owl#General_AI">
        <rdf:type rdf:resource="http://purl.org/ai4se/owl#AI_Type"/>
        <rdfs:comment xml:lang="en">Represents AI systems capable of performing a broad set of distinct tasks with satisfactory performance.

According to ISO/IEC 22989:2022 Information technology - Artificial intelligence - Artificial intelligence concepts and terminology, general AI (AGI, artificial general intelligence)

- type of AI system that addresses a broad range of tasks with a satisfactory level of performance 

Note 1: Compared to narrow AI.
Note 2: AGI is often used in a stronger sense, meaning systems that not only can perform a wide variety of tasks, but all tasks that a human can perform.</rdfs:comment>
        <rdfs:label>General AI</rdfs:label>
    </owl:NamedIndividual>
    


    <!-- http://purl.org/ai4se/owl#Generate -->

    <owl:NamedIndividual rdf:about="http://purl.org/ai4se/owl#Generate">
        <rdf:type rdf:resource="http://purl.org/ai4se/owl#Solution_purpose"/>
        <rdfs:comment xml:lang="en">The purpose of using AI is to generate (parts of) artefacts used in software engineering.</rdfs:comment>
        <rdfs:label>Generate</rdfs:label>
    </owl:NamedIndividual>
    


    <!-- http://purl.org/ai4se/owl#Generative_AI -->

    <owl:NamedIndividual rdf:about="http://purl.org/ai4se/owl#Generative_AI">
        <rdf:type rdf:resource="http://purl.org/ai4se/owl#AI_Type"/>
        <rdfs:comment xml:lang="en">Represents AI systems that use learned or derived knowledge to produce original outputs, such as synthetic text, media, or other content types. It often uses subsymbolic AI like Convolutional Neural Networks (CNNs), Recurrent Neural Networks (RNNs), or Transformer-based models, but also symbolic AI.</rdfs:comment>
        <rdfs:label>Generative AI</rdfs:label>
    </owl:NamedIndividual>
    


    <!-- http://purl.org/ai4se/owl#Improve -->

    <owl:NamedIndividual rdf:about="http://purl.org/ai4se/owl#Improve">
        <rdf:type rdf:resource="http://purl.org/ai4se/owl#Solution_purpose"/>
        <rdfs:comment xml:lang="en">The purpose of using AI is to improve (parts of) artefacts used in software engineering.</rdfs:comment>
        <rdfs:label>Improve</rdfs:label>
    </owl:NamedIndividual>
    


    <!-- http://purl.org/ai4se/owl#Improvement -->

    <owl:NamedIndividual rdf:about="http://purl.org/ai4se/owl#Improvement">
        <rdf:type rdf:resource="http://purl.org/ai4se/papers#SE_target"/>
        <papers:belongsToSEActivity rdf:resource="http://purl.org/ai4se/owl#Process"/>
        <rdfs:comment xml:lang="en">Represents software engineering process improvement activities and processes.

Process improvement is undertaken to provide enhancements to the software life cycle processes and activities to improve their performance and / or outcomes.

According to ISO/IEC/IEEE 12207:2017: Systems and software engineering - Software life cycle processes, process improvement consists of the following tasks:

1) Prioritize and plan improvement opportunities.

2) Implement improvement opportunities and inform relevant stakeholders.

3) Lessons learned are captured and made available.</rdfs:comment>
        <rdfs:label>Process improvement</rdfs:label>
    </owl:NamedIndividual>
    


    <!-- http://purl.org/ai4se/owl#Maintenance -->

    <owl:NamedIndividual rdf:about="http://purl.org/ai4se/owl#Maintenance">
        <rdf:type rdf:resource="http://purl.org/ai4se/papers#SE_target"/>
        <papers:belongsToSEActivity rdf:resource="http://purl.org/ai4se/owl#Develop"/>
        <rdfs:comment xml:lang="en">Represents software maintenance activities and processes. 

Software maintenance is the process of modifying a software or component after delivery to correct faults, improve performance or other attributes, or adapt to a changed environment.

According to ISO/IEC/IEEE 24765: Systems and software engineering - Vocabulary, software maintenance is 

1. totality of activities required to provide cost-effective support to a software system 

2. entitlement of additional rights (such as additional
functionality, upgrade or support) for a previously granted software entitlement</rdfs:comment>
        <rdfs:label>Software maintenance</rdfs:label>
    </owl:NamedIndividual>
    


    <!-- http://purl.org/ai4se/owl#Management -->

    <owl:NamedIndividual rdf:about="http://purl.org/ai4se/owl#Management">
        <rdf:type rdf:resource="http://purl.org/ai4se/papers#SE_target"/>
        <papers:belongsToSEActivity rdf:resource="http://purl.org/ai4se/owl#Process"/>
        <rdfs:comment xml:lang="en">Represents software management activities and processes.

Software management consists of processes that plan, monitor and control the development and maintenance of software throughout its lifecycle. This ensures that software-related activities are conducted systematically and can be quantified.

According to ISO/IEC/IEEE 24765: Systems and software engineering - Vocabulary, management processes are

1. activities that are undertaken in order to ensure that the software engineering processes are performed in a manner consistent with the organization&apos;s policies, goals, and standards.</rdfs:comment>
        <rdfs:label>Process management</rdfs:label>
    </owl:NamedIndividual>
    


    <!-- http://purl.org/ai4se/owl#Monitoring -->

    <owl:NamedIndividual rdf:about="http://purl.org/ai4se/owl#Monitoring">
        <rdf:type rdf:resource="http://purl.org/ai4se/papers#SE_target"/>
        <papers:belongsToSEActivity rdf:resource="http://purl.org/ai4se/owl#Operate"/>
        <rdfs:comment xml:lang="en">Represents software monitoring activities and processes.

Software monitoring is systematically observing, checking, or keeping track of the operations or performance of a software or component.</rdfs:comment>
        <rdfs:label>Software monitoring</rdfs:label>
    </owl:NamedIndividual>
    


    <!-- http://purl.org/ai4se/owl#No_AI_support -->

    <owl:NamedIndividual rdf:about="http://purl.org/ai4se/owl#No_AI_support">
        <rdf:type rdf:resource="http://purl.org/ai4se/owl#Automation_level"/>
        <rdfs:comment xml:lang="en">Represents the case in which the target SE processes or activities are performed without the assistance of AI.</rdfs:comment>
        <rdfs:label>No AI-supported automation</rdfs:label>
    </owl:NamedIndividual>
    


    <!-- http://purl.org/ai4se/owl#Operate -->

    <owl:NamedIndividual rdf:about="http://purl.org/ai4se/owl#Operate">
        <rdf:type rdf:resource="http://purl.org/ai4se/papers#SE_target"/>
        <rdfs:comment xml:lang="en">Represents software operation activities and processs.</rdfs:comment>
        <rdfs:label>Operate</rdfs:label>
    </owl:NamedIndividual>
    


    <!-- http://purl.org/ai4se/owl#Operation -->

    <owl:NamedIndividual rdf:about="http://purl.org/ai4se/owl#Operation">
        <rdf:type rdf:resource="http://purl.org/ai4se/papers#SE_target"/>
        <papers:belongsToSEActivity rdf:resource="http://purl.org/ai4se/owl#Operate"/>
        <rdfs:comment xml:lang="en">Represents software operation activities and processes.

Software operation refers to

1. The use and execution of software in its production environment to perform its intended functions.

2. Running a software to deliver services or perform tasks for users or other systems.</rdfs:comment>
        <rdfs:label>Software operation</rdfs:label>
    </owl:NamedIndividual>
    


    <!-- http://purl.org/ai4se/owl#Process -->

    <owl:NamedIndividual rdf:about="http://purl.org/ai4se/owl#Process">
        <rdf:type rdf:resource="http://purl.org/ai4se/papers#SE_target"/>
        <rdfs:comment xml:lang="en">Represents processes for software engineering along the software lifecycle of software development and operation.</rdfs:comment>
        <rdfs:label>Software Engineering Processes</rdfs:label>
    </owl:NamedIndividual>
    


    <!-- http://purl.org/ai4se/owl#Requirements -->

    <owl:NamedIndividual rdf:about="http://purl.org/ai4se/owl#Requirements">
        <rdf:type rdf:resource="http://purl.org/ai4se/papers#SE_target"/>
        <papers:belongsToSEActivity rdf:resource="http://purl.org/ai4se/owl#Develop"/>
        <rdfs:comment xml:lang="en">Represents requirements engineering activities and processes. 

A software requirement is a condition or capability that must be met by a software or component.

According to ISO/IEC/IEEE 24765: Systems and software engineering - Vocabulary, software requirement is

1. software capability needed by a user to solve a problem or to achieve an objective

2. software capability that must be met or possessed by a system or system component to satisfy a contract, standard, specification, or other formally imposed document

According to ISO/IEC/IEEE 24765: Systems and software engineering - Vocabulary, software requirements engineering is

1. science and discipline concerned with analyzing and documenting software requirements 

2. software requirements elicitation, analysis, specification, verification, and management</rdfs:comment>
        <rdfs:label>Requirements engineering</rdfs:label>
    </owl:NamedIndividual>
    


    <!-- http://purl.org/ai4se/owl#Statistical -->

    <owl:NamedIndividual rdf:about="http://purl.org/ai4se/owl#Statistical">
        <rdf:type rdf:resource="http://purl.org/ai4se/owl#AI_Type"/>
        <papers:belongsToAIType rdf:resource="http://purl.org/ai4se/owl#Subsymbolic"/>
        <rdfs:comment xml:lang="en">Represents subsymbolic AI systems that rely on data and statistical inference to identify patterns and make predictions.</rdfs:comment>
        <rdfs:label>Statistical AI</rdfs:label>
    </owl:NamedIndividual>
    


    <!-- http://purl.org/ai4se/owl#Subsymbolic -->

    <owl:NamedIndividual rdf:about="http://purl.org/ai4se/owl#Subsymbolic">
        <rdf:type rdf:resource="http://purl.org/ai4se/owl#AI_Type"/>
        <rdfs:comment xml:lang="en">Represents AI systems that use numerical models to represent knowledge and computations, such as numerical optimisation and statistical learning, in order to model and solve problems.

According to ISO/IEC 22989:2022 Information technology - Artificial intelligence - Artificial intelligence concepts and terminology, subsymbolic AI is

- AI based on techniques and models that use an implicit encoding of information, that can be derived from experience or raw data.</rdfs:comment>
        <rdfs:label>Subsymbolic AI</rdfs:label>
    </owl:NamedIndividual>
    


    <!-- http://purl.org/ai4se/owl#Symbolic -->

    <owl:NamedIndividual rdf:about="http://purl.org/ai4se/owl#Symbolic">
        <rdf:type rdf:resource="http://purl.org/ai4se/owl#AI_Type"/>
        <rdfs:comment xml:lang="en">Represents AI systems that use approaches relying on the explicit definition of symbols and rules representing knowledge and performing logical reasoning.

According to ISO/IEC 22989:2022 Information technology - Artificial intelligence - Artificial intelligence concepts and terminology, symbolic AI is

- AI based on techniques and models that manipulate symbols and structures according to explicitly defined rules to obtain inferences.</rdfs:comment>
        <rdfs:label>Symbolic AI</rdfs:label>
    </owl:NamedIndividual>
    


    <!-- http://purl.org/ai4se/owl#Testing -->

    <owl:NamedIndividual rdf:about="http://purl.org/ai4se/owl#Testing">
        <rdf:type rdf:resource="http://purl.org/ai4se/papers#SE_target"/>
        <papers:belongsToSEActivity rdf:resource="http://purl.org/ai4se/owl#Develop"/>
        <rdfs:comment xml:lang="en">Represents software testing activities and processes.

Software testing encompasses the processes and activities used to evaluate the quality of a software or a component and of related artefacts.

According to ISO/IEC/IEEE 24765: Systems and software engineering - Vocabulary, software testing is

1. activity in which a system or component is executed under specified conditions, the results are observed or recorded, and an evaluation is made of some aspect of the system or component

2. dynamic verification that a program provides expected behaviors on a finite set of test cases, suitably selected from the usually infinite executions domain.</rdfs:comment>
        <rdfs:label>Software testing</rdfs:label>
    </owl:NamedIndividual>
    


    <!-- http://purl.org/ai4se/owl#Understand -->

    <owl:NamedIndividual rdf:about="http://purl.org/ai4se/owl#Understand">
        <rdf:type rdf:resource="http://purl.org/ai4se/owl#Solution_purpose"/>
        <rdfs:comment xml:lang="en">The purpose of using AI is to gain insight.</rdfs:comment>
        <rdfs:label>Understand</rdfs:label>
    </owl:NamedIndividual>
    


    <!-- 
    ///////////////////////////////////////////////////////////////////////////////////////
    //
    // General axioms
    //
    ///////////////////////////////////////////////////////////////////////////////////////
     -->

    <rdf:Description>
        <rdf:type rdf:resource="http://www.w3.org/2002/07/owl#AllDisjointProperties"/>
        <owl:members rdf:parseType="Collection">
            <rdf:Description rdf:about="http://purl.org/ai4se/papers#hasClassificationAIType"/>
            <rdf:Description rdf:about="http://purl.org/ai4se/papers#hasClassificationAutomationLevel"/>
            <rdf:Description rdf:about="http://purl.org/ai4se/papers#hasClassificationSolutionPurpose"/>
            <rdf:Description rdf:about="http://purl.org/ai4se/papers#hasClassificationSolutionTarget"/>
        </owl:members>
    </rdf:Description>
</rdf:RDF>



<!-- Generated by the OWL API (version 4.5.29.2024-05-13T12:11:03Z) https://github.com/owlcs/owlapi -->

