@prefix : <http://purl.org/ai4se/owl#> .
@prefix owl: <http://www.w3.org/2002/07/owl#> .
@prefix rdf: <http://www.w3.org/1999/02/22-rdf-syntax-ns#> .
@prefix xml: <http://www.w3.org/XML/1998/namespace> .
@prefix xsd: <http://www.w3.org/2001/XMLSchema#> .
@prefix gufo: <http://purl.org/nemo/gufo#> .
@prefix rdfs: <http://www.w3.org/2000/01/rdf-schema#> .
@prefix ai4se: <http://purl.org/ai4se/owl#> .
@base <http://purl.org/ai4se/owl#> .

<http://purl.org/ai4se/owl#> rdf:type owl:Ontology ;
                              owl:versionIRI <http://purl.org/ai4se/owl#/1.0.0> ;
                              owl:imports <http://purl.org/nemo/gufo#/1.0.0> ;
                              <http://purl.org/dc/elements/1.1/creator> "Schieferdecker, Ina K." ;
                              <http://purl.org/dc/elements/1.1/title> "ai4se: A taxonomy of research papers on the support of software engineering (SE) through the use of artificial intelligence (AI) methods and techniques."@en ;
                              <http://purl.org/dc/terms/bibliographicCitation> "Schieferdecker, I.K.: \"ai4se: A taxonomy of research papers on the support of software engineering (SE) through the use of artificial intelligence (AI) methods and techniques\", 2025, http://purl.org/ai4se/doc"@en ;
                              <http://purl.org/dc/terms/license> "https://creativecommons.org/licenses/by/4.0/legalcode.en" ;
                              <http://purl.org/vocab/vann/preferredNamespacePrefix> "ai4se"@en ;
                              <http://purl.org/vocab/vann/preferredNamespaceUri> "http://purl.org/ai4se/owl/"^^xsd:anyURI ;
                              rdfs:comment "tbd"@en ;
                              owl:versionInfo 2 .

#################################################################
#    Object Properties
#################################################################

###  http://purl.org/ai4se/owl#hasAutomationLevel
ai4se:hasAutomationLevel rdf:type owl:ObjectProperty ;
                         rdfs:subPropertyOf gufo:inheresIn ;
                         rdfs:domain <http://purl.org/ai4se/papers#Research_contribution> ;
                         rdfs:range ai4se:AIAutomationLevel ;
                         rdfs:comment "Represents the automation level of the AI solution being proposed, applied or developed in a research paper."@en ;
                         rdfs:label "hasAutomationLevel" .


###  http://purl.org/ai4se/owl#hasSolutionPurpose
ai4se:hasSolutionPurpose rdf:type owl:ObjectProperty ;
                         rdfs:subPropertyOf gufo:inheresIn ;
                         rdfs:domain <http://purl.org/ai4se/papers#Research_contribution> ;
                         rdfs:range ai4se:SolutionPurpose ;
                         rdfs:comment "Represents the purpose of the AI solution being proposed, applied or developed in a research paper."@en ;
                         rdfs:label "hasSolutionPurpose" .


###  http://purl.org/ai4se/owl#isAboutResearchTopic
ai4se:isAboutResearchTopic rdf:type owl:ObjectProperty ;
                           rdfs:subPropertyOf gufo:historicallyDependsOn ;
                           rdfs:domain ai4se:Research_paper ;
                           rdfs:range ai4se:CSO:Topic ;
                           rdfs:comment "Represents the research topics that a research paper contributes to."@en ;
                           rdfs:label "isAboutResearchTopic" .


###  http://purl.org/ai4se/owl#isInResearchCollection
ai4se:isInResearchCollection rdf:type owl:ObjectProperty ;
                             rdfs:subPropertyOf gufo:historicallyDependsOn ;
                             rdf:type owl:TransitiveProperty ,
                                      owl:IrreflexiveProperty ;
                             rdfs:domain ai4se:Research_paper ,
                                         ai4se:Research_paper_collection ;
                             rdfs:range ai4se:Research_paper_collection ;
                             rdfs:comment "Represents the membership of a research paper or research paper collection to a research paper collection."@en ;
                             rdfs:label "isInResearchCollection" .


###  http://purl.org/ai4se/owl#isProperPartOfProcess
ai4se:isProperPartOfProcess rdf:type owl:ObjectProperty ;
                            rdfs:subPropertyOf gufo:isEventProperPartOf ;
                            rdfs:domain ai4se:PrMO:Activity ;
                            rdfs:range ai4se:PrMO:Process ;
                            rdfs:comment "Represents activities being part of processes."@en ;
                            rdfs:label "isPartOfProcess" .


###  http://purl.org/ai4se/owl#mediatesMDSEModel
ai4se:mediatesMDSEModel rdf:type owl:ObjectProperty ;
                        rdfs:subPropertyOf gufo:mediates ;
                        rdfs:domain ai4se:Model-Driven_Software_Engineering ;
                        rdfs:range ai4se:Model .


###  http://purl.org/ai4se/papers#hasAutomationLevelValue
<http://purl.org/ai4se/papers#hasAutomationLevelValue> rdf:type owl:ObjectProperty ;
                                                       rdfs:subPropertyOf gufo:hasReifiedQualityValue ;
                                                       rdf:type owl:FunctionalProperty ;
                                                       rdfs:domain ai4se:AIAutomationLevel ;
                                                       rdfs:range <http://purl.org/ai4se/papers#Automation_level_value> .


###  http://purl.org/ai4se/papers#mediatesContributionResearchTopic
<http://purl.org/ai4se/papers#mediatesContributionResearchTopic> rdf:type owl:ObjectProperty ;
                                                                 rdfs:subPropertyOf gufo:mediates ;
                                                                 rdfs:domain <http://purl.org/ai4se/papers#Research_contribution> ;
                                                                 rdfs:range ai4se:CSO:Topic .


###  http://purl.org/ai4se/papers#mediatesMDSETarget
<http://purl.org/ai4se/papers#mediatesMDSETarget> rdf:type owl:ObjectProperty ;
                                                  rdfs:subPropertyOf gufo:mediates ;
                                                  rdfs:domain ai4se:Model-Driven_Software_Engineering ;
                                                  rdfs:range ai4se:Target .


###  http://purl.org/ai4se/papers#mediatesTarget
<http://purl.org/ai4se/papers#mediatesTarget> rdf:type owl:ObjectProperty ;
                                              rdfs:subPropertyOf gufo:manifestedIn ;
                                              rdf:type owl:FunctionalProperty ;
                                              rdfs:domain <http://purl.org/ai4se/papers#Research_contribution> ;
                                              rdfs:range ai4se:Target .


###  http://purl.org/ai4se/papers#mediatesTopicResearchPaper
<http://purl.org/ai4se/papers#mediatesTopicResearchPaper> rdf:type owl:ObjectProperty ;
                                                          rdfs:subPropertyOf gufo:mediates ;
                                                          rdfs:domain <http://purl.org/ai4se/papers#Research_topic> ;
                                                          rdfs:range ai4se:Research_paper .


###  http://purl.org/ai4se/papers#mediatesTopicResearchTopic
<http://purl.org/ai4se/papers#mediatesTopicResearchTopic> rdf:type owl:ObjectProperty ;
                                                          rdfs:subPropertyOf gufo:mediates ;
                                                          rdfs:domain <http://purl.org/ai4se/papers#Research_topic> ;
                                                          rdfs:range ai4se:CSO:Topic .


###  http://purl.org/ai4se/papers#usesAIType
<http://purl.org/ai4se/papers#usesAIType> rdf:type owl:ObjectProperty ;
                                          rdfs:subPropertyOf gufo:mediates ;
                                          rdfs:domain <http://purl.org/ai4se/papers#Research_contribution> ;
                                          rdfs:range ai4se:Type .


###  http://www.w3.org/2002/07/owl#topObjectProperty
owl:topObjectProperty rdfs:domain ai4se:Research_paper_collection .


#################################################################
#    Classes
#################################################################

###  http://purl.org/ai4se/owl#AIAutomationLevel
ai4se:AIAutomationLevel rdf:type owl:Class ;
                        rdfs:subClassOf gufo:Quality ;
                        rdfs:label """Represents the level of automation provided / enabled by the AI system being used.

According to ISO/IEC 22989:2022 Information technology - Artificial intelligence - Artificial intelligence concepts and terminology, artificial intelligence (AI) is

- <discipline> research and development of mechanisms and applications of AI systems.

and

artificial intelligence system (AI system) is

- engineered system that generates outputs such as content, forecasts, recommendations or decisions for a given set of human-defined objectives."""@en ,
                                   "Level of AI automation" .


###  http://purl.org/ai4se/owl#Miscellaneous
ai4se:Miscellaneous rdf:type owl:Class ;
                    rdfs:comment """This is a collection of the fundamental concepts of the software development life cycle.

As no comprehensive, predefined ontology is available from SWEBOK, ISO, IEC, IEEE, or other sources, a lightweight approach was taken for the ai4se ontology: Fundamental concepts of SDLC needed for the understanding of ai4se are collected and definitions are referred to from selected sources."""@en ;
                    rdfs:isDefinedBy """610.12-1990 - IEEE Standard Glossary of Software Engineering Terminology:

https://ieeexplore.ieee.org/document/159342""" ,
                                     """SWEBOK v4.0: Software Engineering Body of Knowledge 

https://www.computer.org/education/bodies-of-knowledge/software-engineering""" ;
                    rdfs:label "Misc" .


###  http://purl.org/ai4se/owl#Model
ai4se:Model rdf:type owl:Class ;
            rdfs:subClassOf gufo:FunctionalComplex ;
            rdfs:comment """Represents artifacts defining (semi-)formally (1) properties of one or more artefacts used by software engineering activities or processes or (2) properties of software engineering activities or processes.

According to ISO/IEC 22989:2022 Information technology - Artificial intelligence - Artificial intelligence concepts and terminology, model is

- physical, mathematical or otherwise logical representation of a system, entity, phenomenon, process or data.

Note: For the AI4SE ontology, only mathematical or logical representations are relevant."""@en ;
            rdfs:label "Model" .


###  http://purl.org/ai4se/owl#Model-Driven_Software_Engineering
ai4se:Model-Driven_Software_Engineering rdf:type owl:Class ;
                                        rdfs:subClassOf gufo:Relator ;
                                        rdfs:comment """Relates software activities and processes to models used for model-driven software engineering.

Model-driven software engineering (MDSE) refers to software engineering methodologies that focus on creating and exploiting (domain-specific) models. These are conceptual models that describe various aspects of software, its components and/or environment, and the processes and/or activities used to develop and operate it. Rather than just focusing on programming and code, MDSE emphasises the use of models as the primary artefacts in software engineering processes."""@en ;
                                        rdfs:label "Model-Driven Software Engineering" .


###  http://purl.org/ai4se/owl#Research_paper
ai4se:Research_paper rdf:type owl:Class ;
                     rdfs:subClassOf gufo:FunctionalComplex ;
                     rdfs:comment "Represents an artefact that documents research findings, such as new insights, methods or techniques. It has been reviewed, published and is digitally accessible."@en ;
                     rdfs:label "Research paper" .


###  http://purl.org/ai4se/owl#Research_paper_collection
ai4se:Research_paper_collection rdf:type owl:Class ;
                                rdfs:subClassOf gufo:VariableCollection ;
                                rdfs:comment "A collection of research papers contributing to the body of knowledge in a given field, for a research topic, research question(s) or a given problem statement."@en ;
                                rdfs:label "Research paper collection" .


###  http://purl.org/ai4se/owl#SolutionPurpose
ai4se:SolutionPurpose rdf:type owl:Class ;
                      rdfs:subClassOf gufo:Quality ;
                      rdfs:comment "Represents the purpose of using the AI system in a software development / operation processes or activities."@en ;
                      rdfs:label "Solution purpose" .


###  http://purl.org/ai4se/owl#Target
ai4se:Target rdf:type owl:Class ;
             rdfs:subClassOf gufo:Event ;
             rdfs:comment "Represents the primary concept, issue, component, software, or process in a software engineering process or activitiy being addressed."@en ;
             rdfs:label "Solution target" .


###  http://purl.org/ai4se/owl#Type
ai4se:Type rdf:type owl:Class ;
           rdfs:subClassOf gufo:Category ;
           rdfs:comment """Represents the type of the artificial intelligence (AI) system being used.

According to ISO/IEC 22989:2022 Information technology - Artificial intelligence - Artificial intelligence concepts and terminology, artificial intelligence (AI) is

- <discipline> research and development of mechanisms and applications of AI systems.

and

artificial intelligence system (AI system) is

- engineered system that generates outputs such as content, forecasts, recommendations or decisions for a given set of human-defined objectives."""@en ;
           rdfs:label "Type of AI system" .


###  http://purl.org/ai4se/owl#CSO:Topic
ai4se:CSO:Topic rdf:type owl:Class ;
                rdfs:subClassOf ai4se:Miscellaneous ,
                                gufo:Category ;
                rdfs:isDefinedBy "https://cso.kmi.open.ac.uk/" ;
                rdfs:label "Represents the research topics in Computer Science as defined by the Computer Science Ontology CSO."@en ,
                           "CSO:Topic" .


###  http://purl.org/ai4se/owl#ODYSSEY:Phase
ai4se:ODYSSEY:Phase rdf:type owl:Class ;
                    rdfs:subClassOf ai4se:Miscellaneous ;
                    rdfs:comment "Represents a phase in the software development life cycle as e.g. defined in the Software Development Life Cycle Ontology ODYSSEY."@en ;
                    rdfs:isDefinedBy "https://www.scitepress.org/Papers/2018/69577/69577.pdf" ;
                    rdfs:label "SDLC:Phase" .


###  http://purl.org/ai4se/owl#PrMO:Activity
ai4se:PrMO:Activity rdf:type owl:Class ;
                    rdfs:subClassOf ai4se:Miscellaneous ,
                                    gufo:Event ;
                    rdfs:comment """Represents a set of tasks used to produce, operate or maintain software-based products or services as well as to achieve the objectives of the process it belongs to. The activity includes the procedures, standards, policies, and objectives to create and modify a set of work products. 

Adapted to software-related activities from PrMO: an ontology of process-reference models."""@en ;
                    rdfs:isDefinedBy "https://www.redalyc.org/articulo.oa?id=43032606003" ;
                    rdfs:label "PrMO:Activity" .


###  http://purl.org/ai4se/owl#PrMO:Process
ai4se:PrMO:Process rdf:type owl:Class ;
                   rdfs:subClassOf ai4se:PrMO:Activity ;
                   rdfs:comment """Represents a coherent set of policies, organizational structures, technologies; procedures, purposes, objectives, and work products that are needed to design, develop, deploy and maintain a software product.

Defined by PrMO: an ontology of process-reference models"""@en ;
                   rdfs:isDefinedBy "https://www.redalyc.org/articulo.oa?id=43032606003" ;
                   rdfs:label "PrMO:Process" .


###  http://purl.org/ai4se/papers#Automation_level_value
<http://purl.org/ai4se/papers#Automation_level_value> rdf:type owl:Class ;
                                                      owl:equivalentClass [ rdf:type owl:Class ;
                                                                            owl:oneOf ( ai4se:AI-assisted_options
                                                                                        ai4se:AI-assisted_selection
                                                                                        ai4se:AI-driven_full_automation
                                                                                        ai4se:AI-driven_partial_automation
                                                                                        ai4se:No_AI_support
                                                                                      )
                                                                          ] ;
                                                      rdfs:subClassOf gufo:QualityValue ;
                                                      rdfs:comment "Represent the automation levels achieved by an AI system in a research contribution."@en ;
                                                      rdfs:label "Automation level value" .


###  http://purl.org/ai4se/papers#Research_contribution
<http://purl.org/ai4se/papers#Research_contribution> rdf:type owl:Class ;
                                                     rdfs:subClassOf gufo:Relator ;
                                                     rdfs:comment "Represents the specific research contribution(s) made by a specific research paper."@en ;
                                                     rdfs:label "Research contribution" .


###  http://purl.org/ai4se/papers#Research_topic
<http://purl.org/ai4se/papers#Research_topic> rdf:type owl:Class ;
                                              rdfs:subClassOf gufo:Relator ;
                                              rdfs:comment "Represents the research topic of a research paper or of a research contribution."@en ;
                                              rdfs:label "Research topic" .


###  http://purl.org/ai4se/papers#Solution_purpose_value
<http://purl.org/ai4se/papers#Solution_purpose_value> rdf:type owl:Class ;
                                                      rdfs:subClassOf gufo:QualityValue ;
                                                      rdfs:comment "Represents the purpose of an AI system in a research contribution."@en ;
                                                      rdfs:label "Solution purpose value" .


#################################################################
#    Individuals
#################################################################

###  http://purl.org/ai4se/owl#AI-assisted_options
ai4se:AI-assisted_options rdf:type owl:NamedIndividual ,
                                   <http://purl.org/ai4se/papers#Automation_level_value> ;
                          rdfs:comment "Represents the case in which choices, recommendations, or decision-support outputs for the target SE processes or activities are generated or enhanced by an AI system, while retaining human control over the final choice, recommendation or decision, which may differ from the AI outputs."@en ;
                          rdfs:label "AI-assisted options" .


###  http://purl.org/ai4se/owl#AI-assisted_selection
ai4se:AI-assisted_selection rdf:type owl:NamedIndividual ,
                                     <http://purl.org/ai4se/papers#Automation_level_value> ;
                            rdfs:comment "Represents the case in which choices, recommendations, or decision-support outputs for the target SE processes or activities are generated or enhanced by an AI system, where the final choices, recommendations or decisions require human confirmation and do not differ from the AI outputs."@en ;
                            rdfs:label "AI-assisted selection" .


###  http://purl.org/ai4se/owl#AI-driven_full_automation
ai4se:AI-driven_full_automation rdf:type owl:NamedIndividual ,
                                         <http://purl.org/ai4se/papers#Automation_level_value> ;
                                rdfs:comment "Represents the case in which AI is used to automate all tasks or decision-making components within the target SE processes or activities, without requiring human intervention."@en ;
                                rdfs:label "AI-driven full automation" .


###  http://purl.org/ai4se/owl#AI-driven_partial_automation
ai4se:AI-driven_partial_automation rdf:type owl:NamedIndividual ,
                                            <http://purl.org/ai4se/papers#Automation_level_value> ;
                                   rdfs:comment "Represents the case in which AI is used to automate specific tasks or decision-making components within the target SE processes or activities, while other parts of the process remain under human control or require human intervention."@en ;
                                   rdfs:label "AI-driven partial automation" .


###  http://purl.org/ai4se/owl#Agentic_AI
ai4se:Agentic_AI rdf:type owl:NamedIndividual ,
                          ai4se:Type ;
                 rdfs:comment "Represents AI systems that rely on autonomous agents using AI techniques to plan, adapt, and execute multi-step objectives with minimal human control."@en ;
                 rdfs:label "Agentic AI" .


###  http://purl.org/ai4se/owl#Architecture_and_Design
ai4se:Architecture_and_Design rdf:type owl:NamedIndividual ,
                                       ai4se:Target ;
                              rdfs:comment """Represents software architecture and design activities and processes. 

A software architecture defines its fundamental organization, its components, their relationships, and the principles guiding its design and evolution. 
 
According to ISO/IEC/IEEE 42010:2022: Software, systems and enterprise - Architecture description), a software architecture consists of the fundamental concepts or properties of an entity in its environment and governing principles for the realization and evolution of this entity and its related life cycle processes.

Software design is the process of defining the architecture, components, interfaces, and other characteristics of a software or a component.

According to ISO/IEC/IEEE 24765: Systems and software engineering - Vocabulary, software design is  

1. the use of scientific principles, technical information, and imagination in the definition of a software system to perform pre-specified functions with maximum economy and efficiency."""@en ;
                              rdfs:label "Software architecture and design" .


###  http://purl.org/ai4se/owl#Classical_machine_learning
ai4se:Classical_machine_learning rdf:type owl:NamedIndividual ,
                                          ai4se:Type ;
                                 rdfs:comment """Represents subsymbolic AI systems that rely on statistical and algorithmic learning techniques - such as decision trees, support vector machines, linear regression, and clustering - to learn patterns from structured data and make predictions or classifications. These models typically operate on explicitly defined features and do not involve deep neural networks.

This class of AI is used in contrast to deep learning AI."""@en ;
                                 rdfs:label "Classical machine learning" .


###  http://purl.org/ai4se/owl#Coding
ai4se:Coding rdf:type owl:NamedIndividual ,
                      ai4se:Target ;
             rdfs:comment """Represents coding activities and processes. 

Coding (also known as programming) is the process of transforming the design of a software or a component into an executable computer program.

According to ISO/IEC/IEEE 24765: Systems and software engineering - Vocabulary, coding is

1. in software engineering, the process of expressing a computer program in a programming language

2. transforming of logic and data from design specifications (design descriptions) into a programming language."""@en ;
             rdfs:label "Software coding" .


###  http://purl.org/ai4se/owl#Deep_learning
ai4se:Deep_learning rdf:type owl:NamedIndividual ,
                             ai4se:Type ;
                    rdfs:comment """Represents subsymbolic AI systems that rely on deep artificial neural networks to automatically learn features and perform tasks such as classification or prediction, especially from large and complex datasets. 

According to ISO/IEC 22989:2022 Information technology - Artificial intelligence - Artificial intelligence concepts and terminology, deep learning (deep neural network learning) is

- AI approach to creating rich hierarchical representations through the training of neural networks with many hidden layers."""@en ;
                    rdfs:label "Deep learning AI" .


###  http://purl.org/ai4se/owl#Deployment
ai4se:Deployment rdf:type owl:NamedIndividual ,
                          ai4se:Target ;
                 rdfs:comment """Represents software deployment activities and processes.

Software deployment encompasses the processes and activities for placing a software or component into an operational environment.

According to ISO/IEC/IEEE 24765: Systems and software engineering - Vocabulary, deployment is 

1. a phase of a project in which a system is put into operation and cutover issues are resolved."""@en ;
                 rdfs:label "Software deployment" .


###  http://purl.org/ai4se/owl#Develop
ai4se:Develop rdf:type owl:NamedIndividual ,
                       ai4se:Target ;
              rdfs:label """Represents software development activities and processes.

Software development is the set of activities that result in software products, including requirements analysis, design, coding, testing, and maintenance. It encompasses all the activities and processes involved in creating, implementing, and modifying software (artefacts), as well as ensuring that it satisfies stakeholder requirements throughout the software development life cycle."""@en ,
                         "Develop" .


###  http://purl.org/ai4se/owl#General_AI
ai4se:General_AI rdf:type owl:NamedIndividual ,
                          ai4se:Type ;
                 rdfs:comment """Represents AI systems capable of performing a broad set of distinct tasks with satisfactory performance.

According to ISO/IEC 22989:2022 Information technology - Artificial intelligence - Artificial intelligence concepts and terminology, general AI (AGI, artificial general intelligence)

- type of AI system that addresses a broad range of tasks with a satisfactory level of performance 

Note 1: Compared to narrow AI.
Note 2: AGI is often used in a stronger sense, meaning systems that not only can perform a wide variety of tasks, but all tasks that a human can perform."""@en ;
                 rdfs:label "General AI" .


###  http://purl.org/ai4se/owl#Generate
ai4se:Generate rdf:type owl:NamedIndividual ,
                        <http://purl.org/ai4se/papers#Solution_purpose_value> .


###  http://purl.org/ai4se/owl#Generative_AI
ai4se:Generative_AI rdf:type owl:NamedIndividual ,
                             ai4se:Type ;
                    rdfs:comment "Represents AI systems that use learned or derived knowledge to produce original outputs, such as synthetic text, media, or other content types. It often uses subsymbolic AI like Convolutional Neural Networks (CNNs), Recurrent Neural Networks (RNNs), or Transformer-based models, but also symbolic AI."@en ;
                    rdfs:label "Generative AI" .


###  http://purl.org/ai4se/owl#Improve
ai4se:Improve rdf:type owl:NamedIndividual ,
                       <http://purl.org/ai4se/papers#Solution_purpose_value> ;
              rdfs:comment "The purpose of using AI is to improve (parts of) artefacts used in software engineering."@en ;
              rdfs:label "Improve" .


###  http://purl.org/ai4se/owl#Improvement
ai4se:Improvement rdf:type owl:NamedIndividual ,
                           ai4se:Target .


###  http://purl.org/ai4se/owl#Maintenance
ai4se:Maintenance rdf:type owl:NamedIndividual ,
                           ai4se:Target ;
                  rdfs:comment """Represents software maintenance activities and processes. 

Software maintenance is the process of modifying a software or component after delivery to correct faults, improve performance or other attributes, or adapt to a changed environment.

According to ISO/IEC/IEEE 24765: Systems and software engineering - Vocabulary, software maintenance is 

1. totality of activities required to provide cost-effective support to a software system 

2. entitlement of additional rights (such as additional
functionality, upgrade or support) for a previously granted software entitlement"""@en ;
                  rdfs:label "Software maintenance" .


###  http://purl.org/ai4se/owl#Management
ai4se:Management rdf:type owl:NamedIndividual ,
                          ai4se:Target .


###  http://purl.org/ai4se/owl#Monitoring
ai4se:Monitoring rdf:type owl:NamedIndividual ,
                          ai4se:Target ;
                 rdfs:comment """Represents software monitoring activities and processes.

Software monitoring is systematically observing, checking, or keeping track of the operations or performance of a software or component."""@en ;
                 rdfs:label "Software monitoring" .


###  http://purl.org/ai4se/owl#No_AI_support
ai4se:No_AI_support rdf:type owl:NamedIndividual ,
                             <http://purl.org/ai4se/papers#Automation_level_value> ;
                    rdfs:comment "Represents the case in which the target SE processes or activities are performed without the assistance of AI."@en ;
                    rdfs:label "No AI-supported automation" .


###  http://purl.org/ai4se/owl#Operate
ai4se:Operate rdf:type owl:NamedIndividual ,
                       ai4se:Target ;
              rdfs:comment "Represents software operation activities and processs."@en ;
              rdfs:label "Operate" .


###  http://purl.org/ai4se/owl#Operation
ai4se:Operation rdf:type owl:NamedIndividual ,
                         ai4se:Target ;
                rdfs:comment """Represents software operation activities and processes.

Software operation refers to

1. The use and execution of software in its production environment to perform its intended functions.

2. Running a software to deliver services or perform tasks for users or other systems."""@en ;
                rdfs:label "Software operation" .


###  http://purl.org/ai4se/owl#Process
ai4se:Process rdf:type owl:NamedIndividual ,
                       ai4se:Target ;
              rdfs:label "Represents processes for software engineering along the software lifecycle of software development and operation."@en ,
                         "Software Engineering Processes" .


###  http://purl.org/ai4se/owl#Requirements_engineering
ai4se:Requirements_engineering rdf:type owl:NamedIndividual ,
                                        ai4se:Target ;
                               rdfs:comment """Represents requirements engineering activities and processes. 

A software requirement is a condition or capability that must be met by a software or component.

According to ISO/IEC/IEEE 24765: Systems and software engineering - Vocabulary, software requirement is

1. software capability needed by a user to solve a problem or to achieve an objective

2. software capability that must be met or possessed by a system or system component to satisfy a contract, standard, specification, or other formally imposed document

According to ISO/IEC/IEEE 24765: Systems and software engineering - Vocabulary, software requirements engineering is

1. science and discipline concerned with analyzing and documenting software requirements 

2. software requirements elicitation, analysis, specification, verification, and management"""@en ;
                               rdfs:label "Requirements engineering" .


###  http://purl.org/ai4se/owl#Software_Engineering
ai4se:Software_Engineering rdf:type owl:NamedIndividual ,
                                    ai4se:Target ,
                                    ai4se:PrMO:Activity ,
                                    ai4se:PrMO:Process .


###  http://purl.org/ai4se/owl#Statistical
ai4se:Statistical rdf:type owl:NamedIndividual ,
                           ai4se:Type ;
                  rdfs:comment "Represents subsymbolic AI systems that rely on data and statistical inference to identify patterns and make predictions."@en ;
                  rdfs:label "Statistical AI" .


###  http://purl.org/ai4se/owl#Subsymbolic
ai4se:Subsymbolic rdf:type owl:NamedIndividual ,
                           ai4se:Type ;
                  rdfs:comment """Represents AI systems that use numerical models to represent knowledge and computations, such as numerical optimisation and statistical learning, in order to model and solve problems.

According to ISO/IEC 22989:2022 Information technology - Artificial intelligence - Artificial intelligence concepts and terminology, subsymbolic AI is

- AI based on techniques and models that use an implicit encoding of information, that can be derived from experience or raw data."""@en ;
                  rdfs:label "Subsymbolic AI" .


###  http://purl.org/ai4se/owl#Symbolic
ai4se:Symbolic rdf:type owl:NamedIndividual ,
                        ai4se:Type ;
               rdfs:comment """Represents AI systems that use approaches relying on the explicit definition of symbols and rules representing knowledge and performing logical reasoning.

According to ISO/IEC 22989:2022 Information technology - Artificial intelligence - Artificial intelligence concepts and terminology, symbolic AI is

- AI based on techniques and models that manipulate symbols and structures according to explicitly defined rules to obtain inferences."""@en ;
               rdfs:label "Symbolic AI" .


###  http://purl.org/ai4se/owl#Testing
ai4se:Testing rdf:type owl:NamedIndividual ,
                       ai4se:Target ;
              rdfs:comment """Represents software testing activities and processes.

Software testing encompasses the processes and activities used to evaluate the quality of a software or a component and of related artefacts.

According to ISO/IEC/IEEE 24765: Systems and software engineering - Vocabulary, software testing is

1. activity in which a system or component is executed under specified conditions, the results are observed or recorded, and an evaluation is made of some aspect of the system or component

2. dynamic verification that a program provides expected behaviors on a finite set of test cases, suitably selected from the usually infinite executions domain."""@en ;
              rdfs:label "Software testing" .


###  http://purl.org/ai4se/owl#Understand
ai4se:Understand rdf:type owl:NamedIndividual ,
                          <http://purl.org/ai4se/papers#Solution_purpose_value> ;
                 rdfs:comment "The purpose of using AI is to gain insight."@en ;
                 rdfs:label "Understand" .


###  http://purl.org/ai4se/papers#lin_traceability_2021
<http://purl.org/ai4se/papers#lin_traceability_2021> rdf:type owl:NamedIndividual ,
                                                              ai4se:Research_paper .


###  http://purl.org/ai4se/papers#lin_traceability_2021_contrib
<http://purl.org/ai4se/papers#lin_traceability_2021_contrib> rdf:type owl:NamedIndividual ,
                                                                      <http://purl.org/ai4se/papers#Research_contribution> ;
                                                             <http://purl.org/ai4se/papers#mediatesTarget> ai4se:Develop ;
                                                             gufo:hasQualityValue "AI-driven_partial_automation" ,
                                                                                  "Deep_learning" ,
                                                                                  "Generate" ,
                                                                                  "Improve" .


###  Generated by the OWL API (version 4.5.29.2024-05-13T12:11:03Z) https://github.com/owlcs/owlapi
