@prefix : <http://purl.org/ai4se/owl#> .
@prefix owl: <http://www.w3.org/2002/07/owl#> .
@prefix rdf: <http://www.w3.org/1999/02/22-rdf-syntax-ns#> .
@prefix xml: <http://www.w3.org/XML/1998/namespace> .
@prefix xsd: <http://www.w3.org/2001/XMLSchema#> .
@prefix gufo: <http://purl.org/nemo/gufo#> .
@prefix rdfs: <http://www.w3.org/2000/01/rdf-schema#> .
@prefix ai4se: <http://purl.org/ai4se/owl#> .
@base <http://purl.org/ai4se/owl#> .

<http://purl.org/ai4se/owl#> rdf:type owl:Ontology ;
                              owl:versionIRI <http://purl.org/ai4se/owl#/1.0.0> ;
                              owl:imports <http://purl.org/nemo/gufo#/1.0.0> ;
                              <http://purl.org/dc/elements/1.1/creator> "Schieferdecker, Ina K." ;
                              <http://purl.org/dc/elements/1.1/title> "ai4se: A taxonomy of research papers on the support of software engineering (SE) through the use of artificial intelligence (AI) methods and techniques."@en ;
                              <http://purl.org/dc/terms/bibliographicCitation> "Schieferdecker, I.K.: \"ai4se: A taxonomy of research papers on the support of software engineering (SE) through the use of artificial intelligence (AI) methods and techniques\", 2025, http://purl.org/ai4se/doc"@en ;
                              <http://purl.org/dc/terms/license> "https://creativecommons.org/licenses/by/4.0/legalcode.en" ;
                              <http://purl.org/vocab/vann/preferredNamespacePrefix> "ai4se"@en ;
                              <http://purl.org/vocab/vann/preferredNamespaceUri> "http://purl.org/ai4se/owl/"^^xsd:anyURI ;
                              rdfs:comment "tbd"@en ;
                              owl:versionInfo 2 .

#################################################################
#    Object Properties
#################################################################

###  http://purl.org/ai4se/owl#hasAIType
ai4se:hasAIType rdf:type owl:ObjectProperty ;
                rdfs:subPropertyOf gufo:standsInQualifiedAttribution ;
                rdfs:domain ai4se:ResearchPaper ;
                rdfs:range ai4se:Type .


###  http://purl.org/ai4se/owl#hasAutomationLevel
ai4se:hasAutomationLevel rdf:type owl:ObjectProperty ;
                         rdfs:subPropertyOf gufo:standsInQualifiedAttribution ;
                         rdfs:domain ai4se:ResearchPaper ;
                         rdfs:range ai4se:Level .


###  http://purl.org/ai4se/owl#hasSolutionPurpose
ai4se:hasSolutionPurpose rdf:type owl:ObjectProperty ;
                         rdfs:subPropertyOf gufo:standsInQualifiedAttribution ;
                         rdfs:domain ai4se:ResearchPaper ;
                         rdfs:range ai4se:Purpose .


###  http://purl.org/ai4se/owl#hasSolutionTarget
ai4se:hasSolutionTarget rdf:type owl:ObjectProperty ;
                        rdfs:subPropertyOf gufo:standsInQualifiedAttribution ;
                        rdfs:domain ai4se:ResearchPaper ;
                        rdfs:range ai4se:Target .


###  http://purl.org/ai4se/owl#isAboutTopic
ai4se:isAboutTopic rdf:type owl:ObjectProperty ;
                   rdfs:subPropertyOf gufo:inheresIn ;
                   rdfs:domain ai4se:ResearchPaper ;
                   rdfs:range ai4se:CSO:Topic ;
                   rdfs:comment "Represents the focus of a research paper on a research topic."@en ;
                   rdfs:label "isAboutTopic" .


###  http://purl.org/ai4se/owl#isInResearchCollection
ai4se:isInResearchCollection rdf:type owl:ObjectProperty ;
                             rdfs:subPropertyOf gufo:isCollectionMemberOf ,
                                                gufo:isSubCollectionOf ;
                             rdf:type owl:TransitiveProperty ;
                             rdfs:domain ai4se:ResearchPaper ,
                                         ai4se:ResearchPaperCollection ;
                             rdfs:range ai4se:ResearchPaperCollection ;
                             rdfs:comment "Represents the hierarchical inclusion of research paper collections."@en ,
                                          "Represents the membership of a research paper to a research paper collection."@en ;
                             rdfs:label "isInResearchCollection" .


###  http://purl.org/ai4se/owl#isProperPartOfProcess
ai4se:isProperPartOfProcess rdf:type owl:ObjectProperty ;
                            rdfs:subPropertyOf gufo:isEventProperPartOf ;
                            rdf:type owl:TransitiveProperty ;
                            rdfs:domain ai4se:PrMO:Activity ;
                            rdfs:range ai4se:PrMO:Process ;
                            rdfs:comment "Represents activities being part of processes."@en ;
                            rdfs:label "isPartOfProcess" .


#################################################################
#    Classes
#################################################################

###  http://purl.org/ai4se/owl#Level
ai4se:Level rdf:type owl:Class ;
            rdfs:subClassOf gufo:QualityValueAttributionSituation ;
            rdfs:label "Represents the level of automation provided / enabled by the proposed approach, method, and/or technique."@en ,
                       "Level of automation" .


###  http://purl.org/ai4se/owl#Miscellaneous
ai4se:Miscellaneous rdf:type owl:Class ;
                    rdfs:comment """This is a collection of the fundamental concepts of the software development life cycle.

As no comprehensive, predefined ontology is available from SWEBOK, ISO, IEC, IEEE, or other sources, a lightweight approach was taken for the ai4se ontology: Fundamental concepts of SDLC needed for the understanding of ai4se are collected and definitions are referred to from selected sources."""@en ;
                    rdfs:isDefinedBy """610.12-1990 - IEEE Standard Glossary of Software Engineering Terminology:

https://ieeexplore.ieee.org/document/159342""" ,
                                     """SWEBOK v4.0: Software Engineering Body of Knowledge 

https://www.computer.org/education/bodies-of-knowledge/software-engineering""" ;
                    rdfs:label "Misc" .


###  http://purl.org/ai4se/owl#Purpose
ai4se:Purpose rdf:type owl:Class ;
              rdfs:subClassOf gufo:QualityValueAttributionSituation ;
              rdfs:comment "Represents the purpose of using an AI-based solution in a software development / operation processes or activities."@en ;
              rdfs:label "Solution purpose" .


###  http://purl.org/ai4se/owl#ResearchPaper
ai4se:ResearchPaper rdf:type owl:Class ;
                    rdfs:subClassOf gufo:FunctionalComplex ;
                    rdfs:comment "An artifact documenting research findings like new insights, methods, techniques, etc."@en ;
                    rdfs:label "ResearchPaper" .


###  http://purl.org/ai4se/owl#ResearchPaperCollection
ai4se:ResearchPaperCollection rdf:type owl:Class ;
                              rdfs:subClassOf gufo:VariableCollection ;
                              rdfs:comment "A collection of research papers contributing to the body of knowledge in a given field, for a research topic, research question(s) or a given problem statement."@en ;
                              rdfs:label "ResearchPaperCollection" .


###  http://purl.org/ai4se/owl#Target
ai4se:Target rdf:type owl:Class ;
             rdfs:subClassOf gufo:QualityValueAttributionSituation ;
             rdfs:comment "Represents the primary object, system, concept, or issue in a software development / operation process or activitiy being addressed."@en ;
             rdfs:label "Solution target" .


###  http://purl.org/ai4se/owl#Type
ai4se:Type rdf:type owl:Class ;
           rdfs:subClassOf gufo:QualityValueAttributionSituation ;
           rdfs:comment "Represents the type of AI being used in the presented solution."@en ;
           rdfs:label "AI Type" .


###  http://purl.org/ai4se/owl#CSO:Topic
ai4se:CSO:Topic rdf:type owl:Class ;
                rdfs:subClassOf ai4se:Miscellaneous ,
                                gufo:Kind ;
                rdfs:isDefinedBy "https://cso.kmi.open.ac.uk/" ;
                rdfs:label "Represents the research topics in Computer Science as defined by the Computer Science Ontology CSO."@en ,
                           "CSO:Topic" .


###  http://purl.org/ai4se/owl#ODYSSEY:Phase
ai4se:ODYSSEY:Phase rdf:type owl:Class ;
                    rdfs:subClassOf ai4se:Miscellaneous ;
                    rdfs:comment "Represents a phase in the software development life cycle as e.g. defined in the Software Development Life Cycle Ontology ODYSSEY."@en ;
                    rdfs:isDefinedBy "https://www.scitepress.org/Papers/2018/69577/69577.pdf" ;
                    rdfs:label "SDLC:Phase" .


###  http://purl.org/ai4se/owl#PrMO:Activity
ai4se:PrMO:Activity rdf:type owl:Class ;
                    rdfs:subClassOf ai4se:Miscellaneous ,
                                    gufo:Event ;
                    rdfs:comment """Represents a set of tasks used to produce, operate or maintain software-based products or services as well as to achieve the objectives of the process it belongs to. The activity includes the procedures, standards, policies, and objectives to create and modify a set of work products. 

Adapted to software-related activities from PrMO: an ontology of process-reference models."""@en ;
                    rdfs:isDefinedBy "https://www.redalyc.org/articulo.oa?id=43032606003" ;
                    rdfs:label "PrMO:Activity" .


###  http://purl.org/ai4se/owl#PrMO:Process
ai4se:PrMO:Process rdf:type owl:Class ;
                   rdfs:subClassOf ai4se:Miscellaneous ,
                                   ai4se:PrMO:Activity ;
                   rdfs:comment """Represents a coherent set of policies, organizational structures, technologies; procedures, purposes, objectives, and work products that are needed to design, develop, deploy and maintain a software product.

Defined by PrMO: an ontology of process-reference models"""@en ;
                   rdfs:isDefinedBy "https://www.redalyc.org/articulo.oa?id=43032606003" ;
                   rdfs:label "PrMO:Process" .


###  Generated by the OWL API (version 4.5.29.2024-05-13T12:11:03Z) https://github.com/owlcs/owlapi
